<?xml version="1.0" encoding="UTF-8"?>
<rdf:RDF
	xmlns:rdf="http://www.w3.org/1999/02/22-rdf-syntax-ns#"
	xmlns:rdfs="http://www.w3.org/2000/01/rdf-schema#"
	xmlns:skos="http://www.w3.org/2004/02/skos/core#"
	xmlns:skosxl="http://www.w3.org/2008/05/skos-xl#"
	xmlns:owl="http://www.w3.org/2002/07/owl#"
	xmlns:dc="http://purl.org/dc/elements/1.1/"
	xmlns:dcterms="http://purl.org/dc/terms/"
	xmlns:xsd="http://www.w3.org/2001/XMLSchema#"
	xmlns:tags="http://www.holygoat.co.uk/owl/redwood/0.1/tags/"
	xmlns:foaf="http://xmlns.com/foaf/0.1/"
	xmlns:cycAnnot="http://sw.cyc.com/CycAnnotations_v1#"
	xmlns:csw="http://semantic-web.at/ontologies/csw.owl#"
	xmlns:dbpedia="http://dbpedia.org/resource/"
	xmlns:freebase="http://rdf.freebase.com/ns/"
	xmlns:opencyc="http://sw.opencyc.org/concept/"
	xmlns:cyc="http://sw.cyc.com/concept/"
	xmlns:ctag="http://commontag.org/ns#">

<rdf:Description rdf:about="http://resource.geolba.ac.at/doc/157">
	<dcterms:creator rdf:resource="http://resource.geolba.ac.at/user/schmar"/>
</rdf:Description>

<rdf:Description rdf:about="http://resource.geolba.ac.at/doc/17">
	<dcterms:creator rdf:resource="http://resource.geolba.ac.at/user/schmar"/>
</rdf:Description>

<rdf:Description rdf:about="http://resource.geolba.ac.at/doc/78">
	<dcterms:creator rdf:resource="http://resource.geolba.ac.at/user/schmar"/>
</rdf:Description>

<rdf:Description rdf:about="http://resource.geolba.ac.at/doc/76">
	<dcterms:created rdf:datatype="http://www.w3.org/2001/XMLSchema#dateTime">2014-12-09T13:42:17.000Z</dcterms:created>
</rdf:Description>

<rdf:Description rdf:about="http://resource.geolba.ac.at/doc/45">
	<dcterms:created rdf:datatype="http://www.w3.org/2001/XMLSchema#dateTime">2014-09-25T08:51:07.000Z</dcterms:created>
</rdf:Description>

<rdf:Description rdf:about="http://resource.geolba.ac.at/doc/62">
	<url xmlns="http://www.w3.org/2006/vcard/ns#" rdf:resource="http://www.geologie.ac.at"/>
</rdf:Description>

<rdf:Description rdf:about="http://resource.geolba.ac.at/doc/156">
	<skos:prefLabel xml:lang="en">Geomorphologic units and Lithogenetic Units: Concept schemes and all sub-concepts with definition, scope notes and GBA status (1=official use, 2=informal; 3=obsolete)</skos:prefLabel>
</rdf:Description>

<rdf:Description rdf:about="http://resource.geolba.ac.at/doc/66">
	<rdf:type rdf:resource="http://www.w3.org/2004/02/skos/core#Concept"/>
</rdf:Description>

<rdf:Description rdf:about="http://resource.geolba.ac.at/doc/5">
	<dcterms:creator rdf:resource="http://resource.geolba.ac.at/user/schmar"/>
</rdf:Description>

<rdf:Description rdf:about="http://resource.geolba.ac.at/doc/2">
	<skos:narrower rdf:resource="http://resource.geolba.ac.at/doc/20"/>
</rdf:Description>

<rdf:Description rdf:about="http://resource.geolba.ac.at/doc/48">
	<skos:definition xml:lang="de">Der Thesaurus ist in folgende Hierarchiestufen gegliedert: Themenbereich (z.B. Lithologie) – Konzeptschema (z.B. Lithologische Klassifikation) – Topkonzept (oberstes Konzept im Schema, z.B. Magmatisches Material) – Konzept (= Begriff, z.B. Pyroklastika). Die Konzepte untereinander sind durch übergeordnete, untergeordnete und verwandte Konzepte miteinander vernetzt, wobei ein Konzept auch mehrere übergeordnete Konzepte haben kann (z.B. Magmatisches Material, Sedimentäres Material = Polyhierarchie).</skos:definition>
</rdf:Description>

<rdf:Description rdf:about="http://resource.geolba.ac.at/doc/79">
	<skos:topConceptOf rdf:resource="http://resource.geolba.ac.at/doc/0"/>
</rdf:Description>

<rdf:Description rdf:about="http://resource.geolba.ac.at/doc/165">
	<skos:broader rdf:resource="http://resource.geolba.ac.at/doc/159"/>
</rdf:Description>

<rdf:Description rdf:about="http://resource.geolba.ac.at/doc/9">
	<rdf:type rdf:resource="http://www.w3.org/2004/02/skos/core#Concept"/>
</rdf:Description>

<rdf:Description rdf:about="http://resource.geolba.ac.at/doc/66">
	<skos:definition xml:lang="de">PREFIX rdfs:&lt;http://www.w3.org/2000/01/rdf-schema#&gt;&amp;#xa;PREFIX skos:&lt;http://www.w3.org/2004/02/skos/core#&gt;&amp;#xa;SELECT ?URI ?AT ?PL ?HU &amp;#xa;WHERE { &amp;#xa;?URI a skos:Concept . ?URI skos:prefLabel ?AT . FILTER(lang(?AT)='de') . &amp;#xa;?URI skos:exactMatch ?dbp . FILTER regex(str(?dbp), '^http://dbpedia.org'). &amp;#xa;OPTIONAL {?dbp rdfs:label ?PL . FILTER(lang(?PL)='pl')} &amp;#xa;OPTIONAL {?dbp rdfs:label ?HU . FILTER(lang(?HU)='hu')} &amp;#xa;FILTER (BOUND(?PL) || BOUND(?HU)) &amp;#xa;}</skos:definition>
</rdf:Description>

<rdf:Description rdf:about="http://resource.geolba.ac.at/doc/85">
	<dcterms:created rdf:datatype="http://www.w3.org/2001/XMLSchema#dateTime">2015-03-23T09:26:22.000Z</dcterms:created>
</rdf:Description>

<rdf:Description rdf:about="http://resource.geolba.ac.at/doc/3">
	<skos:prefLabel xml:lang="de">GBA_Tektonische_Einheiten</skos:prefLabel>
</rdf:Description>

<rdf:Description rdf:about="http://resource.geolba.ac.at/doc/156">
	<skos:prefLabel xml:lang="de">Geomorphologische Einheiten und Lithogenetische Einheiten: ConceptSchemes und die untergeordneten Konzepten mit Definitionen, Anwendungshinweise und GBA Status (1=offiziell, 2=informell; 3=obsolete)</skos:prefLabel>
</rdf:Description>

<rdf:Description rdf:about="http://resource.geolba.ac.at/doc/73">
	<dcterms:created rdf:datatype="http://www.w3.org/2001/XMLSchema#dateTime">2014-12-09T13:10:14.000Z</dcterms:created>
</rdf:Description>

<rdf:Description rdf:about="http://resource.geolba.ac.at/doc/62">
	<longitude xmlns="http://www.w3.org/2006/vcard/ns#">16.385588</longitude>
</rdf:Description>

<rdf:Description rdf:about="http://resource.geolba.ac.at/doc/2">
	<skos:narrower rdf:resource="http://resource.geolba.ac.at/doc/21"/>
</rdf:Description>

<rdf:Description rdf:about="http://resource.geolba.ac.at/doc/31">
	<dcterms:created rdf:datatype="http://www.w3.org/2001/XMLSchema#dateTime">2014-07-02T13:26:36.000Z</dcterms:created>
</rdf:Description>

<rdf:Description rdf:about="http://resource.geolba.ac.at/doc/0">
	<skos:hasTopConcept rdf:resource="http://resource.geolba.ac.at/doc/71"/>
</rdf:Description>

<rdf:Description rdf:about="http://resource.geolba.ac.at/doc/35">
	<skos:definition xml:lang="de">http://resource.geolba.ac.at/PoolParty/sparql/minres</skos:definition>
</rdf:Description>

<rdf:Description rdf:about="http://resource.geolba.ac.at/doc/10">
	<dcterms:created rdf:datatype="http://www.w3.org/2001/XMLSchema#dateTime">2014-06-16T13:41:49.000Z</dcterms:created>
</rdf:Description>

<rdf:Description rdf:about="http://resource.geolba.ac.at/doc/82">
	<skos:definition xml:lang="en">Square brackets identify interim labels like wild cards to build the hierarchical structure of the GBA Thesaurus. Especially the 'Austrian Stratigraphical Chart' (Piller et al. 2004) uses this kind of structuring concepts (e.g. toponyms). A further use e.g. for attributing geodata, is not recommended.</skos:definition>
</rdf:Description>

<rdf:Description rdf:about="http://resource.geolba.ac.at/doc/157">
	<skos:prefLabel xml:lang="de">Tektonische Begriffe, die nicht mehr verwendet werden sollten (obsolete)</skos:prefLabel>
</rdf:Description>

<rdf:Description rdf:about="http://resource.geolba.ac.at/doc/164">
	<rdf:type rdf:resource="http://www.w3.org/2004/02/skos/core#Concept"/>
</rdf:Description>

<rdf:Description rdf:about="http://resource.geolba.ac.at/doc/12">
	<owl:deprecated rdf:datatype="http://www.w3.org/2001/XMLSchema#boolean">true</owl:deprecated>
</rdf:Description>

<rdf:Description rdf:about="http://resource.geolba.ac.at/doc/64">
	<owl:deprecated rdf:datatype="http://www.w3.org/2001/XMLSchema#boolean">true</owl:deprecated>
</rdf:Description>

<rdf:Description rdf:about="http://resource.geolba.ac.at/doc/74">
	<dcterms:creator rdf:resource="http://resource.geolba.ac.at/user/schmar"/>
</rdf:Description>

<rdf:Description rdf:about="http://resource.geolba.ac.at/doc/0">
	<skos:hasTopConcept rdf:resource="http://resource.geolba.ac.at/doc/73"/>
</rdf:Description>

<rdf:Description rdf:about="http://resource.geolba.ac.at/doc/61">
	<dcterms:created rdf:datatype="http://www.w3.org/2001/XMLSchema#dateTime">2014-10-27T12:10:08.000Z</dcterms:created>
</rdf:Description>

<rdf:Description rdf:about="http://resource.geolba.ac.at/doc/10">
	<rdf:type rdf:resource="http://www.w3.org/2004/02/skos/core#Concept"/>
</rdf:Description>

<rdf:Description rdf:about="http://resource.geolba.ac.at/doc/76">
	<skos:prefLabel xml:lang="en">Event Environment of Geologic Units</skos:prefLabel>
</rdf:Description>

<rdf:Description rdf:about="http://resource.geolba.ac.at/doc/16">
	<skos:definition xml:lang="de">PREFIX dcterms:&lt;http://purl.org/dc/terms/&gt;&amp;#xa;PREFIX category:&lt;http://dbpedia.org/resource/Category:&gt;&amp;#xa;PREFIX comment:&lt;http://www.w3.org/2000/01/rdf-schema#&gt;&amp;#xa;SELECT DISTINCT ?s ?label ?comment&amp;#xa;WHERE {&amp;#xa;{?s dcterms:subject category:Geology_of_Austria} UNION {?s dcterms:subject category:Geology_of_Switzerland} UNION&amp;#xa;{?s dcterms:subject category:Geology_of_Germany} UNION {?s dcterms:subject category:Geology_of_the_Alps} .&amp;#xa;?s rdfs:label ?label . FILTER(lang(?label)='en') . ?s rdfs:comment ?comment . FILTER(lang(?comment)='en')&amp;#xa;}</skos:definition>
</rdf:Description>

<rdf:Description rdf:about="http://resource.geolba.ac.at/doc/75">
	<skos:topConceptOf rdf:resource="http://resource.geolba.ac.at/doc/0"/>
</rdf:Description>

<rdf:Description rdf:about="http://resource.geolba.ac.at/doc/18">
	<dcterms:created rdf:datatype="http://www.w3.org/2001/XMLSchema#dateTime">2014-06-18T08:24:21.000Z</dcterms:created>
</rdf:Description>

<rdf:Description rdf:about="http://resource.geolba.ac.at/doc/30">
	<skos:broader rdf:resource="http://resource.geolba.ac.at/doc/29"/>
</rdf:Description>

<rdf:Description rdf:about="http://resource.geolba.ac.at/doc/5">
	<rdf:type rdf:resource="http://www.w3.org/2004/02/skos/core#Concept"/>
</rdf:Description>

<rdf:Description rdf:about="http://resource.geolba.ac.at/doc/36">
	<dcterms:created rdf:datatype="http://www.w3.org/2001/XMLSchema#dateTime">2014-09-03T11:25:02.000Z</dcterms:created>
</rdf:Description>

<rdf:Description rdf:about="http://resource.geolba.ac.at/doc/78">
	<dcterms:created rdf:datatype="http://www.w3.org/2001/XMLSchema#dateTime">2014-12-09T14:41:13.000Z</dcterms:created>
</rdf:Description>

<rdf:Description rdf:about="http://resource.geolba.ac.at/doc/65">
	<skos:broader rdf:resource="http://resource.geolba.ac.at/doc/38"/>
</rdf:Description>

<rdf:Description rdf:about="http://resource.geolba.ac.at/doc/16">
	<skos:prefLabel xml:lang="en">Geological concepts from Austria, Germany and Switzerland on Wikipedia including descriptions in English</skos:prefLabel>
</rdf:Description>

<rdf:Description rdf:about="http://resource.geolba.ac.at/doc/78">
	<rdf:type rdf:resource="http://www.w3.org/2004/02/skos/core#Concept"/>
</rdf:Description>

<rdf:Description rdf:about="http://resource.geolba.ac.at/doc/10">
	<dcterms:creator rdf:resource="http://resource.geolba.ac.at/user/schmar"/>
</rdf:Description>

<rdf:Description rdf:about="http://resource.geolba.ac.at/doc/0">
	<skos:hasTopConcept rdf:resource="http://resource.geolba.ac.at/doc/75"/>
</rdf:Description>

<rdf:Description rdf:about="http://resource.geolba.ac.at/doc/157">
	<skos:broader rdf:resource="http://resource.geolba.ac.at/doc/3"/>
</rdf:Description>

<rdf:Description rdf:about="http://resource.geolba.ac.at/doc/86">
	<dcterms:created rdf:datatype="http://www.w3.org/2001/XMLSchema#dateTime">2015-03-23T11:27:41.000Z</dcterms:created>
</rdf:Description>

<rdf:Description rdf:about="http://resource.geolba.ac.at/doc/27">
	<dcterms:created rdf:datatype="http://www.w3.org/2001/XMLSchema#dateTime">2014-07-01T11:03:58.000Z</dcterms:created>
</rdf:Description>

<rdf:Description rdf:about="http://resource.geolba.ac.at/doc/23">
	<dcterms:created rdf:datatype="http://www.w3.org/2001/XMLSchema#dateTime">2014-06-18T09:26:14.000Z</dcterms:created>
</rdf:Description>

<rdf:Description rdf:about="http://resource.geolba.ac.at/doc/46">
	<rdf:type rdf:resource="http://www.w3.org/2004/02/skos/core#Concept"/>
</rdf:Description>

<rdf:Description rdf:about="http://resource.geolba.ac.at/doc/31">
	<skos:topConceptOf rdf:resource="http://resource.geolba.ac.at/doc/0"/>
</rdf:Description>

<rdf:Description rdf:about="http://resource.geolba.ac.at/doc/34">
	<dcterms:hasVersion rdf:datatype="http://www.w3.org/2001/XMLSchema#int">1</dcterms:hasVersion>
</rdf:Description>

<rdf:Description rdf:about="http://resource.geolba.ac.at/doc/8">
	<skos:prefLabel xml:lang="en">Rock names with links to INSPIRE or to GeoSciML</skos:prefLabel>
</rdf:Description>

<rdf:Description rdf:about="http://resource.geolba.ac.at/doc/13">
	<skos:prefLabel xml:lang="de">enipedia (TU Delft)</skos:prefLabel>
</rdf:Description>

<rdf:Description rdf:about="http://resource.geolba.ac.at/doc/19">
	<dcterms:created rdf:datatype="http://www.w3.org/2001/XMLSchema#dateTime">2014-06-18T08:47:11.000Z</dcterms:created>
</rdf:Description>

<rdf:Description rdf:about="http://resource.geolba.ac.at/doc/0">
	<skos:hasTopConcept rdf:resource="http://resource.geolba.ac.at/doc/77"/>
</rdf:Description>

<rdf:Description rdf:about="http://resource.geolba.ac.at/doc/71">
	<skos:narrower rdf:resource="http://resource.geolba.ac.at/doc/72"/>
</rdf:Description>

<rdf:Description rdf:about="http://resource.geolba.ac.at/doc/5">
	<dcterms:hasVersion rdf:datatype="http://www.w3.org/2001/XMLSchema#int">2</dcterms:hasVersion>
</rdf:Description>

<rdf:Description rdf:about="http://resource.geolba.ac.at/doc/40">
	<skos:prefLabel xml:lang="de">Technische Fragen</skos:prefLabel>
</rdf:Description>

<rdf:Description rdf:about="http://resource.geolba.ac.at/doc/0">
	<skos:hasTopConcept rdf:resource="http://resource.geolba.ac.at/doc/79"/>
</rdf:Description>

<rdf:Description rdf:about="http://resource.geolba.ac.at/doc/16">
	<dcterms:created rdf:datatype="http://www.w3.org/2001/XMLSchema#dateTime">2014-06-17T15:19:34.000Z</dcterms:created>
</rdf:Description>

<rdf:Description rdf:about="http://resource.geolba.ac.at/doc/18">
	<skos:prefLabel xml:lang="en">Mountains in Austria higher than 3500m</skos:prefLabel>
</rdf:Description>

<rdf:Description rdf:about="http://resource.geolba.ac.at/doc/0">
	<skos:hasTopConcept rdf:resource="http://resource.geolba.ac.at/doc/31"/>
</rdf:Description>

<rdf:Description rdf:about="http://resource.geolba.ac.at/doc/44">
	<dcterms:modified rdf:datatype="http://www.w3.org/2001/XMLSchema#dateTime">2019-09-30T08:32:28.751Z</dcterms:modified>
</rdf:Description>

<rdf:Description rdf:about="http://resource.geolba.ac.at/doc/81">
	<dcterms:created rdf:datatype="http://www.w3.org/2001/XMLSchema#dateTime">2015-01-09T13:16:55.000Z</dcterms:created>
</rdf:Description>

<rdf:Description rdf:about="http://resource.geolba.ac.at/doc/13">
	<dcterms:creator rdf:resource="http://resource.geolba.ac.at/user/schmar"/>
</rdf:Description>

<rdf:Description rdf:about="http://resource.geolba.ac.at/doc/77">
	<dcterms:created rdf:datatype="http://www.w3.org/2001/XMLSchema#dateTime">2014-12-09T14:39:29.000Z</dcterms:created>
</rdf:Description>

<rdf:Description rdf:about="http://resource.geolba.ac.at/doc/13">
	<rdf:type rdf:resource="http://www.w3.org/2004/02/skos/core#Concept"/>
</rdf:Description>

<rdf:Description rdf:about="http://resource.geolba.ac.at/doc/43">
	<dcterms:created rdf:datatype="http://www.w3.org/2001/XMLSchema#dateTime">2014-09-25T08:48:41.000Z</dcterms:created>
</rdf:Description>

<rdf:Description rdf:about="http://resource.geolba.ac.at/doc/80">
	<dcterms:created rdf:datatype="http://www.w3.org/2001/XMLSchema#dateTime">2014-12-18T13:07:49.000Z</dcterms:created>
</rdf:Description>

<rdf:Description rdf:about="http://resource.geolba.ac.at/doc/1">
	<skos:definition xml:lang="de">http://resource.geolba.ac.at/PoolParty/sparql/lithology</skos:definition>
</rdf:Description>

<rdf:Description rdf:about="http://resource.geolba.ac.at/doc/156">
	<skos:broader rdf:resource="http://resource.geolba.ac.at/doc/2"/>
</rdf:Description>

<rdf:Description rdf:about="http://resource.geolba.ac.at/doc/162">
	<skos:broader rdf:resource="http://resource.geolba.ac.at/doc/159"/>
</rdf:Description>

<rdf:Description rdf:about="http://resource.geolba.ac.at/doc/9">
	<skos:prefLabel xml:lang="de">Gesteinsbegriffe, die weder Links nach INSPIRE noch nach GeoSciML haben</skos:prefLabel>
</rdf:Description>

<rdf:Description rdf:about="http://resource.geolba.ac.at/doc/157">
	<skos:prefLabel xml:lang="en">Tectonic concepts, no longer be used (obsolete)</skos:prefLabel>
</rdf:Description>

<rdf:Description rdf:about="http://resource.geolba.ac.at/doc/45">
	<skos:broader rdf:resource="http://resource.geolba.ac.at/doc/38"/>
</rdf:Description>

<rdf:Description rdf:about="http://resource.geolba.ac.at/doc/84">
	<skos:prefLabel xml:lang="de">Farbangaben in Hexadezimal-Farbcodes (Webfarben)?</skos:prefLabel>
</rdf:Description>

<rdf:Description rdf:about="http://resource.geolba.ac.at/doc/76">
	<skos:definition xml:lang="de">PREFIX skos:&lt;http://www.w3.org/2004/02/skos/core#&gt;&amp;#xa;SELECT ?URI ?prefLabel ?definition&amp;#xa;WHERE&amp;#xa;{&amp;#xa;&lt;http://resource.geosciml.org/classifier/cgi/eventenvironment/earth_surface_setting&gt; skos:narrower* ?URI .&amp;#xa;?URI skos:prefLabel ?prefLabel . ?URI skos:definition ?definition&amp;#xa;}</skos:definition>
</rdf:Description>

<rdf:Description rdf:about="http://resource.geolba.ac.at/doc/25">
	<rdf:type rdf:resource="http://www.w3.org/2004/02/skos/core#Concept"/>
</rdf:Description>

<rdf:Description rdf:about="http://resource.geolba.ac.at/doc/30">
	<skos:prefLabel xml:lang="en">All EEA datasets specified with 'Groundwater'</skos:prefLabel>
</rdf:Description>

<rdf:Description rdf:about="http://resource.geolba.ac.at/doc/84">
	<dcterms:created rdf:datatype="http://www.w3.org/2001/XMLSchema#dateTime">2015-03-23T09:19:58.000Z</dcterms:created>
</rdf:Description>

<rdf:Description rdf:about="http://resource.geolba.ac.at/doc/162">
	<rdf:type rdf:resource="http://www.w3.org/2004/02/skos/core#Concept"/>
</rdf:Description>

<rdf:Description rdf:about="http://resource.geolba.ac.at/doc/14">
	<dcterms:created rdf:datatype="http://www.w3.org/2001/XMLSchema#dateTime">2014-06-17T11:05:57.000Z</dcterms:created>
</rdf:Description>

<rdf:Description rdf:about="http://resource.geolba.ac.at/doc/75">
	<skos:prefLabel xml:lang="de">geosciml.org CGI2012</skos:prefLabel>
	<skos:prefLabel xml:lang="en">geosciml.org CGI2012</skos:prefLabel>
</rdf:Description>

<rdf:Description rdf:about="http://resource.geolba.ac.at/doc/158">
	<dcterms:created rdf:datatype="http://www.w3.org/2001/XMLSchema#dateTime">2018-09-27T06:35:00.000Z</dcterms:created>
</rdf:Description>

<rdf:Description rdf:about="http://resource.geolba.ac.at/doc/28">
	<owl:deprecated rdf:datatype="http://www.w3.org/2001/XMLSchema#boolean">true</owl:deprecated>
</rdf:Description>

<rdf:Description rdf:about="http://resource.geolba.ac.at/doc/62">
	<latitude xmlns="http://www.w3.org/2006/vcard/ns#">48.199245</latitude>
</rdf:Description>

<rdf:Description rdf:about="http://resource.geolba.ac.at/doc/31">
	<skos:prefLabel xml:lang="de">de.dbPedia (Wikipedia DE)</skos:prefLabel>
</rdf:Description>

<rdf:Description rdf:about="http://resource.geolba.ac.at/doc/159">
	<skos:topConceptOf rdf:resource="http://resource.geolba.ac.at/doc/158"/>
</rdf:Description>

<rdf:Description rdf:about="http://resource.geolba.ac.at/doc/3">
	<rdf:type rdf:resource="http://www.w3.org/2004/02/skos/core#Concept"/>
</rdf:Description>

<rdf:Description rdf:about="http://resource.geolba.ac.at/doc/30">
	<skos:prefLabel xml:lang="de">Alle EEA Datensätze mit Groundwater im Titel</skos:prefLabel>
</rdf:Description>

<rdf:Description rdf:about="http://resource.geolba.ac.at/doc/62">
	<tel xmlns="http://www.w3.org/2006/vcard/ns#">+43 1 7125674</tel>
</rdf:Description>

<rdf:Description rdf:about="http://resource.geolba.ac.at/doc/74">
	<skos:broader rdf:resource="http://resource.geolba.ac.at/doc/73"/>
</rdf:Description>

<rdf:Description rdf:about="http://resource.geolba.ac.at/doc/49">
	<rdf:type rdf:resource="http://www.w3.org/2004/02/skos/core#Concept"/>
</rdf:Description>

<rdf:Description rdf:about="http://resource.geolba.ac.at/doc/2">
	<dcterms:hasVersion rdf:datatype="http://www.w3.org/2001/XMLSchema#int">2</dcterms:hasVersion>
</rdf:Description>

<rdf:Description rdf:about="http://resource.geolba.ac.at/doc/50">
	<dcterms:creator rdf:resource="http://resource.geolba.ac.at/user/schmar"/>
</rdf:Description>

<rdf:Description rdf:about="http://resource.geolba.ac.at/doc/0">
	<skos:hasTopConcept rdf:resource="http://resource.geolba.ac.at/doc/13"/>
</rdf:Description>

<rdf:Description rdf:about="http://resource.geolba.ac.at/doc/161">
	<dcterms:creator rdf:resource="http://resource.geolba.ac.at/user/schmar"/>
</rdf:Description>

<rdf:Description rdf:about="http://resource.geolba.ac.at/doc/42">
	<dcterms:created rdf:datatype="http://www.w3.org/2001/XMLSchema#dateTime">2014-09-25T08:48:16.000Z</dcterms:created>
</rdf:Description>

<rdf:Description rdf:about="http://resource.geolba.ac.at/doc/62">
	<dcterms:created rdf:datatype="http://www.w3.org/2001/XMLSchema#dateTime">2014-10-27T12:10:32.000Z</dcterms:created>
</rdf:Description>

<rdf:Description rdf:about="http://resource.geolba.ac.at/doc/82">
	<rdf:type rdf:resource="http://www.w3.org/2004/02/skos/core#Concept"/>
</rdf:Description>

<rdf:Description rdf:about="http://resource.geolba.ac.at/doc/81">
	<skos:prefLabel xml:lang="de">Alle Geologischen Einheiten mit Beschreibung in Deutsch und Englisch</skos:prefLabel>
</rdf:Description>

<rdf:Description rdf:about="http://resource.geolba.ac.at/doc/160">
	<dcterms:created rdf:datatype="http://www.w3.org/2001/XMLSchema#dateTime">2018-09-27T06:35:47.000Z</dcterms:created>
</rdf:Description>

<rdf:Description rdf:about="http://resource.geolba.ac.at/doc/82">
	<skos:prefLabel xml:lang="de">Manche Begriffe sind in eckige Klammern [ ] gesetzt, warum?</skos:prefLabel>
</rdf:Description>

<rdf:Description rdf:about="http://resource.geolba.ac.at/doc/71">
	<dcterms:created rdf:datatype="http://www.w3.org/2001/XMLSchema#dateTime">2014-12-09T10:31:55.000Z</dcterms:created>
</rdf:Description>

<rdf:Description rdf:about="http://resource.geolba.ac.at/doc/165">
	<dcterms:created rdf:datatype="http://www.w3.org/2001/XMLSchema#dateTime">2018-09-27T14:11:46.000Z</dcterms:created>
</rdf:Description>

<rdf:Description rdf:about="http://resource.geolba.ac.at/doc/62">
	<dcterms:creator rdf:resource="http://resource.geolba.ac.at/user/schmar"/>
</rdf:Description>

<rdf:Description rdf:about="http://resource.geolba.ac.at/doc/78">
	<skos:prefLabel xml:lang="en">Building materials of monuments</skos:prefLabel>
</rdf:Description>

<rdf:Description rdf:about="http://resource.geolba.ac.at/doc/164">
	<skos:prefLabel xml:lang="en">Concepts with location and coordinates</skos:prefLabel>
</rdf:Description>

<rdf:Description rdf:about="http://resource.geolba.ac.at/doc/0">
	<skos:hasTopConcept rdf:resource="http://resource.geolba.ac.at/doc/15"/>
</rdf:Description>

<rdf:Description rdf:about="http://resource.geolba.ac.at/doc/18">
	<skos:definition xml:lang="de">PREFIX dbpedia: &lt;http://dbpedia.org/resource/&gt;&amp;#xa;PREFIX gn: &lt;http://www.geonames.org/ontology#&gt;&amp;#xa;PREFIX wgs84_pos: &lt;http://www.w3.org/2003/01/geo/wgs84_pos#&gt;&amp;#xa;&amp;#xa;SELECT ?s ?Berg ?alt&amp;#xa;WHERE {&amp;#xa;    ?s gn:featureCode &lt;http://www.geonames.org/ontology#T.MT&gt; . ?s gn:name ?Berg .&amp;#xa;    ?s gn:countryCode 'AT' . ?s wgs84_pos:alt ?alt . FILTER (xsd:integer(?alt) &gt; 3500) &amp;#xa;}</skos:definition>
</rdf:Description>

<rdf:Description rdf:about="http://resource.geolba.ac.at/doc/31">
	<skos:narrower rdf:resource="http://resource.geolba.ac.at/doc/32"/>
</rdf:Description>

<rdf:Description rdf:about="http://resource.geolba.ac.at/doc/45">
	<dcterms:creator rdf:resource="http://resource.geolba.ac.at/user/schmar"/>
</rdf:Description>

<rdf:Description rdf:about="http://resource.geolba.ac.at/doc/23">
	<skos:prefLabel xml:lang="en">Rocks of volcanic origin (volcanic rock)</skos:prefLabel>
</rdf:Description>

<rdf:Description rdf:about="http://resource.geolba.ac.at/doc/9">
	<dcterms:hasVersion rdf:datatype="http://www.w3.org/2001/XMLSchema#int">9</dcterms:hasVersion>
</rdf:Description>

<rdf:Description rdf:about="http://resource.geolba.ac.at/doc/21">
	<skos:broader rdf:resource="http://resource.geolba.ac.at/doc/2"/>
</rdf:Description>

<rdf:Description rdf:about="http://resource.geolba.ac.at/doc/62">
	<fn xmlns="http://www.w3.org/2006/vcard/ns#" xml:lang="en">Geological Survey of Austria</fn>
</rdf:Description>

<rdf:Description rdf:about="http://resource.geolba.ac.at/doc/65">
	<dcterms:created rdf:datatype="http://www.w3.org/2001/XMLSchema#dateTime">2014-10-28T07:40:48.000Z</dcterms:created>
</rdf:Description>

<rdf:Description rdf:about="http://resource.geolba.ac.at/doc/79">
	<skos:prefLabel xml:lang="de">geoexkursionen</skos:prefLabel>
</rdf:Description>

<rdf:Description rdf:about="http://resource.geolba.ac.at/doc/25">
	<skos:prefLabel xml:lang="de">eurostat</skos:prefLabel>
</rdf:Description>

<rdf:Description rdf:about="http://resource.geolba.ac.at/doc/45">
	<skos:prefLabel xml:lang="en">How do I search for a term and if I don’t know the exact wording?</skos:prefLabel>
</rdf:Description>

<rdf:Description rdf:about="http://resource.geolba.ac.at/doc/72">
	<dcterms:created rdf:datatype="http://www.w3.org/2001/XMLSchema#dateTime">2014-12-09T10:33:28.000Z</dcterms:created>
</rdf:Description>

<rdf:Description rdf:about="http://resource.geolba.ac.at/doc/0">
	<skos:hasTopConcept rdf:resource="http://resource.geolba.ac.at/doc/17"/>
</rdf:Description>

<rdf:Description rdf:about="http://resource.geolba.ac.at/doc/41">
	<skos:prefLabel xml:lang="de">Warum wird der Thesaurus als SKOS-Vokabular geführt?</skos:prefLabel>
</rdf:Description>

<rdf:Description rdf:about="http://resource.geolba.ac.at/doc/62">
	<rdf:type rdf:resource="http://www.w3.org/2004/02/skos/core#Concept"/>
</rdf:Description>

<rdf:Description rdf:about="http://resource.geolba.ac.at/doc/50">
	<skos:prefLabel xml:lang="en">In case of any further questions, to whom can I turn to? </skos:prefLabel>
</rdf:Description>

<rdf:Description rdf:about="http://resource.geolba.ac.at/doc/9">
	<dcterms:created rdf:datatype="http://www.w3.org/2001/XMLSchema#dateTime">2014-06-16T13:30:59.000Z</dcterms:created>
</rdf:Description>

<rdf:Description rdf:about="http://resource.geolba.ac.at/doc/21">
	<dcterms:created rdf:datatype="http://www.w3.org/2001/XMLSchema#dateTime">2014-06-18T09:13:33.000Z</dcterms:created>
</rdf:Description>

<rdf:Description rdf:about="http://resource.geolba.ac.at/doc/86">
	<rdf:type rdf:resource="http://www.w3.org/2004/02/skos/core#Concept"/>
</rdf:Description>

<rdf:Description rdf:about="http://resource.geolba.ac.at/doc/164">
	<dcterms:creator rdf:resource="http://resource.geolba.ac.at/user/schmar"/>
</rdf:Description>

<rdf:Description rdf:about="http://resource.geolba.ac.at/doc/82">
	<skos:broader rdf:resource="http://resource.geolba.ac.at/doc/38"/>
	<skos:prefLabel xml:lang="en">Concept labels in square brackets [ ] ?</skos:prefLabel>
</rdf:Description>

<rdf:Description rdf:about="http://resource.geolba.ac.at/doc/49">
	<dcterms:creator rdf:resource="http://resource.geolba.ac.at/user/schmar"/>
</rdf:Description>

<rdf:Description rdf:about="http://resource.geolba.ac.at/doc/50">
	<rdf:type rdf:resource="http://www.w3.org/2004/02/skos/core#Concept"/>
</rdf:Description>

<rdf:Description rdf:about="http://resource.geolba.ac.at/doc/157">
	<rdf:type rdf:resource="http://www.w3.org/2004/02/skos/core#Concept"/>
</rdf:Description>

<rdf:Description rdf:about="http://resource.geolba.ac.at/doc/13">
	<dcterms:created rdf:datatype="http://www.w3.org/2001/XMLSchema#dateTime">2014-06-17T11:05:23.000Z</dcterms:created>
</rdf:Description>

<rdf:Description rdf:about="http://resource.geolba.ac.at/doc/7">
	<dcterms:created rdf:datatype="http://www.w3.org/2001/XMLSchema#dateTime">2014-06-13T12:35:02.000Z</dcterms:created>
</rdf:Description>

<rdf:Description rdf:about="http://resource.geolba.ac.at/doc/17">
	<rdf:type rdf:resource="http://www.w3.org/2004/02/skos/core#Concept"/>
</rdf:Description>

<rdf:Description rdf:about="http://resource.geolba.ac.at/doc/28">
	<dcterms:hasVersion rdf:datatype="http://www.w3.org/2001/XMLSchema#int">1</dcterms:hasVersion>
</rdf:Description>

<rdf:Description rdf:about="http://resource.geolba.ac.at/doc/19">
	<skos:definition xml:lang="de">PREFIX skos:&lt;http://www.w3.org/2004/02/skos/core#&gt;&amp;#xa;PREFIX geo:&lt;http://www.w3.org/2003/01/geo/wgs84_pos#&gt;&amp;#xa;&amp;#xa;SELECT &amp;#xa;?URI ?prefLabelDE ?lat ?long&amp;#xa;WHERE&amp;#xa;{&amp;#xa;?URI a skos:Concept . ?URI skos:prefLabel ?prefLabelDE . FILTER(lang(?prefLabelDE)='de') .&amp;#xa;?URI geo:lat ?lat  . ?URI geo:long ?long&amp;#xa;}&amp;#xa;ORDER BY ?prefLabelDE</skos:definition>
</rdf:Description>

<rdf:Description rdf:about="http://resource.geolba.ac.at/doc/37">
	<dcterms:creator rdf:resource="http://resource.geolba.ac.at/user/schmar"/>
</rdf:Description>

<rdf:Description rdf:about="http://resource.geolba.ac.at/doc/32">
	<dcterms:created rdf:datatype="http://www.w3.org/2001/XMLSchema#dateTime">2014-07-02T13:27:11.000Z</dcterms:created>
</rdf:Description>

<rdf:Description rdf:about="http://resource.geolba.ac.at/doc/84">
	<skos:prefLabel xml:lang="en">Color specification in hexadecimal codes (web colors)?</skos:prefLabel>
</rdf:Description>

<rdf:Description rdf:about="http://resource.geolba.ac.at/doc/16">
	<skos:broader rdf:resource="http://resource.geolba.ac.at/doc/15"/>
</rdf:Description>

<rdf:Description rdf:about="http://resource.geolba.ac.at/doc/66">
	<skos:prefLabel xml:lang="de">Gesteinsbegriffe mit polnischen und ungarischen Namen aus Wikipedia</skos:prefLabel>
</rdf:Description>

<rdf:Description rdf:about="http://resource.geolba.ac.at/doc/164">
	<dcterms:created rdf:datatype="http://www.w3.org/2001/XMLSchema#dateTime">2018-09-27T14:09:20.000Z</dcterms:created>
</rdf:Description>

<rdf:Description rdf:about="http://resource.geolba.ac.at/doc/49">
	<dcterms:created rdf:datatype="http://www.w3.org/2001/XMLSchema#dateTime">2014-09-25T08:54:14.000Z</dcterms:created>
</rdf:Description>

<rdf:Description rdf:about="http://resource.geolba.ac.at/doc/86">
	<skos:prefLabel xml:lang="de">Worum handelt es sich beim „GBA-Status“?</skos:prefLabel>
</rdf:Description>

<rdf:Description rdf:about="http://resource.geolba.ac.at/doc/75">
	<skos:narrower rdf:resource="http://resource.geolba.ac.at/doc/76"/>
</rdf:Description>

<rdf:Description rdf:about="http://resource.geolba.ac.at/doc/0">
	<dcterms:description xml:lang="de">Sparql Bookmarks</dcterms:description>
</rdf:Description>

<rdf:Description rdf:about="http://resource.geolba.ac.at/doc/41">
	<skos:broader rdf:resource="http://resource.geolba.ac.at/doc/40"/>
</rdf:Description>

<rdf:Description rdf:about="http://resource.geolba.ac.at/doc/82">
	<dcterms:creator rdf:resource="http://resource.geolba.ac.at/user/schmar"/>
</rdf:Description>

<rdf:Description rdf:about="http://resource.geolba.ac.at/doc/16">
	<dcterms:hasVersion rdf:datatype="http://www.w3.org/2001/XMLSchema#int">4</dcterms:hasVersion>
</rdf:Description>

<rdf:Description rdf:about="http://resource.geolba.ac.at/doc/29">
	<rdf:type rdf:resource="http://www.w3.org/2004/02/skos/core#Concept"/>
</rdf:Description>

<rdf:Description rdf:about="http://resource.geolba.ac.at/doc/84">
	<skos:definition xml:lang="de">Bei manchen Konzepten (Thesaurusbegriffen) gibt es Angaben zur farblichen Darstellung. Diese beziehen sich auf die INSPIRE-Datenspezifikation, sowie auf internationale Standards. Die Angabe erfolgt hexadezimal als Webfarbe in RGB, zur Darstellung auf Bildschirmen. Der Link auf color-hex.com bietet weitere Informationen, wie z.B. die Umrechnung in andere Farbmodelle.</skos:definition>
</rdf:Description>

<rdf:Description rdf:about="http://resource.geolba.ac.at/doc/85">
	<skos:prefLabel xml:lang="en">What is a 'Data Viewer' and how to use it?</skos:prefLabel>
</rdf:Description>

<rdf:Description rdf:about="http://resource.geolba.ac.at/doc/33">
	<dcterms:created rdf:datatype="http://www.w3.org/2001/XMLSchema#dateTime">2014-07-02T13:37:03.000Z</dcterms:created>
</rdf:Description>

<rdf:Description rdf:about="http://resource.geolba.ac.at/doc/71">
	<skos:topConceptOf rdf:resource="http://resource.geolba.ac.at/doc/0"/>
</rdf:Description>

<rdf:Description rdf:about="http://resource.geolba.ac.at/doc/2">
	<skos:narrower rdf:resource="http://resource.geolba.ac.at/doc/7"/>
</rdf:Description>

<rdf:Description rdf:about="http://resource.geolba.ac.at/doc/25">
	<dcterms:creator rdf:resource="http://resource.geolba.ac.at/user/schmar"/>
</rdf:Description>

<rdf:Description rdf:about="http://resource.geolba.ac.at/doc/166">
	<dcterms:created rdf:datatype="http://www.w3.org/2001/XMLSchema#dateTime">2018-09-28T06:52:28.000Z</dcterms:created>
</rdf:Description>

<rdf:Description rdf:about="http://resource.geolba.ac.at/doc/75">
	<skos:definition xml:lang="de">http://resource.geosciml.org/sparql/cgi201211</skos:definition>
</rdf:Description>

<rdf:Description rdf:about="http://resource.geolba.ac.at/doc/74">
	<rdf:type rdf:resource="http://www.w3.org/2004/02/skos/core#Concept"/>
</rdf:Description>

<rdf:Description rdf:about="http://resource.geolba.ac.at/doc/11">
	<dcterms:created rdf:datatype="http://www.w3.org/2001/XMLSchema#dateTime">2014-06-16T13:47:16.000Z</dcterms:created>
</rdf:Description>

<rdf:Description rdf:about="http://resource.geolba.ac.at/doc/49">
	<skos:broader rdf:resource="http://resource.geolba.ac.at/doc/39"/>
</rdf:Description>

<rdf:Description rdf:about="http://resource.geolba.ac.at/doc/48">
	<dcterms:created rdf:datatype="http://www.w3.org/2001/XMLSchema#dateTime">2014-09-25T08:53:39.000Z</dcterms:created>
</rdf:Description>

<rdf:Description rdf:about="http://resource.geolba.ac.at/doc/50">
	<dcterms:created rdf:datatype="http://www.w3.org/2001/XMLSchema#dateTime">2014-09-25T08:54:47.000Z</dcterms:created>
</rdf:Description>

<rdf:Description rdf:about="http://resource.geolba.ac.at/doc/21">
	<dcterms:hasVersion rdf:datatype="http://www.w3.org/2001/XMLSchema#int">1</dcterms:hasVersion>
</rdf:Description>

<rdf:Description rdf:about="http://resource.geolba.ac.at/doc/65">
	<rdf:type rdf:resource="http://www.w3.org/2004/02/skos/core#Concept"/>
</rdf:Description>

<rdf:Description rdf:about="http://resource.geolba.ac.at/doc/26">
	<dcterms:created rdf:datatype="http://www.w3.org/2001/XMLSchema#dateTime">2014-06-20T12:49:32.000Z</dcterms:created>
</rdf:Description>

<rdf:Description rdf:about="http://resource.geolba.ac.at/doc/61">
	<dcterms:description xml:lang="de">Organisation</dcterms:description>
</rdf:Description>

<rdf:Description rdf:about="http://resource.geolba.ac.at/doc/65">
	<dcterms:creator rdf:resource="http://resource.geolba.ac.at/user/schmar"/>
</rdf:Description>

<rdf:Description rdf:about="http://resource.geolba.ac.at/doc/42">
	<skos:prefLabel xml:lang="de">Was ist Linked Open Data?</skos:prefLabel>
</rdf:Description>

<rdf:Description rdf:about="http://resource.geolba.ac.at/doc/37">
	<dcterms:title xml:lang="de">FAQ</dcterms:title>
</rdf:Description>

<rdf:Description rdf:about="http://resource.geolba.ac.at/doc/15">
	<skos:definition xml:lang="de">http://dbpedia.org/sparql</skos:definition>
</rdf:Description>

<rdf:Description rdf:about="http://resource.geolba.ac.at/doc/50">
	<skos:broader rdf:resource="http://resource.geolba.ac.at/doc/39"/>
</rdf:Description>

<rdf:Description rdf:about="http://resource.geolba.ac.at/doc/65">
	<skos:prefLabel xml:lang="de">Wie suche ich eine bestimmte 'Lithostratigrafische Einheit'?</skos:prefLabel>
</rdf:Description>

<rdf:Description rdf:about="http://resource.geolba.ac.at/doc/2">
	<dcterms:created rdf:datatype="http://www.w3.org/2001/XMLSchema#dateTime">2014-06-13T09:14:34.000Z</dcterms:created>
</rdf:Description>

<rdf:Description rdf:about="http://resource.geolba.ac.at/doc/77">
	<dcterms:creator rdf:resource="http://resource.geolba.ac.at/user/schmar"/>
</rdf:Description>

<rdf:Description rdf:about="http://resource.geolba.ac.at/doc/38">
	<skos:narrower rdf:resource="http://resource.geolba.ac.at/doc/44"/>
</rdf:Description>

<rdf:Description rdf:about="http://resource.geolba.ac.at/doc/13">
	<skos:narrower rdf:resource="http://resource.geolba.ac.at/doc/14"/>
</rdf:Description>

<rdf:Description rdf:about="http://resource.geolba.ac.at/doc/156">
	<dcterms:creator rdf:resource="http://resource.geolba.ac.at/user/schmar"/>
</rdf:Description>

<rdf:Description rdf:about="http://resource.geolba.ac.at/doc/33">
	<dcterms:hasVersion rdf:datatype="http://www.w3.org/2001/XMLSchema#int">1</dcterms:hasVersion>
</rdf:Description>

<rdf:Description rdf:about="http://resource.geolba.ac.at/doc/41">
	<dcterms:creator rdf:resource="http://resource.geolba.ac.at/user/schmar"/>
</rdf:Description>

<rdf:Description rdf:about="http://resource.geolba.ac.at/doc/77">
	<skos:definition xml:lang="de">http://heritagedata.org/live/sparql</skos:definition>
</rdf:Description>

<rdf:Description rdf:about="http://resource.geolba.ac.at/doc/10">
	<skos:prefLabel xml:lang="de">Lithologische Begriffe (Gesteine) mit Fotos oder Abbildungen</skos:prefLabel>
</rdf:Description>

<rdf:Description rdf:about="http://resource.geolba.ac.at/doc/19">
	<skos:prefLabel xml:lang="en">Stratigraphic units with location and coordinates</skos:prefLabel>
</rdf:Description>

<rdf:Description rdf:about="http://resource.geolba.ac.at/doc/39">
	<dcterms:created rdf:datatype="http://www.w3.org/2001/XMLSchema#dateTime">2014-09-25T08:47:06.000Z</dcterms:created>
</rdf:Description>

<rdf:Description rdf:about="http://resource.geolba.ac.at/doc/26">
	<skos:prefLabel xml:lang="en">Bogs in Austria (from Geonames.org)</skos:prefLabel>
</rdf:Description>

<rdf:Description rdf:about="http://resource.geolba.ac.at/doc/78">
	<skos:broader rdf:resource="http://resource.geolba.ac.at/doc/77"/>
</rdf:Description>

<rdf:Description rdf:about="http://resource.geolba.ac.at/doc/88">
	<dcterms:created rdf:datatype="http://www.w3.org/2001/XMLSchema#dateTime">2015-06-12T08:05:00.000Z</dcterms:created>
</rdf:Description>

<rdf:Description rdf:about="http://resource.geolba.ac.at/doc/38">
	<skos:narrower rdf:resource="http://resource.geolba.ac.at/doc/86"/>
	<skos:narrower rdf:resource="http://resource.geolba.ac.at/doc/84"/>
</rdf:Description>

<rdf:Description rdf:about="http://resource.geolba.ac.at/doc/163">
	<dcterms:created rdf:datatype="http://www.w3.org/2001/XMLSchema#dateTime">2018-09-27T14:06:33.000Z</dcterms:created>
</rdf:Description>

<rdf:Description rdf:about="http://resource.geolba.ac.at/doc/81">
	<skos:broader rdf:resource="http://resource.geolba.ac.at/doc/2"/>
</rdf:Description>

<rdf:Description rdf:about="http://resource.geolba.ac.at/doc/3">
	<skos:topConceptOf rdf:resource="http://resource.geolba.ac.at/doc/0"/>
</rdf:Description>

<rdf:Description rdf:about="http://resource.geolba.ac.at/doc/166">
	<skos:broader rdf:resource="http://resource.geolba.ac.at/doc/159"/>
</rdf:Description>

<rdf:Description rdf:about="http://resource.geolba.ac.at/doc/154">
	<skos:broader rdf:resource="http://resource.geolba.ac.at/doc/38"/>
</rdf:Description>

<rdf:Description rdf:about="http://resource.geolba.ac.at/doc/38">
	<skos:narrower rdf:resource="http://resource.geolba.ac.at/doc/85"/>
</rdf:Description>

<rdf:Description rdf:about="http://resource.geolba.ac.at/doc/77">
	<rdf:type rdf:resource="http://www.w3.org/2004/02/skos/core#Concept"/>
</rdf:Description>

<rdf:Description rdf:about="http://resource.geolba.ac.at/doc/20">
	<dcterms:created rdf:datatype="http://www.w3.org/2001/XMLSchema#dateTime">2014-06-18T09:00:33.000Z</dcterms:created>
</rdf:Description>

<rdf:Description rdf:about="http://resource.geolba.ac.at/doc/1">
	<skos:narrower rdf:resource="http://resource.geolba.ac.at/doc/23"/>
</rdf:Description>

<rdf:Description rdf:about="http://resource.geolba.ac.at/doc/21">
	<rdf:type rdf:resource="http://www.w3.org/2004/02/skos/core#Concept"/>
</rdf:Description>

<rdf:Description rdf:about="http://resource.geolba.ac.at/doc/24">
	<skos:broader rdf:resource="http://resource.geolba.ac.at/doc/3"/>
</rdf:Description>

<rdf:Description rdf:about="http://resource.geolba.ac.at/doc/42">
	<skos:prefLabel xml:lang="en">What is Linked Open Data?</skos:prefLabel>
</rdf:Description>

<rdf:Description rdf:about="http://resource.geolba.ac.at/doc/29">
	<skos:prefLabel xml:lang="de">environment agency EEA</skos:prefLabel>
</rdf:Description>

<rdf:Description rdf:about="http://resource.geolba.ac.at/doc/86">
	<skos:broader rdf:resource="http://resource.geolba.ac.at/doc/38"/>
</rdf:Description>

<rdf:Description rdf:about="http://resource.geolba.ac.at/doc/88">
	<skos:prefLabel xml:lang="en">Geologic units, marked by the GBA editorial team, to official use</skos:prefLabel>
</rdf:Description>

<rdf:Description rdf:about="http://resource.geolba.ac.at/doc/35">
	<skos:narrower rdf:resource="http://resource.geolba.ac.at/doc/36"/>
</rdf:Description>

<rdf:Description rdf:about="http://resource.geolba.ac.at/doc/63">
	<rdfs:label xml:lang="de">GBA_URL</rdfs:label>
</rdf:Description>

<rdf:Description rdf:about="http://resource.geolba.ac.at/doc/5">
	<dcterms:created rdf:datatype="http://www.w3.org/2001/XMLSchema#dateTime">2014-06-13T09:17:22.000Z</dcterms:created>
</rdf:Description>

<rdf:Description rdf:about="http://resource.geolba.ac.at/doc/30">
	<dcterms:created rdf:datatype="http://www.w3.org/2001/XMLSchema#dateTime">2014-07-01T11:43:35.000Z</dcterms:created>
</rdf:Description>

<rdf:Description rdf:about="http://resource.geolba.ac.at/doc/4">
	<skos:prefLabel xml:lang="en">GBA_Timescale</skos:prefLabel>
</rdf:Description>

<rdf:Description rdf:about="http://resource.geolba.ac.at/doc/62">
	<extended-address xmlns="http://www.w3.org/2006/vcard/ns#" xml:lang="en">A-1030 Vienna, Neulinggasse 38</extended-address>
</rdf:Description>

<rdf:Description rdf:about="http://resource.geolba.ac.at/doc/39">
	<rdf:type rdf:resource="http://www.w3.org/2004/02/skos/core#Concept"/>
</rdf:Description>

<rdf:Description rdf:about="http://resource.geolba.ac.at/doc/155">
	<owl:deprecated rdf:datatype="http://www.w3.org/2001/XMLSchema#boolean">true</owl:deprecated>
</rdf:Description>

<rdf:Description rdf:about="http://resource.geolba.ac.at/doc/35">
	<skos:prefLabel xml:lang="de">GBA_Rohstoffgeologie</skos:prefLabel>
</rdf:Description>

<rdf:Description rdf:about="http://resource.geolba.ac.at/doc/2">
	<skos:narrower rdf:resource="http://resource.geolba.ac.at/doc/88"/>
</rdf:Description>

<rdf:Description rdf:about="http://resource.geolba.ac.at/doc/159">
	<rdf:type rdf:resource="http://www.w3.org/2004/02/skos/core#Concept"/>
</rdf:Description>

<rdf:Description rdf:about="http://resource.geolba.ac.at/doc/88">
	<skos:definition xml:lang="de">PREFIX skos:&lt;http://www.w3.org/2004/02/skos/core#&gt;&amp;#xa;PREFIX gba:&lt;http://resource.geolba.ac.at/PoolParty/schema/GBA/&gt;&amp;#xa;SELECT ?URI ?prefLabelDE&amp;#xa;WHERE&amp;#xa;{&amp;#xa;?URI a skos:Concept . ?URI skos:prefLabel ?prefLabelDE . FILTER(lang(?prefLabelDE)='de') .&amp;#xa;?URI gba:GBA_Status ?status . FILTER regex(str(?status), '1')&amp;#xa;}&amp;#xa;ORDER BY ?prefLabelDE</skos:definition>
</rdf:Description>

<rdf:Description rdf:about="http://resource.geolba.ac.at/doc/37">
	<rdf:type rdf:resource="http://www.w3.org/2004/02/skos/core#ConceptScheme"/>
</rdf:Description>

<rdf:Description rdf:about="http://resource.geolba.ac.at/doc/15">
	<dcterms:creator rdf:resource="http://resource.geolba.ac.at/user/schmar"/>
</rdf:Description>

<rdf:Description rdf:about="http://resource.geolba.ac.at/doc/39">
	<skos:narrower rdf:resource="http://resource.geolba.ac.at/doc/49"/>
</rdf:Description>

<rdf:Description rdf:about="http://resource.geolba.ac.at/doc/164">
	<skos:broader rdf:resource="http://resource.geolba.ac.at/doc/159"/>
</rdf:Description>

<rdf:Description rdf:about="http://resource.geolba.ac.at/doc/39">
	<skos:narrower rdf:resource="http://resource.geolba.ac.at/doc/48"/>
</rdf:Description>

<rdf:Description rdf:about="http://resource.geolba.ac.at/doc/40">
	<skos:narrower rdf:resource="http://resource.geolba.ac.at/doc/41"/>
</rdf:Description>

<rdf:Description rdf:about="http://resource.geolba.ac.at/doc/84">
	<rdf:type rdf:resource="http://www.w3.org/2004/02/skos/core#Concept"/>
</rdf:Description>

<rdf:Description rdf:about="http://resource.geolba.ac.at/doc/166">
	<dcterms:creator rdf:resource="http://resource.geolba.ac.at/user/schmar"/>
</rdf:Description>

<rdf:Description rdf:about="http://resource.geolba.ac.at/doc/11">
	<skos:broader rdf:resource="http://resource.geolba.ac.at/doc/1"/>
</rdf:Description>

<rdf:Description rdf:about="http://resource.geolba.ac.at/doc/154">
	<dcterms:creator rdf:resource="http://resource.geolba.ac.at/user/schmar"/>
</rdf:Description>

<rdf:Description rdf:about="http://resource.geolba.ac.at/doc/76">
	<skos:broader rdf:resource="http://resource.geolba.ac.at/doc/75"/>
</rdf:Description>

<rdf:Description rdf:about="http://resource.geolba.ac.at/doc/85">
	<skos:prefLabel xml:lang="de">Was ist der 'DataViewer' und wie ist er zu verwenden?</skos:prefLabel>
</rdf:Description>

<rdf:Description rdf:about="http://resource.geolba.ac.at/doc/84">
	<skos:broader rdf:resource="http://resource.geolba.ac.at/doc/38"/>
</rdf:Description>

<rdf:Description rdf:about="http://resource.geolba.ac.at/doc/23">
	<skos:definition xml:lang="de">PREFIX skos:&lt;http://www.w3.org/2004/02/skos/core#&gt;&amp;#xa;SELECT ?URI ?prefLabelDE ?descDE&amp;#xa;WHERE&amp;#xa;{&amp;#xa;&lt;http://resource.geolba.ac.at/lithology/6&gt; skos:narrower* ?URI .&amp;#xa;?URI skos:prefLabel ?prefLabelDE . FILTER(lang(?prefLabelDE)='de') .&amp;#xa;OPTIONAL {?URI skos:definition ?descDE . FILTER(lang(?descDE)='de')}&amp;#xa;}</skos:definition>
</rdf:Description>

<rdf:Description rdf:about="http://resource.geolba.ac.at/doc/78">
	<skos:definition xml:lang="de">PREFIX skos:&lt;http://www.w3.org/2004/02/skos/core#&gt;&amp;#xa;SELECT ?category ?material ?s&amp;#xa;WHERE&amp;#xa;{  &amp;#xa;&lt;http://purl.org/heritagedata/schemes/eh_tbm/concepts/98216&gt; skos:narrower ?URI .&amp;#xa;?URI skos:prefLabel ?category .&amp;#xa;OPTIONAL {?URI skos:narrower ?s . ?s skos:prefLabel ?material}&amp;#xa;}</skos:definition>
</rdf:Description>

<rdf:Description rdf:about="http://resource.geolba.ac.at/doc/40">
	<skos:narrower rdf:resource="http://resource.geolba.ac.at/doc/43"/>
	<rdf:type rdf:resource="http://www.w3.org/2004/02/skos/core#Concept"/>
</rdf:Description>

<rdf:Description rdf:about="http://resource.geolba.ac.at/doc/72">
	<skos:definition xml:lang="de">PREFIX skos:&lt;http://www.w3.org/2004/02/skos/core#&gt;&amp;#xa;SELECT ?URI ?prefLabelDE ?prefLabelEN ?prefLabelFR ?prefLabelES&amp;#xa;WHERE&amp;#xa;{&amp;#xa;&lt;http://reegle.info/glossary/973&gt; skos:narrower* ?URI .&amp;#xa;?URI skos:prefLabel ?prefLabelDE . FILTER(lang(?prefLabelDE)='de') .&amp;#xa;OPTIONAL {?URI skos:prefLabel ?prefLabelEN . FILTER(lang(?prefLabelEN)='en')}&amp;#xa;OPTIONAL {?URI skos:prefLabel ?prefLabelFR . FILTER(lang(?prefLabelFR)='fr')}&amp;#xa;OPTIONAL {?URI skos:prefLabel ?prefLabelES . FILTER(lang(?prefLabelES)='es')}&amp;#xa;}</skos:definition>
</rdf:Description>

<rdf:Description rdf:about="http://resource.geolba.ac.at/doc/32">
	<skos:prefLabel xml:lang="en">Triassic rock units on Wikipedia including descriptions in German</skos:prefLabel>
</rdf:Description>

<rdf:Description rdf:about="http://resource.geolba.ac.at/doc/8">
	<dcterms:creator rdf:resource="http://resource.geolba.ac.at/user/schmar"/>
</rdf:Description>

<rdf:Description rdf:about="http://resource.geolba.ac.at/doc/0">
	<dcterms:hasVersion rdf:datatype="http://www.w3.org/2001/XMLSchema#int">2</dcterms:hasVersion>
</rdf:Description>

<rdf:Description rdf:about="http://resource.geolba.ac.at/doc/40">
	<skos:narrower rdf:resource="http://resource.geolba.ac.at/doc/42"/>
</rdf:Description>

<rdf:Description rdf:about="http://resource.geolba.ac.at/doc/86">
	<skos:prefLabel xml:lang="en">What is the „GBA-Status“ about?</skos:prefLabel>
</rdf:Description>

<rdf:Description rdf:about="http://resource.geolba.ac.at/doc/24">
	<skos:prefLabel xml:lang="de">Alle tektonischen Einheiten der Kategorie 'Decke' innerhalb des Oberostalpin</skos:prefLabel>
</rdf:Description>

<rdf:Description rdf:about="http://resource.geolba.ac.at/doc/155">
	<rdfs:label xml:lang="de">Geomorphologie und Lithogenetik: ConceptSchemes und die untergeordneten Konzepte mit Definitionen, Anwendungshinweise und GBA Status (1=official use, 2=informal; 3=obsolete), wenn vorhanden</rdfs:label>
</rdf:Description>

<rdf:Description rdf:about="http://resource.geolba.ac.at/doc/17">
	<skos:prefLabel xml:lang="de">factForge</skos:prefLabel>
</rdf:Description>

<rdf:Description rdf:about="http://resource.geolba.ac.at/doc/62">
	<fn xmlns="http://www.w3.org/2006/vcard/ns#" xml:lang="de">Geologische Bundesanstalt</fn>
</rdf:Description>

<rdf:Description rdf:about="http://resource.geolba.ac.at/doc/39">
	<skos:narrower rdf:resource="http://resource.geolba.ac.at/doc/50"/>
</rdf:Description>

<rdf:Description rdf:about="http://resource.geolba.ac.at/doc/167">
	<rdf:type rdf:resource="http://www.w3.org/2004/02/skos/core#Concept"/>
</rdf:Description>

<rdf:Description rdf:about="http://resource.geolba.ac.at/doc/32">
	<skos:prefLabel xml:lang="de">Gesteinseinheiten der Trias aus Wikipedia mit Beschreibungen auf Deutsch</skos:prefLabel>
</rdf:Description>

<rdf:Description rdf:about="http://resource.geolba.ac.at/doc/7">
	<skos:prefLabel xml:lang="de">Alle TopConcepts und ConceptSchemes im Thesaurus Geologische Einheiten</skos:prefLabel>
</rdf:Description>

<rdf:Description rdf:about="http://resource.geolba.ac.at/doc/11">
	<skos:prefLabel xml:lang="en">Lithological concepts (rock) including links to Dbpedia (Wikipedia)</skos:prefLabel>
</rdf:Description>

<rdf:Description rdf:about="http://resource.geolba.ac.at/doc/4">
	<skos:definition xml:lang="de">http://resource.geolba.ac.at/PoolParty/sparql/GeologicTimeScale</skos:definition>
</rdf:Description>

<rdf:Description rdf:about="http://resource.geolba.ac.at/doc/43">
	<skos:prefLabel xml:lang="en">Can I download or export individually created lists of information from the Thesaurus?</skos:prefLabel>
</rdf:Description>

<rdf:Description rdf:about="http://resource.geolba.ac.at/doc/18">
	<rdf:type rdf:resource="http://www.w3.org/2004/02/skos/core#Concept"/>
</rdf:Description>

<rdf:Description rdf:about="http://resource.geolba.ac.at/doc/38">
	<skos:narrower rdf:resource="http://resource.geolba.ac.at/doc/65"/>
</rdf:Description>

<rdf:Description rdf:about="http://resource.geolba.ac.at/doc/31">
	<rdf:type rdf:resource="http://www.w3.org/2004/02/skos/core#Concept"/>
</rdf:Description>

<rdf:Description rdf:about="http://resource.geolba.ac.at/doc/66">
	<skos:prefLabel xml:lang="en">Rock names including polish and hungarian translations from Wikipedia</skos:prefLabel>
</rdf:Description>

<rdf:Description rdf:about="http://resource.geolba.ac.at/doc/162">
	<skos:prefLabel xml:lang="en">All concepts with descriptions in German and English</skos:prefLabel>
</rdf:Description>

<rdf:Description rdf:about="http://resource.geolba.ac.at/doc/8">
	<dcterms:hasVersion rdf:datatype="http://www.w3.org/2001/XMLSchema#int">6</dcterms:hasVersion>
</rdf:Description>

<rdf:Description rdf:about="http://resource.geolba.ac.at/doc/13">
	<skos:definition xml:lang="de">http://enipedia.tudelft.nl/sparql/</skos:definition>
</rdf:Description>

<rdf:Description rdf:about="http://resource.geolba.ac.at/doc/62">
	<skos:prefLabel xml:lang="en">Geological Survey of Austria</skos:prefLabel>
</rdf:Description>

<rdf:Description rdf:about="http://resource.geolba.ac.at/doc/7">
	<skos:prefLabel xml:lang="en">All top concepts and concept schemes for geologic units</skos:prefLabel>
</rdf:Description>

<rdf:Description rdf:about="http://resource.geolba.ac.at/doc/18">
	<dcterms:creator rdf:resource="http://resource.geolba.ac.at/user/schmar"/>
</rdf:Description>

<rdf:Description rdf:about="http://resource.geolba.ac.at/doc/43">
	<skos:broader rdf:resource="http://resource.geolba.ac.at/doc/40"/>
</rdf:Description>

<rdf:Description rdf:about="http://resource.geolba.ac.at/doc/27">
	<skos:scopeNote xml:lang="de">10 Autoren aus der Gemeinsamen Normdatei (GND), die eine Publikation über den Dachstein verfasst haben.</skos:scopeNote>
</rdf:Description>

<rdf:Description rdf:about="http://resource.geolba.ac.at/doc/1">
	<skos:prefLabel xml:lang="en">GBA_Lithology</skos:prefLabel>
</rdf:Description>

<rdf:Description rdf:about="http://resource.geolba.ac.at/doc/31">
	<dcterms:hasVersion rdf:datatype="http://www.w3.org/2001/XMLSchema#int">1</dcterms:hasVersion>
</rdf:Description>

<rdf:Description rdf:about="http://resource.geolba.ac.at/doc/71">
	<skos:definition xml:lang="de">http://poolparty.reegle.info/PoolParty/sparql/glossary</skos:definition>
</rdf:Description>

<rdf:Description rdf:about="http://resource.geolba.ac.at/doc/3">
	<skos:narrower rdf:resource="http://resource.geolba.ac.at/doc/157"/>
</rdf:Description>

<rdf:Description rdf:about="http://resource.geolba.ac.at/doc/10">
	<skos:definition xml:lang="de">PREFIX skos:&lt;http://www.w3.org/2004/02/skos/core#&gt;&amp;#xa;PREFIX foaf:&lt;http://xmlns.com/foaf/0.1/&gt;&amp;#xa;SELECT ?URI ?prefLabelDE ?foto&amp;#xa;WHERE {&amp;#xa;?URI a skos:Concept . ?URI skos:prefLabel ?prefLabelDE . FILTER(lang(?prefLabelDE)='de') .&amp;#xa;?URI foaf:depiction ?foto&amp;#xa;}&amp;#xa;ORDER BY ?prefLabelDE</skos:definition>
</rdf:Description>

<rdf:Description rdf:about="http://resource.geolba.ac.at/doc/14">
	<skos:broader rdf:resource="http://resource.geolba.ac.at/doc/13"/>
</rdf:Description>

<rdf:Description rdf:about="http://resource.geolba.ac.at/doc/61">
	<rdf:type rdf:resource="http://www.w3.org/2004/02/skos/core#ConceptScheme"/>
</rdf:Description>

<rdf:Description rdf:about="http://resource.geolba.ac.at/doc/8">
	<rdf:type rdf:resource="http://www.w3.org/2004/02/skos/core#Concept"/>
</rdf:Description>

<rdf:Description rdf:about="http://resource.geolba.ac.at/doc/62">
	<foaf:name xml:lang="en">Geological Survey of Austria</foaf:name>
</rdf:Description>

<rdf:Description rdf:about="http://resource.geolba.ac.at/doc/23">
	<skos:prefLabel xml:lang="de">Gesteine vulkanischen Ursprungs (Vulkanite) im GBA Thesaurus</skos:prefLabel>
</rdf:Description>

<rdf:Description rdf:about="http://resource.geolba.ac.at/doc/11">
	<skos:definition xml:lang="de">PREFIX skos:&lt;http://www.w3.org/2004/02/skos/core#&gt;&amp;#xa;SELECT ?URI ?prefLabelDE ?DBpedia&amp;#xa;WHERE {&amp;#xa;?URI a skos:Concept . ?URI skos:prefLabel ?prefLabelDE . FILTER(lang(?prefLabelDE)='de') .&amp;#xa;?URI ?p ?DBpedia . FILTER regex(str(?DBpedia), '^http://dbpedia.org')&amp;#xa;}&amp;#xa;ORDER BY ?prefLabelDE&amp;#xa;</skos:definition>
</rdf:Description>

<rdf:Description rdf:about="http://resource.geolba.ac.at/doc/43">
	<rdf:type rdf:resource="http://www.w3.org/2004/02/skos/core#Concept"/>
</rdf:Description>

<rdf:Description rdf:about="http://resource.geolba.ac.at/doc/32">
	<skos:broader rdf:resource="http://resource.geolba.ac.at/doc/31"/>
</rdf:Description>

<rdf:Description rdf:about="http://resource.geolba.ac.at/doc/47">
	<skos:definition xml:lang="de">Ein Thesaurus ist eine Sammlung von Begriffen (=Konzepte), die im Gegensatz zu anderen Begriffssammlungen (z.B. Glossar, Lexikon, Wörterbuch, etc.) die Beziehungen der Begriffe zueinander definiert (Übergeordnete, untergeordnete und verwandte Begriffe), und damit die Bedeutung der Begriffe (Semantik) zusätzlich zur Begriffsbeschreibung präzisiert.</skos:definition>
</rdf:Description>

<rdf:Description rdf:about="http://resource.geolba.ac.at/doc/80">
	<rdf:type rdf:resource="http://www.w3.org/2004/02/skos/core#Concept"/>
</rdf:Description>

<rdf:Description rdf:about="http://resource.geolba.ac.at/doc/14">
	<skos:prefLabel xml:lang="en">Geothermal power plants worldwide</skos:prefLabel>
</rdf:Description>

<rdf:Description rdf:about="http://resource.geolba.ac.at/doc/0">
	<dcterms:modified rdf:datatype="http://www.w3.org/2001/XMLSchema#dateTime">2019-08-09T06:47:43.611Z</dcterms:modified>
</rdf:Description>

<rdf:Description rdf:about="http://resource.geolba.ac.at/doc/158">
	<dcterms:creator rdf:resource="http://resource.geolba.ac.at/user/schmar"/>
</rdf:Description>

<rdf:Description rdf:about="http://resource.geolba.ac.at/doc/4">
	<rdf:type rdf:resource="http://www.w3.org/2004/02/skos/core#Concept"/>
</rdf:Description>

<rdf:Description rdf:about="http://resource.geolba.ac.at/doc/1">
	<skos:topConceptOf rdf:resource="http://resource.geolba.ac.at/doc/0"/>
</rdf:Description>

<rdf:Description rdf:about="http://resource.geolba.ac.at/doc/47">
	<skos:prefLabel xml:lang="en">What is a Thesaurus?</skos:prefLabel>
</rdf:Description>

<rdf:Description rdf:about="http://resource.geolba.ac.at/doc/11">
	<rdf:type rdf:resource="http://www.w3.org/2004/02/skos/core#Concept"/>
</rdf:Description>

<rdf:Description rdf:about="http://resource.geolba.ac.at/doc/40">
	<skos:prefLabel xml:lang="en">technical issues</skos:prefLabel>
</rdf:Description>

<rdf:Description rdf:about="http://resource.geolba.ac.at/doc/4">
	<dcterms:creator rdf:resource="http://resource.geolba.ac.at/user/schmar"/>
</rdf:Description>

<rdf:Description rdf:about="http://resource.geolba.ac.at/doc/87">
	<owl:deprecated rdf:datatype="http://www.w3.org/2001/XMLSchema#boolean">true</owl:deprecated>
</rdf:Description>

<rdf:Description rdf:about="http://resource.geolba.ac.at/doc/23">
	<rdf:type rdf:resource="http://www.w3.org/2004/02/skos/core#Concept"/>
</rdf:Description>

<rdf:Description rdf:about="http://resource.geolba.ac.at/doc/158">
	<dcterms:title xml:lang="de">Bookmarks</dcterms:title>
</rdf:Description>

<rdf:Description rdf:about="http://resource.geolba.ac.at/doc/163">
	<rdf:type rdf:resource="http://www.w3.org/2004/02/skos/core#Concept"/>
</rdf:Description>

<rdf:Description rdf:about="http://resource.geolba.ac.at/doc/75">
	<dcterms:creator rdf:resource="http://resource.geolba.ac.at/user/schmar"/>
</rdf:Description>

<rdf:Description rdf:about="http://resource.geolba.ac.at/doc/62">
	<street-address xmlns="http://www.w3.org/2006/vcard/ns#">Neulinggasse 38</street-address>
</rdf:Description>

<rdf:Description rdf:about="http://resource.geolba.ac.at/doc/77">
	<skos:prefLabel xml:lang="en">GB heritage data</skos:prefLabel>
</rdf:Description>

<rdf:Description rdf:about="http://resource.geolba.ac.at/doc/10">
	<skos:prefLabel xml:lang="en">Lithological concepts (rock) including images or depictions</skos:prefLabel>
</rdf:Description>

<rdf:Description rdf:about="http://resource.geolba.ac.at/doc/3">
	<skos:narrower rdf:resource="http://resource.geolba.ac.at/doc/24"/>
</rdf:Description>

<rdf:Description rdf:about="http://resource.geolba.ac.at/doc/35">
	<rdf:type rdf:resource="http://www.w3.org/2004/02/skos/core#Concept"/>
</rdf:Description>

<rdf:Description rdf:about="http://resource.geolba.ac.at/doc/11">
	<dcterms:hasVersion rdf:datatype="http://www.w3.org/2001/XMLSchema#int">2</dcterms:hasVersion>
</rdf:Description>

<rdf:Description rdf:about="http://resource.geolba.ac.at/doc/64">
	<rdfs:label xml:lang="de">GBA_GEO</rdfs:label>
</rdf:Description>

<rdf:Description rdf:about="http://resource.geolba.ac.at/doc/43">
	<dcterms:creator rdf:resource="http://resource.geolba.ac.at/user/schmar"/>
</rdf:Description>

<rdf:Description rdf:about="http://resource.geolba.ac.at/doc/23">
	<dcterms:hasVersion rdf:datatype="http://www.w3.org/2001/XMLSchema#int">1</dcterms:hasVersion>
</rdf:Description>

<rdf:Description rdf:about="http://resource.geolba.ac.at/doc/48">
	<skos:prefLabel xml:lang="en">How does the hierarchy work in the Thesaurus?</skos:prefLabel>
</rdf:Description>

<rdf:Description rdf:about="http://resource.geolba.ac.at/doc/24">
	<skos:definition xml:lang="de">PREFIX skos:&lt;http://www.w3.org/2004/02/skos/core#&gt;&amp;#xa;SELECT ?s ?prefLabelDE&amp;#xa;WHERE {&amp;#xa;&lt;http://resource.geolba.ac.at/tectonicunit/115&gt; skos:narrower* ?s . &amp;#xa;?s skos:prefLabel ?prefLabelDE . FILTER(lang(?prefLabelDE)='de') .&amp;#xa;?s skos:related &lt;http://resource.geolba.ac.at/tectonicunit/15&gt;&amp;#xa;}</skos:definition>
</rdf:Description>

<rdf:Description rdf:about="http://resource.geolba.ac.at/doc/77">
	<skos:prefLabel xml:lang="de">heritage data (GB)</skos:prefLabel>
</rdf:Description>

<rdf:Description rdf:about="http://resource.geolba.ac.at/doc/0">
	<dcterms:description xml:lang="de">&amp; # x a ; (HTML Codierung) als Zeilenumbruch für die SPARQL-Abfragen verwenden</dcterms:description>
</rdf:Description>

<rdf:Description rdf:about="http://resource.geolba.ac.at/doc/44">
	<skos:broader rdf:resource="http://resource.geolba.ac.at/doc/38"/>
</rdf:Description>

<rdf:Description rdf:about="http://resource.geolba.ac.at/doc/86">
	<dcterms:creator rdf:resource="http://resource.geolba.ac.at/user/horchr"/>
</rdf:Description>

<rdf:Description rdf:about="http://resource.geolba.ac.at/doc/31">
	<dcterms:creator rdf:resource="http://resource.geolba.ac.at/user/schmar"/>
</rdf:Description>

<rdf:Description rdf:about="http://resource.geolba.ac.at/doc/3">
	<skos:prefLabel xml:lang="en">GBA_TectonicUnits</skos:prefLabel>
</rdf:Description>

<rdf:Description rdf:about="http://resource.geolba.ac.at/doc/79">
	<rdf:type rdf:resource="http://www.w3.org/2004/02/skos/core#Concept"/>
</rdf:Description>

<rdf:Description rdf:about="http://resource.geolba.ac.at/doc/74">
	<dcterms:created rdf:datatype="http://www.w3.org/2001/XMLSchema#dateTime">2014-12-09T13:10:54.000Z</dcterms:created>
</rdf:Description>

<rdf:Description rdf:about="http://resource.geolba.ac.at/doc/71">
	<rdf:type rdf:resource="http://www.w3.org/2004/02/skos/core#Concept"/>
</rdf:Description>

<rdf:Description rdf:about="http://resource.geolba.ac.at/doc/27">
	<dcterms:hasVersion rdf:datatype="http://www.w3.org/2001/XMLSchema#int">10</dcterms:hasVersion>
</rdf:Description>

<rdf:Description rdf:about="http://resource.geolba.ac.at/doc/71">
	<dcterms:creator rdf:resource="http://resource.geolba.ac.at/user/schmar"/>
</rdf:Description>

<rdf:Description rdf:about="http://resource.geolba.ac.at/doc/1">
	<skos:narrower rdf:resource="http://resource.geolba.ac.at/doc/8"/>
</rdf:Description>

<rdf:Description rdf:about="http://resource.geolba.ac.at/doc/48">
	<skos:definition xml:lang="en">The Thesaurus is structured in the following hierarchy levels: Domain (e.g. Lithology) – concept scheme (e.g. lithological classification) – top concept (uppermost concept in the scheme, e.g. igneous material) – concept (=term, e.g. pyroclastics). The concepts are linked to each other via superordinate, subordinated or related concepts. One concept can have more than just one superordinate concept (e.g. igneous material, sedimentary material = poly hierarchy).</skos:definition>
</rdf:Description>

<rdf:Description rdf:about="http://resource.geolba.ac.at/doc/46">
	<skos:prefLabel xml:lang="en">Why are there identical terms in various domains?</skos:prefLabel>
</rdf:Description>

<rdf:Description rdf:about="http://resource.geolba.ac.at/doc/15">
	<skos:topConceptOf rdf:resource="http://resource.geolba.ac.at/doc/0"/>
</rdf:Description>

<rdf:Description rdf:about="http://resource.geolba.ac.at/doc/5">
	<skos:definition xml:lang="de">http://resource.geolba.ac.at/PoolParty/sparql/structure</skos:definition>
</rdf:Description>

<rdf:Description rdf:about="http://resource.geolba.ac.at/doc/2">
	<dcterms:creator rdf:resource="http://resource.geolba.ac.at/user/schmar"/>
</rdf:Description>

<rdf:Description rdf:about="http://resource.geolba.ac.at/doc/83">
	<rdf:type rdf:resource="http://www.w3.org/2004/02/skos/core#Concept"/>
</rdf:Description>

<rdf:Description rdf:about="http://resource.geolba.ac.at/doc/45">
	<skos:prefLabel xml:lang="de">Wie suche ich nach einem Begriff, auch wenn ich den exakten Wortlaut nicht kenne?</skos:prefLabel>
</rdf:Description>

<rdf:Description rdf:about="http://resource.geolba.ac.at/doc/2">
	<rdf:type rdf:resource="http://www.w3.org/2004/02/skos/core#Concept"/>
	<skos:prefLabel xml:lang="en">GBA_GeologicUnit</skos:prefLabel>
</rdf:Description>

<rdf:Description rdf:about="http://resource.geolba.ac.at/doc/161">
	<skos:broader rdf:resource="http://resource.geolba.ac.at/doc/159"/>
</rdf:Description>

<rdf:Description rdf:about="http://resource.geolba.ac.at/doc/25">
	<dcterms:created rdf:datatype="http://www.w3.org/2001/XMLSchema#dateTime">2014-06-20T08:12:45.000Z</dcterms:created>
</rdf:Description>

<rdf:Description rdf:about="http://resource.geolba.ac.at/doc/8">
	<dcterms:created rdf:datatype="http://www.w3.org/2001/XMLSchema#dateTime">2014-06-16T12:01:52.000Z</dcterms:created>
</rdf:Description>

<rdf:Description rdf:about="http://resource.geolba.ac.at/doc/15">
	<skos:prefLabel xml:lang="de">dbPedia.org (Wikipedia)</skos:prefLabel>
</rdf:Description>

<rdf:Description rdf:about="http://resource.geolba.ac.at/doc/35">
	<dcterms:created rdf:datatype="http://www.w3.org/2001/XMLSchema#dateTime">2014-09-03T11:23:23.000Z</dcterms:created>
</rdf:Description>

<rdf:Description rdf:about="http://resource.geolba.ac.at/doc/41">
	<dcterms:created rdf:datatype="http://www.w3.org/2001/XMLSchema#dateTime">2014-09-25T08:47:52.000Z</dcterms:created>
</rdf:Description>

<rdf:Description rdf:about="http://resource.geolba.ac.at/doc/157">
	<dcterms:created rdf:datatype="http://www.w3.org/2001/XMLSchema#dateTime">2016-10-19T12:54:23.000Z</dcterms:created>
</rdf:Description>

<rdf:Description rdf:about="http://resource.geolba.ac.at/doc/62">
	<region xmlns="http://www.w3.org/2006/vcard/ns#" xml:lang="de">Wien</region>
</rdf:Description>

<rdf:Description rdf:about="http://resource.geolba.ac.at/doc/17">
	<dcterms:created rdf:datatype="http://www.w3.org/2001/XMLSchema#dateTime">2014-06-18T08:23:18.000Z</dcterms:created>
</rdf:Description>

<rdf:Description rdf:about="http://resource.geolba.ac.at/doc/83">
	<dcterms:creator rdf:resource="http://resource.geolba.ac.at/user/schmar"/>
</rdf:Description>

<rdf:Description rdf:about="http://resource.geolba.ac.at/doc/44">
	<skos:prefLabel xml:lang="de">Wie finde ich Begriffe (=Konzepte), die auf INSPIRE-Codes verlinkt sind?</skos:prefLabel>
</rdf:Description>

<rdf:Description rdf:about="http://resource.geolba.ac.at/doc/27">
	<skos:topConceptOf rdf:resource="http://resource.geolba.ac.at/doc/0"/>
</rdf:Description>

<rdf:Description rdf:about="http://resource.geolba.ac.at/doc/38">
	<dcterms:created rdf:datatype="http://www.w3.org/2001/XMLSchema#dateTime">2014-09-25T08:46:43.000Z</dcterms:created>
</rdf:Description>

<rdf:Description rdf:about="http://resource.geolba.ac.at/doc/25">
	<dcterms:hasVersion rdf:datatype="http://www.w3.org/2001/XMLSchema#int">1</dcterms:hasVersion>
</rdf:Description>

<rdf:Description rdf:about="http://resource.geolba.ac.at/doc/46">
	<dcterms:creator rdf:resource="http://resource.geolba.ac.at/user/schmar"/>
</rdf:Description>

<rdf:Description rdf:about="http://resource.geolba.ac.at/doc/29">
	<dcterms:created rdf:datatype="http://www.w3.org/2001/XMLSchema#dateTime">2014-07-01T11:43:12.000Z</dcterms:created>
</rdf:Description>

<rdf:Description rdf:about="http://resource.geolba.ac.at/doc/0">
	<skos:hasTopConcept rdf:resource="http://resource.geolba.ac.at/doc/25"/>
</rdf:Description>

<rdf:Description rdf:about="http://resource.geolba.ac.at/doc/37">
	<dcterms:created rdf:datatype="http://www.w3.org/2001/XMLSchema#dateTime">2014-09-25T08:46:08.000Z</dcterms:created>
</rdf:Description>

<rdf:Description rdf:about="http://resource.geolba.ac.at/doc/162">
	<dcterms:created rdf:datatype="http://www.w3.org/2001/XMLSchema#dateTime">2018-09-27T14:03:19.000Z</dcterms:created>
</rdf:Description>

<rdf:Description rdf:about="http://resource.geolba.ac.at/doc/19">
	<skos:broader rdf:resource="http://resource.geolba.ac.at/doc/2"/>
</rdf:Description>

<rdf:Description rdf:about="http://resource.geolba.ac.at/doc/14">
	<rdf:type rdf:resource="http://www.w3.org/2004/02/skos/core#Concept"/>
</rdf:Description>

<rdf:Description rdf:about="http://resource.geolba.ac.at/doc/7">
	<skos:broader rdf:resource="http://resource.geolba.ac.at/doc/2"/>
</rdf:Description>

<rdf:Description rdf:about="http://resource.geolba.ac.at/doc/82">
	<dcterms:created rdf:datatype="http://www.w3.org/2001/XMLSchema#dateTime">2015-03-23T07:58:42.000Z</dcterms:created>
</rdf:Description>

<rdf:Description rdf:about="http://resource.geolba.ac.at/doc/161">
	<rdf:type rdf:resource="http://www.w3.org/2004/02/skos/core#Concept"/>
</rdf:Description>

<rdf:Description rdf:about="http://resource.geolba.ac.at/doc/13">
	<dcterms:hasVersion rdf:datatype="http://www.w3.org/2001/XMLSchema#int">5</dcterms:hasVersion>
</rdf:Description>

<rdf:Description rdf:about="http://resource.geolba.ac.at/doc/0">
	<skos:hasTopConcept rdf:resource="http://resource.geolba.ac.at/doc/29"/>
</rdf:Description>

<rdf:Description rdf:about="http://resource.geolba.ac.at/doc/74">
	<skos:definition xml:lang="de">PREFIX dc:&lt;http://purl.org/dc/elements/1.1/&gt;&amp;#xa;PREFIX n0pred: &lt;http://reegle.info/schema#&gt;&amp;#xa;SELECT ?project ?title ?mainActivities ?expectedImpact ?purpose ?background ?budget&amp;#xa;WHERE &amp;#xa;{&amp;#xa; ?project a &lt;http://reegle.info/schema#Project&gt; . &amp;#xa;?project dc:title ?title;&amp;#xa;n0pred:mainActivities ?mainActivities;&amp;#xa;n0pred:expectedImpact ?expectedImpact;&amp;#xa;n0pred:budget ?budget;&amp;#xa;n0pred:purpose ?purpose . FILTER regex(str(?mainActivities), 'geothermal')&amp;#xa;OPTIONAL {?project n0pred:background ?background}&amp;#xa;} </skos:definition>
</rdf:Description>

<rdf:Description rdf:about="http://resource.geolba.ac.at/doc/1">
	<dcterms:created rdf:datatype="http://www.w3.org/2001/XMLSchema#dateTime">2014-06-13T09:13:50.000Z</dcterms:created>
</rdf:Description>

<rdf:Description rdf:about="http://resource.geolba.ac.at/doc/36">
	<skos:broader rdf:resource="http://resource.geolba.ac.at/doc/35"/>
</rdf:Description>

<rdf:Description rdf:about="http://resource.geolba.ac.at/doc/47">
	<skos:definition xml:lang="en">A Thesaurus is a collection of concepts (=terms), which in contrary to other collections of concepts (e.g. glossary, lexicon, dictionary, etc.) includes the correlation to other concepts (superordinate, subordinate, related).  This thereby increases the significance of each concept (semantics).</skos:definition>
</rdf:Description>

<rdf:Description rdf:about="http://resource.geolba.ac.at/doc/26">
	<rdf:type rdf:resource="http://www.w3.org/2004/02/skos/core#Concept"/>
</rdf:Description>

<rdf:Description rdf:about="http://resource.geolba.ac.at/doc/0">
	<skos:hasTopConcept rdf:resource="http://resource.geolba.ac.at/doc/27"/>
</rdf:Description>

<rdf:Description rdf:about="http://resource.geolba.ac.at/doc/61">
	<skos:hasTopConcept rdf:resource="http://resource.geolba.ac.at/doc/62"/>
</rdf:Description>

<rdf:Description rdf:about="http://resource.geolba.ac.at/doc/35">
	<skos:topConceptOf rdf:resource="http://resource.geolba.ac.at/doc/0"/>
</rdf:Description>

<rdf:Description rdf:about="http://resource.geolba.ac.at/doc/29">
	<skos:narrower rdf:resource="http://resource.geolba.ac.at/doc/30"/>
</rdf:Description>

<rdf:Description rdf:about="http://resource.geolba.ac.at/doc/46">
	<skos:definition xml:lang="en">For the same reason geosciences have the same term for various domains. For example “clay” is defined as a mineral, as a lithologic material, or as a mineral resource. With the use of so-called URIs (Unform Resource Identifier, web addresses with unique identifiers) the desired concept can be referenced exactly.</skos:definition>
</rdf:Description>

<rdf:Description rdf:about="http://resource.geolba.ac.at/doc/47">
	<dcterms:created rdf:datatype="http://www.w3.org/2001/XMLSchema#dateTime">2014-09-25T08:53:06.000Z</dcterms:created>
</rdf:Description>

<rdf:Description rdf:about="http://resource.geolba.ac.at/doc/31">
	<skos:definition xml:lang="de">http://de.dbpedia.org/sparql</skos:definition>
</rdf:Description>

<rdf:Description rdf:about="http://resource.geolba.ac.at/doc/40">
	<dcterms:created rdf:datatype="http://www.w3.org/2001/XMLSchema#dateTime">2014-09-25T08:47:23.000Z</dcterms:created>
</rdf:Description>

<rdf:Description rdf:about="http://resource.geolba.ac.at/doc/165">
	<dcterms:creator rdf:resource="http://resource.geolba.ac.at/user/schmar"/>
</rdf:Description>

<rdf:Description rdf:about="http://resource.geolba.ac.at/doc/9">
	<dcterms:creator rdf:resource="http://resource.geolba.ac.at/user/schmar"/>
</rdf:Description>

<rdf:Description rdf:about="http://resource.geolba.ac.at/doc/38">
	<dcterms:creator rdf:resource="http://resource.geolba.ac.at/user/schmar"/>
</rdf:Description>

<rdf:Description rdf:about="http://resource.geolba.ac.at/doc/17">
	<dcterms:hasVersion rdf:datatype="http://www.w3.org/2001/XMLSchema#int">5</dcterms:hasVersion>
</rdf:Description>

<rdf:Description rdf:about="http://resource.geolba.ac.at/doc/1">
	<dcterms:hasVersion rdf:datatype="http://www.w3.org/2001/XMLSchema#int">2</dcterms:hasVersion>
</rdf:Description>

<rdf:Description rdf:about="http://resource.geolba.ac.at/doc/160">
	<skos:prefLabel xml:lang="en">10 concepts, recently modified</skos:prefLabel>
</rdf:Description>

<rdf:Description rdf:about="http://resource.geolba.ac.at/doc/11">
	<skos:prefLabel xml:lang="de">Lithologische Begriffe (Gesteine) mit Links nach DBpedia (Wikipedia)</skos:prefLabel>
</rdf:Description>

<rdf:Description rdf:about="http://resource.geolba.ac.at/doc/38">
	<rdf:type rdf:resource="http://www.w3.org/2004/02/skos/core#Concept"/>
</rdf:Description>

<rdf:Description rdf:about="http://resource.geolba.ac.at/doc/159">
	<dcterms:created rdf:datatype="http://www.w3.org/2001/XMLSchema#dateTime">2018-09-27T06:35:28.000Z</dcterms:created>
</rdf:Description>

<rdf:Description rdf:about="http://resource.geolba.ac.at/doc/62">
	<country-name xmlns="http://www.w3.org/2006/vcard/ns#" xml:lang="de">Österreich</country-name>
</rdf:Description>

<rdf:Description rdf:about="http://resource.geolba.ac.at/doc/15">
	<skos:narrower rdf:resource="http://resource.geolba.ac.at/doc/16"/>
	<dcterms:created rdf:datatype="http://www.w3.org/2001/XMLSchema#dateTime">2014-06-17T15:18:18.000Z</dcterms:created>
</rdf:Description>

<rdf:Description rdf:about="http://resource.geolba.ac.at/doc/36">
	<skos:prefLabel xml:lang="en">Types of commodities (mineral resources) in Austria including abbreviations</skos:prefLabel>
</rdf:Description>

<rdf:Description rdf:about="http://resource.geolba.ac.at/doc/30">
	<dcterms:hasVersion rdf:datatype="http://www.w3.org/2001/XMLSchema#int">1</dcterms:hasVersion>
</rdf:Description>

<rdf:Description rdf:about="http://resource.geolba.ac.at/doc/29">
	<dcterms:hasVersion rdf:datatype="http://www.w3.org/2001/XMLSchema#int">3</dcterms:hasVersion>
</rdf:Description>

<rdf:Description rdf:about="http://resource.geolba.ac.at/doc/44">
	<skos:prefLabel xml:lang="en">How can I search for terms (concepts), which are linked to INSPIRE-Codes?</skos:prefLabel>
</rdf:Description>

<rdf:Description rdf:about="http://resource.geolba.ac.at/doc/20">
	<skos:broader rdf:resource="http://resource.geolba.ac.at/doc/2"/>
</rdf:Description>

<rdf:Description rdf:about="http://resource.geolba.ac.at/doc/2">
	<skos:prefLabel xml:lang="de">GBA_Geologische_Einheiten</skos:prefLabel>
</rdf:Description>

<rdf:Description rdf:about="http://resource.geolba.ac.at/doc/161">
	<dcterms:created rdf:datatype="http://www.w3.org/2001/XMLSchema#dateTime">2018-09-27T11:24:55.000Z</dcterms:created>
</rdf:Description>

<rdf:Description rdf:about="http://resource.geolba.ac.at/doc/1">
	<skos:prefLabel xml:lang="de">GBA_Lithologie</skos:prefLabel>
</rdf:Description>

<rdf:Description rdf:about="http://resource.geolba.ac.at/doc/75">
	<rdf:type rdf:resource="http://www.w3.org/2004/02/skos/core#Concept"/>
</rdf:Description>

<rdf:Description rdf:about="http://resource.geolba.ac.at/doc/48">
	<skos:broader rdf:resource="http://resource.geolba.ac.at/doc/39"/>
</rdf:Description>

<rdf:Description rdf:about="http://resource.geolba.ac.at/doc/79">
	<dcterms:created rdf:datatype="http://www.w3.org/2001/XMLSchema#dateTime">2014-12-18T13:07:06.000Z</dcterms:created>
</rdf:Description>

<rdf:Description rdf:about="http://resource.geolba.ac.at/doc/24">
	<dcterms:created rdf:datatype="http://www.w3.org/2001/XMLSchema#dateTime">2014-06-18T12:23:08.000Z</dcterms:created>
</rdf:Description>

<rdf:Description rdf:about="http://resource.geolba.ac.at/doc/4">
	<dcterms:created rdf:datatype="http://www.w3.org/2001/XMLSchema#dateTime">2014-06-13T09:17:08.000Z</dcterms:created>
</rdf:Description>

<rdf:Description rdf:about="http://resource.geolba.ac.at/doc/167">
	<dcterms:created rdf:datatype="http://www.w3.org/2001/XMLSchema#dateTime">2018-10-02T11:14:57.000Z</dcterms:created>
</rdf:Description>

<rdf:Description rdf:about="http://resource.geolba.ac.at/doc/62">
	<logo xmlns="http://www.w3.org/2006/vcard/ns#" rdf:resource="http://www.geologie.ac.at/fileadmin/template/images/logo.jpg"/>
</rdf:Description>

<rdf:Description rdf:about="http://resource.geolba.ac.at/doc/74">
	<skos:prefLabel xml:lang="de">Geothermal-Projekte auf reegle-data</skos:prefLabel>
</rdf:Description>

<rdf:Description rdf:about="http://resource.geolba.ac.at/doc/26">
	<dcterms:creator rdf:resource="http://resource.geolba.ac.at/user/schmar"/>
</rdf:Description>

<rdf:Description rdf:about="http://resource.geolba.ac.at/doc/37">
	<dcterms:subject xml:lang="de">frequently asked questions</dcterms:subject>
</rdf:Description>

<rdf:Description rdf:about="http://resource.geolba.ac.at/doc/88">
	<skos:broader rdf:resource="http://resource.geolba.ac.at/doc/2"/>
</rdf:Description>

<rdf:Description rdf:about="http://resource.geolba.ac.at/doc/24">
	<skos:prefLabel xml:lang="en">All Tectonic units of type 'Nappe' within Upper Austro-Alpine Nappes</skos:prefLabel>
</rdf:Description>

<rdf:Description rdf:about="http://resource.geolba.ac.at/doc/66">
	<dcterms:created rdf:datatype="http://www.w3.org/2001/XMLSchema#dateTime">2014-10-28T07:42:17.000Z</dcterms:created>
</rdf:Description>

<rdf:Description rdf:about="http://resource.geolba.ac.at/doc/61">
	<dcterms:subject xml:lang="de">Organisation</dcterms:subject>
</rdf:Description>

<rdf:Description rdf:about="http://resource.geolba.ac.at/doc/14">
	<dcterms:creator rdf:resource="http://resource.geolba.ac.at/user/schmar"/>
</rdf:Description>

<rdf:Description rdf:about="http://resource.geolba.ac.at/doc/1">
	<skos:narrower rdf:resource="http://resource.geolba.ac.at/doc/9"/>
</rdf:Description>

<rdf:Description rdf:about="http://resource.geolba.ac.at/doc/42">
	<rdf:type rdf:resource="http://www.w3.org/2004/02/skos/core#Concept"/>
</rdf:Description>

<rdf:Description rdf:about="http://resource.geolba.ac.at/doc/85">
	<skos:broader rdf:resource="http://resource.geolba.ac.at/doc/38"/>
</rdf:Description>

<rdf:Description rdf:about="http://resource.geolba.ac.at/doc/75">
	<dcterms:created rdf:datatype="http://www.w3.org/2001/XMLSchema#dateTime">2014-12-09T13:41:09.000Z</dcterms:created>
</rdf:Description>

<rdf:Description rdf:about="http://resource.geolba.ac.at/doc/26">
	<skos:broader rdf:resource="http://resource.geolba.ac.at/doc/17"/>
</rdf:Description>

<rdf:Description rdf:about="http://resource.geolba.ac.at/doc/42">
	<dcterms:creator rdf:resource="http://resource.geolba.ac.at/user/schmar"/>
</rdf:Description>

<rdf:Description rdf:about="http://resource.geolba.ac.at/doc/44">
	<dcterms:created rdf:datatype="http://www.w3.org/2001/XMLSchema#dateTime">2014-09-25T08:50:23.000Z</dcterms:created>
</rdf:Description>

<rdf:Description rdf:about="http://resource.geolba.ac.at/doc/9">
	<skos:definition xml:lang="de">PREFIX skos:&lt;http://www.w3.org/2004/02/skos/core#&gt;&amp;#xa;SELECT ?URI ?prefLabelDE ?descDE&amp;#xa;WHERE {&amp;#xa;?URI a skos:Concept . ?URI skos:prefLabel ?prefLabelDE . FILTER(lang(?prefLabelDE)='de') .&amp;#xa;OPTIONAL {?URI skos:definition ?descDE . FILTER(lang(?descDE)='de')} .&amp;#xa;&amp;#xa;OPTIONAL {?URI ?p1 ?inspire . FILTER (regex(str(?inspire), '^http://inspire.ec.europa.eu'))} &amp;#xa;OPTIONAL {?URI ?p2 ?gsml . FILTER (regex(str(?gsml), '^http://resource.geosciml.org'))} &amp;#xa;FILTER (!BOUND(?inspire) &amp;&amp; !BOUND(?gsml))&amp;#xa;}&amp;#xa;ORDER BY ?prefLabelDE</skos:definition>
</rdf:Description>

<rdf:Description rdf:about="http://resource.geolba.ac.at/doc/0">
	<dcterms:created rdf:datatype="http://www.w3.org/2001/XMLSchema#dateTime">2014-06-13T09:13:01.000Z</dcterms:created>
</rdf:Description>

<rdf:Description rdf:about="http://resource.geolba.ac.at/doc/17">
	<skos:definition xml:lang="de">http://factforge.net/sparql</skos:definition>
</rdf:Description>

<rdf:Description rdf:about="http://resource.geolba.ac.at/doc/26">
	<skos:prefLabel xml:lang="de">Moore in Österreich (aus Geonames.org)</skos:prefLabel>
</rdf:Description>

<rdf:Description rdf:about="http://resource.geolba.ac.at/doc/30">
	<dcterms:creator rdf:resource="http://resource.geolba.ac.at/user/schmar"/>
</rdf:Description>

<rdf:Description rdf:about="http://resource.geolba.ac.at/doc/10">
	<dcterms:hasVersion rdf:datatype="http://www.w3.org/2001/XMLSchema#int">2</dcterms:hasVersion>
</rdf:Description>

<rdf:Description rdf:about="http://resource.geolba.ac.at/doc/3">
	<dcterms:created rdf:datatype="http://www.w3.org/2001/XMLSchema#dateTime">2014-06-13T09:14:57.000Z</dcterms:created>
</rdf:Description>

<rdf:Description rdf:about="http://resource.geolba.ac.at/doc/156">
	<rdf:type rdf:resource="http://www.w3.org/2004/02/skos/core#Concept"/>
</rdf:Description>

<rdf:Description rdf:about="http://resource.geolba.ac.at/doc/154">
	<dcterms:created rdf:datatype="http://www.w3.org/2001/XMLSchema#dateTime">2016-04-28T07:45:12.000Z</dcterms:created>
</rdf:Description>

<rdf:Description rdf:about="http://resource.geolba.ac.at/doc/29">
	<dcterms:creator rdf:resource="http://resource.geolba.ac.at/user/schmar"/>
</rdf:Description>

<rdf:Description rdf:about="http://resource.geolba.ac.at/doc/30">
	<rdf:type rdf:resource="http://www.w3.org/2004/02/skos/core#Concept"/>
</rdf:Description>

<rdf:Description rdf:about="http://resource.geolba.ac.at/doc/167">
	<skos:prefLabel xml:lang="de">Alle Begriffe in einer Tabelle (erweiterter SQL Export)</skos:prefLabel>
</rdf:Description>

<rdf:Description rdf:about="http://resource.geolba.ac.at/doc/46">
	<dcterms:created rdf:datatype="http://www.w3.org/2001/XMLSchema#dateTime">2014-09-25T08:52:24.000Z</dcterms:created>
</rdf:Description>

<rdf:Description rdf:about="http://resource.geolba.ac.at/doc/23">
	<skos:broader rdf:resource="http://resource.geolba.ac.at/doc/1"/>
</rdf:Description>

<rdf:Description rdf:about="http://resource.geolba.ac.at/doc/62">
	<skos:topConceptOf rdf:resource="http://resource.geolba.ac.at/doc/61"/>
</rdf:Description>

<rdf:Description rdf:about="http://resource.geolba.ac.at/doc/66">
	<dcterms:creator rdf:resource="http://resource.geolba.ac.at/user/schmar"/>
</rdf:Description>

<rdf:Description rdf:about="http://resource.geolba.ac.at/doc/36">
	<dcterms:creator rdf:resource="http://resource.geolba.ac.at/user/schmar"/>
</rdf:Description>

<rdf:Description rdf:about="http://resource.geolba.ac.at/doc/3">
	<dcterms:hasVersion rdf:datatype="http://www.w3.org/2001/XMLSchema#int">2</dcterms:hasVersion>
</rdf:Description>

<rdf:Description rdf:about="http://resource.geolba.ac.at/doc/154">
	<skos:prefLabel xml:lang="en">Is it possible to visualize Thesaurus concepts graphically?</skos:prefLabel>
</rdf:Description>

<rdf:Description rdf:about="http://resource.geolba.ac.at/doc/62">
	<rdf:type rdf:resource="http://www.w3.org/2006/vcard/ns#Organization"/>
</rdf:Description>

<rdf:Description rdf:about="http://resource.geolba.ac.at/doc/36">
	<rdf:type rdf:resource="http://www.w3.org/2004/02/skos/core#Concept"/>
</rdf:Description>

<rdf:Description rdf:about="http://resource.geolba.ac.at/doc/21">
	<skos:prefLabel xml:lang="de">Valide stratigrafische Einheiten Österreichs mit Erläuterungen von 2014</skos:prefLabel>
</rdf:Description>

<rdf:Description rdf:about="http://resource.geolba.ac.at/doc/24">
	<rdf:type rdf:resource="http://www.w3.org/2004/02/skos/core#Concept"/>
</rdf:Description>

<rdf:Description rdf:about="http://resource.geolba.ac.at/doc/159">
	<skos:narrower rdf:resource="http://resource.geolba.ac.at/doc/167"/>
</rdf:Description>

<rdf:Description rdf:about="http://resource.geolba.ac.at/doc/158">
	<dcterms:subject xml:lang="de">Dokumentation</dcterms:subject>
</rdf:Description>

<rdf:Description rdf:about="http://resource.geolba.ac.at/doc/16">
	<skos:prefLabel xml:lang="de">Geologische Begriffe in Österreich, Deutschland und Schweiz in Wikipedia mit Beschreibungen auf Englisch</skos:prefLabel>
</rdf:Description>

<rdf:Description rdf:about="http://resource.geolba.ac.at/doc/27">
	<skos:definition xml:lang="de">http://zbw.eu/beta/sparql/gnd/query</skos:definition>
</rdf:Description>

<rdf:Description rdf:about="http://resource.geolba.ac.at/doc/158">
	<rdf:type rdf:resource="http://www.w3.org/2004/02/skos/core#ConceptScheme"/>
</rdf:Description>

<rdf:Description rdf:about="http://resource.geolba.ac.at/doc/159">
	<skos:narrower rdf:resource="http://resource.geolba.ac.at/doc/166"/>
</rdf:Description>

<rdf:Description rdf:about="http://resource.geolba.ac.at/doc/17">
	<skos:narrower rdf:resource="http://resource.geolba.ac.at/doc/18"/>
</rdf:Description>

<rdf:Description rdf:about="http://resource.geolba.ac.at/doc/163">
	<skos:prefLabel xml:lang="en">Concepts, idenitified by the GBA editorial team, to official use</skos:prefLabel>
</rdf:Description>

<rdf:Description rdf:about="http://resource.geolba.ac.at/doc/160">
	<skos:prefLabel xml:lang="de">10 Begriffe, die zuletzt bearbeitet wurden</skos:prefLabel>
</rdf:Description>

<rdf:Description rdf:about="http://resource.geolba.ac.at/doc/0">
	<dcterms:contributor rdf:resource="http://resource.geolba.ac.at/user/schmar"/>
</rdf:Description>

<rdf:Description rdf:about="http://resource.geolba.ac.at/doc/24">
	<dcterms:creator rdf:resource="http://resource.geolba.ac.at/user/schmar"/>
</rdf:Description>

<rdf:Description rdf:about="http://resource.geolba.ac.at/doc/159">
	<skos:narrower rdf:resource="http://resource.geolba.ac.at/doc/165"/>
</rdf:Description>

<rdf:Description rdf:about="http://resource.geolba.ac.at/doc/80">
	<skos:definition xml:lang="de">PREFIX dcterms:&lt;http://purl.org/dc/terms/&gt;&amp;#xa;PREFIX skos:&lt;http://www.w3.org/2004/02/skos/core#&gt;&amp;#xa;PREFIX ep: &lt;http://resource.geolba.ac.at/PoolParty/schema/gbaex/&gt;&amp;#xa;SELECT ?URI ?Nummer ?Titel ?Kommentar ?Keywords ?Fossilien&amp;#xa;WHERE {&amp;#xa;?URI a ep:Exkursionspunkt ; skos:notation ?Nummer ; &amp;#xa;skos:prefLabel ?Titel ; dcterms:description ?Keywords ;&amp;#xa;skos:definition ?Kommentar ; dcterms:subject &lt;http://resource.geolba.ac.at/gbaex/597&gt; ; &amp;#xa;skos:broader &lt;http://resource.geolba.ac.at/gbaex/582&gt; ;&amp;#xa;ep:Autobus 'true'^^&lt;http://www.w3.org/2001/XMLSchema#boolean&gt; .&amp;#xa;OPTIONAL {?URI dcterms:subject ?Subject . &amp;#xa;?Subject skos:broader &lt;http://resource.geolba.ac.at/gbaex/593&gt; .&amp;#xa;?Subject skos:prefLabel ?Fossilien}&amp;#xa;}</skos:definition>
</rdf:Description>

<rdf:Description rdf:about="http://resource.geolba.ac.at/doc/9">
	<skos:prefLabel xml:lang="en">Rock names neither linked to INSPIRE nor to GeoSciML</skos:prefLabel>
</rdf:Description>

<rdf:Description rdf:about="http://resource.geolba.ac.at/doc/61">
	<dcterms:creator rdf:resource="http://resource.geolba.ac.at/user/schmar"/>
</rdf:Description>

<rdf:Description rdf:about="http://resource.geolba.ac.at/doc/62">
	<extended-address xmlns="http://www.w3.org/2006/vcard/ns#" xml:lang="de">A-1030 Wien, Neulinggasse 38</extended-address>
</rdf:Description>

<rdf:Description rdf:about="http://resource.geolba.ac.at/doc/76">
	<skos:prefLabel xml:lang="de">Bildungsmilieu Geologischer Einheiten</skos:prefLabel>
</rdf:Description>

<rdf:Description rdf:about="http://resource.geolba.ac.at/doc/46">
	<skos:broader rdf:resource="http://resource.geolba.ac.at/doc/38"/>
</rdf:Description>

<rdf:Description rdf:about="http://resource.geolba.ac.at/doc/33">
	<rdf:type rdf:resource="http://www.w3.org/2004/02/skos/core#Concept"/>
</rdf:Description>

<rdf:Description rdf:about="http://resource.geolba.ac.at/doc/5">
	<skos:topConceptOf rdf:resource="http://resource.geolba.ac.at/doc/0"/>
</rdf:Description>

<rdf:Description rdf:about="http://resource.geolba.ac.at/doc/48">
	<rdf:type rdf:resource="http://www.w3.org/2004/02/skos/core#Concept"/>
</rdf:Description>

<rdf:Description rdf:about="http://resource.geolba.ac.at/doc/84">
	<skos:definition xml:lang="en">Some concepts provide color codes for visualization purposes. These codes are conform to INSPIRE and international standards. The notation is hexadecimal coded for web display. A link to color-hex.com guides you to other color models and conversion tools.</skos:definition>
</rdf:Description>

<rdf:Description rdf:about="http://resource.geolba.ac.at/doc/2">
	<skos:narrower rdf:resource="http://resource.geolba.ac.at/doc/19"/>
</rdf:Description>

<rdf:Description rdf:about="http://resource.geolba.ac.at/doc/85">
	<dcterms:creator rdf:resource="http://resource.geolba.ac.at/user/schmar"/>
</rdf:Description>

<rdf:Description rdf:about="http://resource.geolba.ac.at/doc/9">
	<skos:broader rdf:resource="http://resource.geolba.ac.at/doc/1"/>
</rdf:Description>

<rdf:Description rdf:about="http://resource.geolba.ac.at/doc/6">
	<owl:deprecated rdf:datatype="http://www.w3.org/2001/XMLSchema#boolean">true</owl:deprecated>
</rdf:Description>

<rdf:Description rdf:about="http://resource.geolba.ac.at/doc/45">
	<rdf:type rdf:resource="http://www.w3.org/2004/02/skos/core#Concept"/>
</rdf:Description>

<rdf:Description rdf:about="http://resource.geolba.ac.at/doc/166">
	<skos:prefLabel xml:lang="de">Begriffe mit Fotos oder Abbildungen</skos:prefLabel>
</rdf:Description>

<rdf:Description rdf:about="http://resource.geolba.ac.at/doc/72">
	<skos:prefLabel xml:lang="de">Bestandteile zur Geothermie-Nutzung in de, en, fr, es</skos:prefLabel>
</rdf:Description>

<rdf:Description rdf:about="http://resource.geolba.ac.at/doc/33">
	<dcterms:creator rdf:resource="http://resource.geolba.ac.at/user/schmar"/>
</rdf:Description>

<rdf:Description rdf:about="http://resource.geolba.ac.at/doc/29">
	<skos:topConceptOf rdf:resource="http://resource.geolba.ac.at/doc/0"/>
</rdf:Description>

<rdf:Description rdf:about="http://resource.geolba.ac.at/doc/156">
	<dcterms:created rdf:datatype="http://www.w3.org/2001/XMLSchema#dateTime">2016-06-02T11:49:18.000Z</dcterms:created>
</rdf:Description>

<rdf:Description rdf:about="http://resource.geolba.ac.at/doc/36">
	<skos:definition xml:lang="de">PREFIX skos:&lt;http://www.w3.org/2004/02/skos/core#&gt;&amp;#xa;SELECT ?URI ?Code ?Commodity_EN ?Commodity_DE ?Hierarchie ?Hierarchie_URI ?Hierarchie_Bez_DE ?Hierarchie_Bez_EN &amp;#xa;WHERE {&amp;#xa;?URI a skos:Concept . &amp;#xa;?URI skos:prefLabel ?Commodity_DE . FILTER(lang(?Commodity_DE)='de') . &amp;#xa;?URI skos:prefLabel ?Commodity_EN . FILTER(lang(?Commodity_EN)='en').&amp;#xa;?URI skos:notation ?Code .&amp;#xa;?URI skos:broader ?Hierarchie_URI . &amp;#xa;?Hierarchie_URI skos:prefLabel ?Hierarchie_Bez_DE . FILTER(lang(?Hierarchie_Bez_DE)='de') . &amp;#xa;?Hierarchie_URI skos:prefLabel ?Hierarchie_Bez_EN . FILTER(lang(?Hierarchie_Bez_EN)='en') . &amp;#xa;?Hierarchie_URI skos:notation ?Hierarchie&amp;#xa;} &amp;#xa;ORDER BY ?Hierarchie</skos:definition>
</rdf:Description>

<rdf:Description rdf:about="http://resource.geolba.ac.at/doc/38">
	<skos:narrower rdf:resource="http://resource.geolba.ac.at/doc/83"/>
</rdf:Description>

<rdf:Description rdf:about="http://resource.geolba.ac.at/doc/165">
	<rdf:type rdf:resource="http://www.w3.org/2004/02/skos/core#Concept"/>
</rdf:Description>

<rdf:Description rdf:about="http://resource.geolba.ac.at/doc/62">
	<skos:prefLabel xml:lang="de">Geologische Bundesanstalt</skos:prefLabel>
</rdf:Description>

<rdf:Description rdf:about="http://resource.geolba.ac.at/doc/21">
	<dcterms:creator rdf:resource="http://resource.geolba.ac.at/user/schmar"/>
</rdf:Description>

<rdf:Description rdf:about="http://resource.geolba.ac.at/doc/14">
	<skos:definition xml:lang="de">PREFIX property:&lt;http://enipedia.tudelft.nl/wiki/Property:&gt;&amp;#xa;SELECT DISTINCT ?s ?Country&amp;#xa;WHERE {?s property:Primary_fuel_type  ?o . FILTER (regex(str(?o), 'Geothermal')) .&amp;#xa;?s property:Country ?Country } &amp;#xa;ORDER BY ?Country&amp;#xa;</skos:definition>
</rdf:Description>

<rdf:Description rdf:about="http://resource.geolba.ac.at/doc/38">
	<skos:narrower rdf:resource="http://resource.geolba.ac.at/doc/82"/>
</rdf:Description>

<rdf:Description rdf:about="http://resource.geolba.ac.at/doc/65">
	<skos:prefLabel xml:lang="en">How do I search for a 'Lithostratigraphic Unit'?</skos:prefLabel>
</rdf:Description>

<rdf:Description rdf:about="http://resource.geolba.ac.at/doc/8">
	<skos:definition xml:lang="de">PREFIX skos:&lt;http://www.w3.org/2004/02/skos/core#&gt;&amp;#xa;SELECT ?URI ?prefLabelDE ?descDE ?inspire ?gsml&amp;#xa;WHERE {&amp;#xa;?URI a skos:Concept . ?URI skos:prefLabel ?prefLabelDE . FILTER(lang(?prefLabelDE)='de') .&amp;#xa;OPTIONAL {?URI skos:definition ?descDE . FILTER(lang(?descDE)='de')} .&amp;#xa;&amp;#xa;OPTIONAL {?URI ?p1 ?inspire . FILTER (regex(str(?inspire), '^http://inspire.ec.europa.eu'))} &amp;#xa;OPTIONAL {?URI ?p2 ?gsml . FILTER (regex(str(?gsml), '^http://resource.geosciml.org'))} &amp;#xa;FILTER (BOUND(?inspire) || BOUND(?gsml))&amp;#xa;}&amp;#xa;ORDER BY ?prefLabelDE</skos:definition>
</rdf:Description>

<rdf:Description rdf:about="http://resource.geolba.ac.at/doc/62">
	<region xmlns="http://www.w3.org/2006/vcard/ns#" xml:lang="en">Vienna</region>
</rdf:Description>

<rdf:Description rdf:about="http://resource.geolba.ac.at/doc/73">
	<dcterms:creator rdf:resource="http://resource.geolba.ac.at/user/schmar"/>
</rdf:Description>

<rdf:Description rdf:about="http://resource.geolba.ac.at/doc/0">
	<rdf:type rdf:resource="http://www.w3.org/2004/02/skos/core#ConceptScheme"/>
</rdf:Description>

<rdf:Description rdf:about="http://resource.geolba.ac.at/doc/81">
	<skos:definition xml:lang="de">PREFIX skos:&lt;http://www.w3.org/2004/02/skos/core#&gt;&amp;#xa;SELECT ?URI ?prefLabelDE ?definitionDE ?prefLabelEN ?definitionEN &amp;#xa;WHERE {&amp;#xa;?URI a skos:Concept ; skos:prefLabel ?prefLabelDE . &amp;#xa;FILTER(lang(?prefLabelDE)='de') . FILTER (!strStarts(?prefLabelDE, '['^^xsd:string)) .&amp;#xa;OPTIONAL{?URI skos:prefLabel ?prefLabelEN . FILTER(lang(?prefLabelEN)='en')} &amp;#xa;OPTIONAL{?URI skos:definition ?definitionDE . FILTER(lang(?definitionDE)='de')} &amp;#xa;OPTIONAL{?URI skos:definition ?definitionEN . FILTER(lang(?definitionEN)='en')}&amp;#xa;} &amp;#xa;ORDER BY ?prefLabelDE&amp;#xa;</skos:definition>
</rdf:Description>

<rdf:Description rdf:about="http://resource.geolba.ac.at/doc/0">
	<dcterms:subject xml:lang="de">Dokumentation</dcterms:subject>
	<dcterms:creator rdf:resource="http://resource.geolba.ac.at/user/schmar"/>
</rdf:Description>

<rdf:Description rdf:about="http://resource.geolba.ac.at/doc/163">
	<dcterms:creator rdf:resource="http://resource.geolba.ac.at/user/schmar"/>
</rdf:Description>

<rdf:Description rdf:about="http://resource.geolba.ac.at/doc/17">
	<skos:topConceptOf rdf:resource="http://resource.geolba.ac.at/doc/0"/>
</rdf:Description>

<rdf:Description rdf:about="http://resource.geolba.ac.at/doc/10">
	<skos:broader rdf:resource="http://resource.geolba.ac.at/doc/1"/>
</rdf:Description>

<rdf:Description rdf:about="http://resource.geolba.ac.at/doc/46">
	<skos:prefLabel xml:lang="de">Warum findet man ein und denselben Begriff in verschiedenen Themenbereichen?</skos:prefLabel>
</rdf:Description>

<rdf:Description rdf:about="http://resource.geolba.ac.at/doc/80">
	<skos:prefLabel xml:lang="en">Excursion points with fossils in Lower Austria suitable for busses</skos:prefLabel>
</rdf:Description>

<rdf:Description rdf:about="http://resource.geolba.ac.at/doc/1">
	<skos:narrower rdf:resource="http://resource.geolba.ac.at/doc/66"/>
</rdf:Description>

<rdf:Description rdf:about="http://resource.geolba.ac.at/doc/16">
	<dcterms:creator rdf:resource="http://resource.geolba.ac.at/user/schmar"/>
</rdf:Description>

<rdf:Description rdf:about="http://resource.geolba.ac.at/doc/26">
	<skos:definition xml:lang="de">PREFIX gn: &lt;http://www.geonames.org/ontology#&gt;&amp;#xa;SELECT ?s ?Moor ?Bundesland &amp;#xa;WHERE {&amp;#xa;    ?s gn:featureCode &lt;http://www.geonames.org/ontology#H.MOOR&gt; . ?s gn:name ?Moor .&amp;#xa;    ?s gn:countryCode 'AT' . ?s gn:parentADM1 ?admin . ?admin gn:name ?Bundesland &amp;#xa;}</skos:definition>
</rdf:Description>

<rdf:Description rdf:about="http://resource.geolba.ac.at/doc/33">
	<skos:definition xml:lang="de">http://bnb.data.bl.uk/sparql</skos:definition>
</rdf:Description>

<rdf:Description rdf:about="http://resource.geolba.ac.at/doc/49">
	<skos:prefLabel xml:lang="de">Kann ich Informationen aus dem Thesaurus kopieren und verwenden?</skos:prefLabel>
</rdf:Description>

<rdf:Description rdf:about="http://resource.geolba.ac.at/doc/79">
	<skos:narrower rdf:resource="http://resource.geolba.ac.at/doc/80"/>
</rdf:Description>

<rdf:Description rdf:about="http://resource.geolba.ac.at/doc/73">
	<rdf:type rdf:resource="http://www.w3.org/2004/02/skos/core#Concept"/>
</rdf:Description>

<rdf:Description rdf:about="http://resource.geolba.ac.at/doc/22">
	<rdfs:label xml:lang="de">Geologische Einheiten, die vom GBA-Redaktionsteam zur offiziellen Verwendung (official use) gekennzeichnet sind.</rdfs:label>
</rdf:Description>

<rdf:Description rdf:about="http://resource.geolba.ac.at/doc/154">
	<skos:prefLabel xml:lang="de">Kann ich Thesaurusbegriffe visuell darstellen?</skos:prefLabel>
</rdf:Description>

<rdf:Description rdf:about="http://resource.geolba.ac.at/doc/13">
	<skos:topConceptOf rdf:resource="http://resource.geolba.ac.at/doc/0"/>
</rdf:Description>

<rdf:Description rdf:about="http://resource.geolba.ac.at/doc/165">
	<skos:prefLabel xml:lang="en">Concepts with links to INSPIRE or to GeoSciML</skos:prefLabel>
</rdf:Description>

<rdf:Description rdf:about="http://resource.geolba.ac.at/doc/16">
	<rdf:type rdf:resource="http://www.w3.org/2004/02/skos/core#Concept"/>
</rdf:Description>

<rdf:Description rdf:about="http://resource.geolba.ac.at/doc/15">
	<dcterms:hasVersion rdf:datatype="http://www.w3.org/2001/XMLSchema#int">5</dcterms:hasVersion>
</rdf:Description>

<rdf:Description rdf:about="http://resource.geolba.ac.at/doc/157">
	<skos:definition xml:lang="de">PREFIX skos:&lt;http://www.w3.org/2004/02/skos/core#&gt;&amp;#xa;PREFIX gba:&lt;http://resource.geolba.ac.at/PoolParty/schema/GBA/&gt;&amp;#xa;SELECT ?URI ?prefLabelDE&amp;#xa;WHERE&amp;#xa;{&amp;#xa;?URI a skos:Concept . ?URI skos:prefLabel ?prefLabelDE . FILTER(lang(?prefLabelDE)='de') .&amp;#xa;?URI gba:GBA_Status ?status . FILTER regex(str(?status), '3')&amp;#xa;}&amp;#xa;ORDER BY ?prefLabelDE</skos:definition>
</rdf:Description>

<rdf:Description rdf:about="http://resource.geolba.ac.at/doc/163">
	<skos:broader rdf:resource="http://resource.geolba.ac.at/doc/159"/>
</rdf:Description>

<rdf:Description rdf:about="http://resource.geolba.ac.at/doc/66">
	<skos:broader rdf:resource="http://resource.geolba.ac.at/doc/1"/>
</rdf:Description>

<rdf:Description rdf:about="http://resource.geolba.ac.at/doc/38">
	<skos:narrower rdf:resource="http://resource.geolba.ac.at/doc/46"/>
</rdf:Description>

<rdf:Description rdf:about="http://resource.geolba.ac.at/doc/83">
	<dcterms:created rdf:datatype="http://www.w3.org/2001/XMLSchema#dateTime">2015-03-23T09:18:47.000Z</dcterms:created>
</rdf:Description>

<rdf:Description rdf:about="http://resource.geolba.ac.at/doc/50">
	<skos:prefLabel xml:lang="de">An wen kann ich mich im Falle von Fragen, oder Kommentaren zum Thesaurus wenden?</skos:prefLabel>
</rdf:Description>

<rdf:Description rdf:about="http://resource.geolba.ac.at/doc/41">
	<rdf:type rdf:resource="http://www.w3.org/2004/02/skos/core#Concept"/>
</rdf:Description>

<rdf:Description rdf:about="http://resource.geolba.ac.at/doc/19">
	<skos:prefLabel xml:lang="de">Stratigrafische Einheiten mit Referenzpunkt und Koordinatenangabe</skos:prefLabel>
</rdf:Description>

<rdf:Description rdf:about="http://resource.geolba.ac.at/doc/25">
	<skos:topConceptOf rdf:resource="http://resource.geolba.ac.at/doc/0"/>
</rdf:Description>

<rdf:Description rdf:about="http://resource.geolba.ac.at/doc/41">
	<skos:definition xml:lang="en">In SKOS (Simple Knowledge Organization System) the meaning of a concept can be defined by the definition and the linkage to other concepts. A further modelling of the concepts into defined classes, properties and attributes (i.e. creating objects for data models) would be possible in e.g. OWL (Web Ontology Language, formal logic based representation). But for the geological survey of Austria it would cost too much effort and budget. Therefore the geological survey intends to construct a high-quality SKOS-vocabulary for geoscientific terms (like these terms should/ and have been used in publications). The ‘organizational knowledge’ of our institution is documented by an editorial team which also ensures the quality of each description.</skos:definition>
</rdf:Description>

<rdf:Description rdf:about="http://resource.geolba.ac.at/doc/38">
	<skos:narrower rdf:resource="http://resource.geolba.ac.at/doc/45"/>
</rdf:Description>

<rdf:Description rdf:about="http://resource.geolba.ac.at/doc/81">
	<dcterms:creator rdf:resource="http://resource.geolba.ac.at/user/schmar"/>
</rdf:Description>

<rdf:Description rdf:about="http://resource.geolba.ac.at/doc/83">
	<skos:broader rdf:resource="http://resource.geolba.ac.at/doc/38"/>
</rdf:Description>

<rdf:Description rdf:about="http://resource.geolba.ac.at/doc/48">
	<dcterms:creator rdf:resource="http://resource.geolba.ac.at/user/schmar"/>
</rdf:Description>

<rdf:Description rdf:about="http://resource.geolba.ac.at/doc/6">
	<rdfs:label xml:lang="de">Alle Geologischen Einheiten mit Beschreibung in Deutsch und Englisch</rdfs:label>
</rdf:Description>

<rdf:Description rdf:about="http://resource.geolba.ac.at/doc/62">
	<email xmlns="http://www.w3.org/2006/vcard/ns#" rdf:resource="mailto:office@geologie.ac.at"/>
</rdf:Description>

<rdf:Description rdf:about="http://resource.geolba.ac.at/doc/156">
	<skos:definition xml:lang="de">PREFIX skos:&lt;http://www.w3.org/2004/02/skos/core#&gt;&amp;#xa;PREFIX gba:&lt;http://resource.geolba.ac.at/PoolParty/schema/GBA/&gt;&amp;#xa;SELECT DISTINCT ?URI (STR(?Lde) AS ?Label_de) (STR(?Len) AS ?Label_en) (STR(?Dde) AS ?Def_de) (STR(?Den) AS ?Def_en)&amp;#xa; (STR(?Notede) AS ?Note_de) (STR(?Noteen) AS ?Note_en) (STR(?topLde) AS ?topLabel_de) ?GBA_Status&amp;#xa;WHERE{VALUES ?CS {&lt;http://resource.geolba.ac.at/GeologicUnit/235&gt; &lt;http://resource.geolba.ac.at/GeologicUnit/1&gt;} &amp;#xa;?CS skos:hasTopConcept ?topURI . ?topURI skos:narrower* ?URI; skos:prefLabel ?topLde .&amp;#xa;FILTER(lang(?topLde)='de') . &amp;#xa;?URI skos:prefLabel ?Lde; skos:prefLabel ?Len; skos:definition ?Dde; skos:definition ?Den .&amp;#xa;OPTIONAL {?URI skos:scopeNote ?Notede ; skos:scopeNote ?Noteen . FILTER(lang(?Notede)='de') . FILTER(lang(?Noteen)='en')}&amp;#xa;OPTIONAL {?URI gba:GBA_Status ?GBA_Status}&amp;#xa;FILTER(lang(?Lde)='de') . FILTER(lang(?Len)='en') . FILTER(lang(?Dde)='de') . FILTER(lang(?Den)='en') }</skos:definition>
</rdf:Description>

<rdf:Description rdf:about="http://resource.geolba.ac.at/doc/27">
	<skos:scopeNote xml:lang="de">PREFIX gndo:&lt;http://d-nb.info/standards/elementset/gnd#&gt;&amp;#xa;select ?URI ?Name ?Publikation&amp;#xa;where {&amp;#xa;?URI gndo:preferredNameForThePerson ?Name . &amp;#xa;?URI gndo:publication ?Publikation . FILTER(regex(str(?Publikation),'Dachstein')) . &amp;#xa;}&amp;#xa;LIMIT 10</skos:scopeNote>
</rdf:Description>

<rdf:Description rdf:about="http://resource.geolba.ac.at/doc/43">
	<skos:prefLabel xml:lang="de">Kann ich individuell zusammengestellte Informationen aus dem Thesaurus als Listen downloaden oder exportieren?</skos:prefLabel>
</rdf:Description>

<rdf:Description rdf:about="http://resource.geolba.ac.at/doc/62">
	<foaf:name xml:lang="de">Geologische Bundesanstalt</foaf:name>
</rdf:Description>

<rdf:Description rdf:about="http://resource.geolba.ac.at/doc/85">
	<rdf:type rdf:resource="http://www.w3.org/2004/02/skos/core#Concept"/>
</rdf:Description>

<rdf:Description rdf:about="http://resource.geolba.ac.at/doc/7">
	<dcterms:creator rdf:resource="http://resource.geolba.ac.at/user/schmar"/>
</rdf:Description>

<rdf:Description rdf:about="http://resource.geolba.ac.at/doc/88">
	<dcterms:creator rdf:resource="http://resource.geolba.ac.at/user/schmar"/>
</rdf:Description>

<rdf:Description rdf:about="http://resource.geolba.ac.at/doc/7">
	<rdf:type rdf:resource="http://www.w3.org/2004/02/skos/core#Concept"/>
</rdf:Description>

<rdf:Description rdf:about="http://resource.geolba.ac.at/doc/88">
	<rdf:type rdf:resource="http://www.w3.org/2004/02/skos/core#Concept"/>
</rdf:Description>

<rdf:Description rdf:about="http://resource.geolba.ac.at/doc/42">
	<skos:broader rdf:resource="http://resource.geolba.ac.at/doc/40"/>
</rdf:Description>

<rdf:Description rdf:about="http://resource.geolba.ac.at/doc/0">
	<skos:hasTopConcept rdf:resource="http://resource.geolba.ac.at/doc/5"/>
</rdf:Description>

<rdf:Description rdf:about="http://resource.geolba.ac.at/doc/76">
	<rdf:type rdf:resource="http://www.w3.org/2004/02/skos/core#Concept"/>
</rdf:Description>

<rdf:Description rdf:about="http://resource.geolba.ac.at/doc/167">
	<skos:broader rdf:resource="http://resource.geolba.ac.at/doc/159"/>
</rdf:Description>

<rdf:Description rdf:about="http://resource.geolba.ac.at/doc/21">
	<skos:prefLabel xml:lang="en">Valid stratigraphic units of Austria with descriptions from 2014</skos:prefLabel>
</rdf:Description>

<rdf:Description rdf:about="http://resource.geolba.ac.at/doc/29">
	<skos:definition xml:lang="de">http://semantic.eea.europa.eu/sparql</skos:definition>
</rdf:Description>

<rdf:Description rdf:about="http://resource.geolba.ac.at/doc/33">
	<skos:topConceptOf rdf:resource="http://resource.geolba.ac.at/doc/0"/>
</rdf:Description>

<rdf:Description rdf:about="http://resource.geolba.ac.at/doc/41">
	<skos:definition xml:lang="de">In SKOS (Simple Knowledge Organization System) können Begriffe durch Begriffsdefinitionen und einer Vernetzung untereinander in ihrer Bedeutung festgelegt werden. Eine weitergehende Modellierung der Begriffswelt in definierte Klassen und Eigenschaften (Objektbildung i.S. eines Datenmodells) wäre z.B. auch in OWL (OntologyWebLanguage, formale logikbasierte Darstellung) möglich, ist für die GBA aber zu aufwendig und zu teuer. Die GBA versucht deshalb ein qualitativ hochwertiges SKOS-Vokabular geowissenschaftlicher Begriffe (wie sie in eigenen Publikationen verwendet wurden bzw. werden sollen) aufzubauen. Das Wissen der GBA wird dabei von einem eigenen Redaktionsteam dokumentiert, und die Qualität der Beschreibungen gesichert.</skos:definition>
</rdf:Description>

<rdf:Description rdf:about="http://resource.geolba.ac.at/doc/20">
	<skos:definition xml:lang="de">PREFIX dcterms:&lt;http://purl.org/dc/terms/&gt;&amp;#xa;PREFIX skos:&lt;http://www.w3.org/2004/02/skos/core#&gt;&amp;#xa;SELECT ?URI ?prefLabelDE ?date&amp;#xa;WHERE&amp;#xa;{&amp;#xa;?URI a skos:Concept . ?URI skos:prefLabel ?prefLabelDE . FILTER(lang(?prefLabelDE)='de') .&amp;#xa;?URI dcterms:modified ?date&amp;#xa;}&amp;#xa;ORDER BY DESC (?date)&amp;#xa;LIMIT 10</skos:definition>
</rdf:Description>

<rdf:Description rdf:about="http://resource.geolba.ac.at/doc/22">
	<owl:deprecated rdf:datatype="http://www.w3.org/2001/XMLSchema#boolean">true</owl:deprecated>
</rdf:Description>

<rdf:Description rdf:about="http://resource.geolba.ac.at/doc/30">
	<skos:definition xml:lang="de">PREFIX a: &lt;http://www.eea.europa.eu/portal_types/Data#&gt;&amp;#xa;PREFIX dcterms: &lt;http://purl.org/dc/terms/&gt;&amp;#xa;&amp;#xa;SELECT DISTINCT ?subj ?issued ?title ?description WHERE {&amp;#xa;?subj a a:Data ;&amp;#xa;dcterms:title ?title ;&amp;#xa;dcterms:description ?description;&amp;#xa;dcterms:issued ?issued. FILTER(regex(str(?title),'Groundwater')).&amp;#xa;} ORDER BY ?effective</skos:definition>
</rdf:Description>

<rdf:Description rdf:about="http://resource.geolba.ac.at/doc/19">
	<rdf:type rdf:resource="http://www.w3.org/2004/02/skos/core#Concept"/>
</rdf:Description>

<rdf:Description rdf:about="http://resource.geolba.ac.at/doc/14">
	<skos:prefLabel xml:lang="de">Geothermal-Kraftwerke weltweit</skos:prefLabel>
</rdf:Description>

<rdf:Description rdf:about="http://resource.geolba.ac.at/doc/167">
	<dcterms:creator rdf:resource="http://resource.geolba.ac.at/user/schmar"/>
</rdf:Description>

<rdf:Description rdf:about="http://resource.geolba.ac.at/doc/19">
	<dcterms:hasVersion rdf:datatype="http://www.w3.org/2001/XMLSchema#int">1</dcterms:hasVersion>
</rdf:Description>

<rdf:Description rdf:about="http://resource.geolba.ac.at/doc/34">
	<owl:deprecated rdf:datatype="http://www.w3.org/2001/XMLSchema#boolean">true</owl:deprecated>
</rdf:Description>

<rdf:Description rdf:about="http://resource.geolba.ac.at/doc/0">
	<skos:hasTopConcept rdf:resource="http://resource.geolba.ac.at/doc/2"/>
</rdf:Description>

<rdf:Description rdf:about="http://resource.geolba.ac.at/doc/7">
	<dcterms:hasVersion rdf:datatype="http://www.w3.org/2001/XMLSchema#int">3</dcterms:hasVersion>
</rdf:Description>

<rdf:Description rdf:about="http://resource.geolba.ac.at/doc/62">
	<rdf:type rdf:resource="http://www.w3.org/2006/vcard/ns#Kind"/>
</rdf:Description>

<rdf:Description rdf:about="http://resource.geolba.ac.at/doc/154">
	<rdf:type rdf:resource="http://www.w3.org/2004/02/skos/core#Concept"/>
</rdf:Description>

<rdf:Description rdf:about="http://resource.geolba.ac.at/doc/32">
	<rdf:type rdf:resource="http://www.w3.org/2004/02/skos/core#Concept"/>
</rdf:Description>

<rdf:Description rdf:about="http://resource.geolba.ac.at/doc/0">
	<skos:hasTopConcept rdf:resource="http://resource.geolba.ac.at/doc/1"/>
</rdf:Description>

<rdf:Description rdf:about="http://resource.geolba.ac.at/doc/1">
	<skos:narrower rdf:resource="http://resource.geolba.ac.at/doc/10"/>
</rdf:Description>

<rdf:Description rdf:about="http://resource.geolba.ac.at/doc/20">
	<rdf:type rdf:resource="http://www.w3.org/2004/02/skos/core#Concept"/>
</rdf:Description>

<rdf:Description rdf:about="http://resource.geolba.ac.at/doc/3">
	<skos:definition xml:lang="de">http://resource.geolba.ac.at/PoolParty/sparql/tectonicunit</skos:definition>
</rdf:Description>

<rdf:Description rdf:about="http://resource.geolba.ac.at/doc/73">
	<skos:narrower rdf:resource="http://resource.geolba.ac.at/doc/74"/>
</rdf:Description>

<rdf:Description rdf:about="http://resource.geolba.ac.at/doc/0">
	<skos:hasTopConcept rdf:resource="http://resource.geolba.ac.at/doc/4"/>
</rdf:Description>

<rdf:Description rdf:about="http://resource.geolba.ac.at/doc/1">
	<skos:narrower rdf:resource="http://resource.geolba.ac.at/doc/11"/>
</rdf:Description>

<rdf:Description rdf:about="http://resource.geolba.ac.at/doc/62">
	<country-name xmlns="http://www.w3.org/2006/vcard/ns#" xml:lang="en">Austria</country-name>
</rdf:Description>

<rdf:Description rdf:about="http://resource.geolba.ac.at/doc/27">
	<skos:prefLabel xml:lang="de">dt. Zentralbibliothek ZBW</skos:prefLabel>
	<skos:prefLabel xml:lang="en">dt. Zentralbibliothek ZBW</skos:prefLabel>
</rdf:Description>

<rdf:Description rdf:about="http://resource.geolba.ac.at/doc/158">
	<skos:hasTopConcept rdf:resource="http://resource.geolba.ac.at/doc/159"/>
</rdf:Description>

<rdf:Description rdf:about="http://resource.geolba.ac.at/doc/32">
	<dcterms:hasVersion rdf:datatype="http://www.w3.org/2001/XMLSchema#int">1</dcterms:hasVersion>
</rdf:Description>

<rdf:Description rdf:about="http://resource.geolba.ac.at/doc/20">
	<dcterms:hasVersion rdf:datatype="http://www.w3.org/2001/XMLSchema#int">1</dcterms:hasVersion>
</rdf:Description>

<rdf:Description rdf:about="http://resource.geolba.ac.at/doc/73">
	<skos:definition xml:lang="de">http://sparql.reegle.info</skos:definition>
</rdf:Description>

<rdf:Description rdf:about="http://resource.geolba.ac.at/doc/40">
	<dcterms:creator rdf:resource="http://resource.geolba.ac.at/user/schmar"/>
</rdf:Description>

<rdf:Description rdf:about="http://resource.geolba.ac.at/doc/62">
	<postal-code xmlns="http://www.w3.org/2006/vcard/ns#">1030</postal-code>
</rdf:Description>

<rdf:Description rdf:about="http://resource.geolba.ac.at/doc/0">
	<skos:hasTopConcept rdf:resource="http://resource.geolba.ac.at/doc/3"/>
</rdf:Description>

<rdf:Description rdf:about="http://resource.geolba.ac.at/doc/166">
	<rdf:type rdf:resource="http://www.w3.org/2004/02/skos/core#Concept"/>
</rdf:Description>

<rdf:Description rdf:about="http://resource.geolba.ac.at/doc/25">
	<skos:definition xml:lang="de">http://eurostat.linked-statistics.org/sparql</skos:definition>
</rdf:Description>

<rdf:Description rdf:about="http://resource.geolba.ac.at/doc/165">
	<skos:prefLabel xml:lang="de">Begriffe mit Links nach INSPIRE oder GeoSciML</skos:prefLabel>
</rdf:Description>

<rdf:Description rdf:about="http://resource.geolba.ac.at/doc/39">
	<dcterms:creator rdf:resource="http://resource.geolba.ac.at/user/schmar"/>
</rdf:Description>

<rdf:Description rdf:about="http://resource.geolba.ac.at/doc/73">
	<skos:prefLabel xml:lang="de">reegle-data</skos:prefLabel>
</rdf:Description>

<rdf:Description rdf:about="http://resource.geolba.ac.at/doc/61">
	<dcterms:title xml:lang="de">Organisation</dcterms:title>
</rdf:Description>

<rdf:Description rdf:about="http://resource.geolba.ac.at/doc/2">
	<skos:definition xml:lang="de">http://resource.geolba.ac.at/PoolParty/sparql/GeologicUnit</skos:definition>
	<skos:narrower rdf:resource="http://resource.geolba.ac.at/doc/156"/>
</rdf:Description>

<rdf:Description rdf:about="http://resource.geolba.ac.at/doc/159">
	<skos:narrower rdf:resource="http://resource.geolba.ac.at/doc/160"/>
</rdf:Description>

<rdf:Description rdf:about="http://resource.geolba.ac.at/doc/24">
	<dcterms:hasVersion rdf:datatype="http://www.w3.org/2001/XMLSchema#int">1</dcterms:hasVersion>
</rdf:Description>

<rdf:Description rdf:about="http://resource.geolba.ac.at/doc/80">
	<skos:prefLabel xml:lang="de">Autobustaugliche Exkursionspunkte zum Thema Fossilien in Niederösterreich</skos:prefLabel>
</rdf:Description>

<rdf:Description rdf:about="http://resource.geolba.ac.at/doc/48">
	<skos:prefLabel xml:lang="de">Wie funktioniert die Hierarchie im Thesaurus?</skos:prefLabel>
</rdf:Description>

<rdf:Description rdf:about="http://resource.geolba.ac.at/doc/87">
	<rdfs:label xml:lang="de">official use</rdfs:label>
</rdf:Description>

<rdf:Description rdf:about="http://resource.geolba.ac.at/doc/41">
	<skos:prefLabel xml:lang="en">Why is the Thesaurus formatted as a SKOS-vocabulary?</skos:prefLabel>
</rdf:Description>

<rdf:Description rdf:about="http://resource.geolba.ac.at/doc/5">
	<skos:prefLabel xml:lang="en">GBA_Structure</skos:prefLabel>
</rdf:Description>

<rdf:Description rdf:about="http://resource.geolba.ac.at/doc/44">
	<rdf:type rdf:resource="http://www.w3.org/2004/02/skos/core#Concept"/>
</rdf:Description>

<rdf:Description rdf:about="http://resource.geolba.ac.at/doc/159">
	<dcterms:creator rdf:resource="http://resource.geolba.ac.at/user/schmar"/>
</rdf:Description>

<rdf:Description rdf:about="http://resource.geolba.ac.at/doc/44">
	<dcterms:creator rdf:resource="http://resource.geolba.ac.at/user/schmar"/>
</rdf:Description>

<rdf:Description rdf:about="http://resource.geolba.ac.at/doc/88">
	<skos:prefLabel xml:lang="de">Geologische Einheiten, die vom GBA-Redaktionsteam zur offiziellen Verwendung (official use) gekennzeichnet sind.</skos:prefLabel>
</rdf:Description>

<rdf:Description rdf:about="http://resource.geolba.ac.at/doc/38">
	<skos:narrower rdf:resource="http://resource.geolba.ac.at/doc/154"/>
</rdf:Description>

<rdf:Description rdf:about="http://resource.geolba.ac.at/doc/81">
	<rdf:type rdf:resource="http://www.w3.org/2004/02/skos/core#Concept"/>
</rdf:Description>

<rdf:Description rdf:about="http://resource.geolba.ac.at/doc/20">
	<skos:prefLabel xml:lang="en">10 concepts of geologic units, recently modified</skos:prefLabel>
</rdf:Description>

<rdf:Description rdf:about="http://resource.geolba.ac.at/doc/158">
	<dcterms:description xml:lang="de">Bookmarks</dcterms:description>
</rdf:Description>

<rdf:Description rdf:about="http://resource.geolba.ac.at/doc/45">
	<skos:definition xml:lang="de">&lt;img alt='' src='http://resource.geolba.ac.at/PoolParty/OpenConfigPathResourceProvider/frontendroot?fileName=custom/images/searchbutton.png'&gt;&lt;/img&gt; Auf der Thesaurus-Startseite $1http://resource.geolba.ac.at/$2http://resource.geolba.ac.at/$3 können im oberen grauen Suchfeld auch Wortteile (oder auch nichts!) eingegeben werden. Die Suche über den orangenen Suchbutton liefert dann alle Begriffe (auch Alternativbegriffe) über alle Themenbereiche in denen der gesuchte Wortteil vorkommt. Die Suche kann anschließend auf alle Bescheibungstexte als sogenannte Volltextsuche erweitert werden. Befindet man sich schon innerhalb eines gewissen Themenbereichs, bekommt man konkrete Begriffe (ab 3 Buchstaben) zur Suche vorgeschlagen.</skos:definition>
</rdf:Description>

<rdf:Description rdf:about="http://resource.geolba.ac.at/doc/77">
	<skos:topConceptOf rdf:resource="http://resource.geolba.ac.at/doc/0"/>
</rdf:Description>

<rdf:Description rdf:about="http://resource.geolba.ac.at/doc/32">
	<dcterms:creator rdf:resource="http://resource.geolba.ac.at/user/schmar"/>
</rdf:Description>

<rdf:Description rdf:about="http://resource.geolba.ac.at/doc/159">
	<skos:narrower rdf:resource="http://resource.geolba.ac.at/doc/164"/>
</rdf:Description>

<rdf:Description rdf:about="http://resource.geolba.ac.at/doc/12">
	<rdfs:label xml:lang="de">x</rdfs:label>
</rdf:Description>

<rdf:Description rdf:about="http://resource.geolba.ac.at/doc/3">
	<dcterms:creator rdf:resource="http://resource.geolba.ac.at/user/schmar"/>
</rdf:Description>

<rdf:Description rdf:about="http://resource.geolba.ac.at/doc/2">
	<skos:topConceptOf rdf:resource="http://resource.geolba.ac.at/doc/0"/>
</rdf:Description>

<rdf:Description rdf:about="http://resource.geolba.ac.at/doc/36">
	<skos:prefLabel xml:lang="de">Rohstoffarten Österreichs mit Kurzbezeichnung</skos:prefLabel>
</rdf:Description>

<rdf:Description rdf:about="http://resource.geolba.ac.at/doc/7">
	<skos:definition xml:lang="de">PREFIX rdfs: &lt;http://www.w3.org/2000/01/rdf-schema#&gt;&amp;#xa;PREFIX skos: &lt;http://www.w3.org/2004/02/skos/core#&gt;&amp;#xa;SELECT ?topConcept ?prefLabel ?conceptScheme ?Label &amp;#xa;WHERE&amp;#xa; {&amp;#xa;?conceptScheme a skos:ConceptScheme . &amp;#xa;?conceptScheme rdfs:label ?Label . &amp;#xa;?conceptScheme skos:hasTopConcept ?topConcept . &amp;#xa;?topConcept skos:prefLabel ?prefLabel. FILTER( lang(?prefLabel) = 'de' )&amp;#xa;}</skos:definition>
</rdf:Description>

<rdf:Description rdf:about="http://resource.geolba.ac.at/doc/72">
	<skos:broader rdf:resource="http://resource.geolba.ac.at/doc/71"/>
</rdf:Description>

<rdf:Description rdf:about="http://resource.geolba.ac.at/doc/159">
	<skos:narrower rdf:resource="http://resource.geolba.ac.at/doc/163"/>
</rdf:Description>

<rdf:Description rdf:about="http://resource.geolba.ac.at/doc/20">
	<skos:prefLabel xml:lang="de">10 Begriffe geologischer Einheiten die zuletzt bearbeitet wurden</skos:prefLabel>
</rdf:Description>

<rdf:Description rdf:about="http://resource.geolba.ac.at/doc/19">
	<dcterms:creator rdf:resource="http://resource.geolba.ac.at/user/schmar"/>
</rdf:Description>

<rdf:Description rdf:about="http://resource.geolba.ac.at/doc/159">
	<skos:narrower rdf:resource="http://resource.geolba.ac.at/doc/162"/>
</rdf:Description>

<rdf:Description rdf:about="http://resource.geolba.ac.at/doc/160">
	<dcterms:creator rdf:resource="http://resource.geolba.ac.at/user/schmar"/>
</rdf:Description>

<rdf:Description rdf:about="http://resource.geolba.ac.at/doc/159">
	<skos:narrower rdf:resource="http://resource.geolba.ac.at/doc/161"/>
</rdf:Description>

<rdf:Description rdf:about="http://resource.geolba.ac.at/doc/76">
	<dcterms:creator rdf:resource="http://resource.geolba.ac.at/user/schmar"/>
</rdf:Description>

<rdf:Description rdf:about="http://resource.geolba.ac.at/doc/80">
	<skos:broader rdf:resource="http://resource.geolba.ac.at/doc/79"/>
</rdf:Description>

<rdf:Description rdf:about="http://resource.geolba.ac.at/doc/20">
	<dcterms:creator rdf:resource="http://resource.geolba.ac.at/user/schmar"/>
</rdf:Description>

<rdf:Description rdf:about="http://resource.geolba.ac.at/doc/82">
	<skos:definition xml:lang="de">Eckige Klammern kennzeichnen provisorische Begriffe, die als Platzhalter zur hierarchischen Gliederung des GBA Thesaurus notwendig sind. Speziell bei der Einarbeitung der 'Stratigraphischen Tabelle von Österreich' (Piller et al. 2004) wurden informelle Gliederungsbegriffe (z.B. Toponyme) in Klammer gesetzt. Eine weitere Verwendung z.B. zur Attributierung von Geodaten, ist daher ebenfalls nur als Provisorium sinnvoll.</skos:definition>
</rdf:Description>

<rdf:Description rdf:about="http://resource.geolba.ac.at/doc/73">
	<skos:topConceptOf rdf:resource="http://resource.geolba.ac.at/doc/0"/>
</rdf:Description>

<rdf:Description rdf:about="http://resource.geolba.ac.at/doc/163">
	<skos:prefLabel xml:lang="de">Begriffe, die vom GBA-Redaktionsteam zur offiziellen Verwendung (official use) gekennzeichnet sind</skos:prefLabel>
</rdf:Description>

<rdf:Description rdf:about="http://resource.geolba.ac.at/doc/162">
	<dcterms:creator rdf:resource="http://resource.geolba.ac.at/user/schmar"/>
</rdf:Description>

<rdf:Description rdf:about="http://resource.geolba.ac.at/doc/49">
	<skos:prefLabel xml:lang="en">Is it legal to use or copy information from the thesaurus?</skos:prefLabel>
</rdf:Description>

<rdf:Description rdf:about="http://resource.geolba.ac.at/doc/1">
	<rdf:type rdf:resource="http://www.w3.org/2004/02/skos/core#Concept"/>
</rdf:Description>

<rdf:Description rdf:about="http://resource.geolba.ac.at/doc/47">
	<dcterms:creator rdf:resource="http://resource.geolba.ac.at/user/schmar"/>
</rdf:Description>

<rdf:Description rdf:about="http://resource.geolba.ac.at/doc/0">
	<skos:hasTopConcept rdf:resource="http://resource.geolba.ac.at/doc/33"/>
</rdf:Description>

<rdf:Description rdf:about="http://resource.geolba.ac.at/doc/32">
	<skos:definition xml:lang="de">PREFIX rdfs:&lt;http://www.w3.org/2000/01/rdf-schema#&gt;&amp;#xa;PREFIX dcterms:&lt;http://purl.org/dc/terms/&gt;&amp;#xa;PREFIX dbpo:&lt;http://dbpedia.org/ontology/&gt;&amp;#xa;SELECT ?Wikipedia ?Name ?Beschreibung&amp;#xa;WHERE {&amp;#xa;?URI dcterms:subject &lt;http://de.dbpedia.org/resource/Kategorie:Gesteinseinheit_der_Trias&gt; . &amp;#xa;?URI rdfs:label ?Name . ?URI dbpo:abstract ?Beschreibung .&amp;#xa;?URI &lt;http://xmlns.com/foaf/0.1/isPrimaryTopicOf&gt; ?Wikipedia&amp;#xa;}</skos:definition>
</rdf:Description>

<rdf:Description rdf:about="http://resource.geolba.ac.at/doc/1">
	<dcterms:creator rdf:resource="http://resource.geolba.ac.at/user/schmar"/>
</rdf:Description>

<rdf:Description rdf:about="http://resource.geolba.ac.at/doc/45">
	<skos:definition xml:lang="en">&lt;img alt='' src='http://resource.geolba.ac.at/PoolParty/OpenConfigPathResourceProvider/frontendroot?fileName=custom/images/searchbutton.png'&gt;&lt;/img&gt; On the start page of the Thesaurus $1http://resource.geolba.ac.at/$2http://resource.geolba.ac.at/$3 in the grey search box above just word parts can be entered (or even left blank!). The search triggered by pressing the orange search button, will then provide all concepts from all domains which include the word part (including alternative terms). The search can further been extended to a full text search. If you are navigating already within a certain domain, the search will suggest auto complete terms (minimum 3 letters).</skos:definition>
</rdf:Description>

<rdf:Description rdf:about="http://resource.geolba.ac.at/doc/4">
	<skos:topConceptOf rdf:resource="http://resource.geolba.ac.at/doc/0"/>
</rdf:Description>

<rdf:Description rdf:about="http://resource.geolba.ac.at/doc/47">
	<rdf:type rdf:resource="http://www.w3.org/2004/02/skos/core#Concept"/>
</rdf:Description>

<rdf:Description rdf:about="http://resource.geolba.ac.at/doc/35">
	<dcterms:creator rdf:resource="http://resource.geolba.ac.at/user/schmar"/>
</rdf:Description>

<rdf:Description rdf:about="http://resource.geolba.ac.at/doc/4">
	<dcterms:hasVersion rdf:datatype="http://www.w3.org/2001/XMLSchema#int">2</dcterms:hasVersion>
</rdf:Description>

<rdf:Description rdf:about="http://resource.geolba.ac.at/doc/2">
	<skos:narrower rdf:resource="http://resource.geolba.ac.at/doc/81"/>
</rdf:Description>

<rdf:Description rdf:about="http://resource.geolba.ac.at/doc/162">
	<skos:prefLabel xml:lang="de">Alle Begriffe mit Beschreibung in Deutsch und Englisch</skos:prefLabel>
</rdf:Description>

<rdf:Description rdf:about="http://resource.geolba.ac.at/doc/72">
	<dcterms:creator rdf:resource="http://resource.geolba.ac.at/user/schmar"/>
</rdf:Description>

<rdf:Description rdf:about="http://resource.geolba.ac.at/doc/0">
	<skos:hasTopConcept rdf:resource="http://resource.geolba.ac.at/doc/35"/>
</rdf:Description>

<rdf:Description rdf:about="http://resource.geolba.ac.at/doc/8">
	<skos:broader rdf:resource="http://resource.geolba.ac.at/doc/1"/>
</rdf:Description>

<rdf:Description rdf:about="http://resource.geolba.ac.at/doc/84">
	<dcterms:creator rdf:resource="http://resource.geolba.ac.at/user/schmar"/>
</rdf:Description>

<rdf:Description rdf:about="http://resource.geolba.ac.at/doc/63">
	<owl:deprecated rdf:datatype="http://www.w3.org/2001/XMLSchema#boolean">true</owl:deprecated>
</rdf:Description>

<rdf:Description rdf:about="http://resource.geolba.ac.at/doc/23">
	<dcterms:creator rdf:resource="http://resource.geolba.ac.at/user/schmar"/>
</rdf:Description>

<rdf:Description rdf:about="http://resource.geolba.ac.at/doc/72">
	<rdf:type rdf:resource="http://www.w3.org/2004/02/skos/core#Concept"/>
</rdf:Description>

<rdf:Description rdf:about="http://resource.geolba.ac.at/doc/8">
	<skos:prefLabel xml:lang="de">Gesteinsbegriffe mit Links nach INSPIRE oder GeoSciML</skos:prefLabel>
</rdf:Description>

<rdf:Description rdf:about="http://resource.geolba.ac.at/doc/18">
	<skos:broader rdf:resource="http://resource.geolba.ac.at/doc/17"/>
</rdf:Description>

<rdf:Description rdf:about="http://resource.geolba.ac.at/doc/160">
	<rdf:type rdf:resource="http://www.w3.org/2004/02/skos/core#Concept"/>
</rdf:Description>

<rdf:Description rdf:about="http://resource.geolba.ac.at/doc/167">
	<skos:prefLabel xml:lang="en">All concepts in a one table (extended SQL dump)</skos:prefLabel>
</rdf:Description>

<rdf:Description rdf:about="http://resource.geolba.ac.at/doc/72">
	<skos:prefLabel xml:lang="en">Geothermal components in ge, en, fr, es</skos:prefLabel>
</rdf:Description>

<rdf:Description rdf:about="http://resource.geolba.ac.at/doc/46">
	<skos:definition xml:lang="de">Weil in den Geowissenschaften auch in der Literatur die gleiche Bezeichnung (Wortlaut, Literal) für verschiedene Fachbereiche verwendet wird. Zum Beispiel „Ton“ als Mineral, als lithologische Materialbeschreibung, oder auch als Rohstoffart. Durch die Verwendung von sogenannten URI’s (Webadressen als eindeutige Identifikatoren) kann exakt auf den gewünschten Begriff referenziert werden.</skos:definition>
</rdf:Description>

<rdf:Description rdf:about="http://resource.geolba.ac.at/doc/77">
	<skos:narrower rdf:resource="http://resource.geolba.ac.at/doc/78"/>
</rdf:Description>

<rdf:Description rdf:about="http://resource.geolba.ac.at/doc/11">
	<dcterms:creator rdf:resource="http://resource.geolba.ac.at/user/schmar"/>
</rdf:Description>

<rdf:Description rdf:about="http://resource.geolba.ac.at/doc/71">
	<skos:prefLabel xml:lang="de">reegle</skos:prefLabel>
	<skos:prefLabel xml:lang="en">reegle</skos:prefLabel>
</rdf:Description>

<rdf:Description rdf:about="http://resource.geolba.ac.at/doc/17">
	<skos:narrower rdf:resource="http://resource.geolba.ac.at/doc/26"/>
</rdf:Description>

<rdf:Description rdf:about="http://resource.geolba.ac.at/doc/26">
	<dcterms:hasVersion rdf:datatype="http://www.w3.org/2001/XMLSchema#int">1</dcterms:hasVersion>
</rdf:Description>

<rdf:Description rdf:about="http://resource.geolba.ac.at/doc/81">
	<skos:prefLabel xml:lang="en">All Geologic units with descriptions in German and English</skos:prefLabel>
</rdf:Description>

<rdf:Description rdf:about="http://resource.geolba.ac.at/doc/164">
	<skos:prefLabel xml:lang="de">Begriffe mit Referenzpunkt und Koordinatenangabe</skos:prefLabel>
</rdf:Description>

<rdf:Description rdf:about="http://resource.geolba.ac.at/doc/15">
	<rdf:type rdf:resource="http://www.w3.org/2004/02/skos/core#Concept"/>
</rdf:Description>

<rdf:Description rdf:about="http://resource.geolba.ac.at/doc/33">
	<skos:prefLabel xml:lang="de">brit. nat. bibliography (BNB)</skos:prefLabel>
</rdf:Description>

<rdf:Description rdf:about="http://resource.geolba.ac.at/doc/62">
	<appliedType xmlns="http://schema.semantic-web.at/ppt/" rdf:resource="http://www.w3.org/2006/vcard/ns#Organization"/>
</rdf:Description>

<rdf:Description rdf:about="http://resource.geolba.ac.at/doc/14">
	<dcterms:hasVersion rdf:datatype="http://www.w3.org/2001/XMLSchema#int">3</dcterms:hasVersion>
</rdf:Description>

<rdf:Description rdf:about="http://resource.geolba.ac.at/doc/4">
	<skos:prefLabel xml:lang="de">GBA_Zeitskala</skos:prefLabel>
</rdf:Description>

<rdf:Description rdf:about="http://resource.geolba.ac.at/doc/160">
	<skos:broader rdf:resource="http://resource.geolba.ac.at/doc/159"/>
</rdf:Description>

<rdf:Description rdf:about="http://resource.geolba.ac.at/doc/78">
	<skos:prefLabel xml:lang="de">Baumaterialien (Denkmäler)</skos:prefLabel>
</rdf:Description>

<rdf:Description rdf:about="http://resource.geolba.ac.at/doc/74">
	<skos:prefLabel xml:lang="en">Geothermal projects on reegle-data</skos:prefLabel>
</rdf:Description>

<rdf:Description rdf:about="http://resource.geolba.ac.at/doc/35">
	<skos:prefLabel xml:lang="en">GBA_Mineral Resources</skos:prefLabel>
</rdf:Description>

<rdf:Description rdf:about="http://resource.geolba.ac.at/doc/18">
	<skos:prefLabel xml:lang="de">Berge über 3500m in Österreich</skos:prefLabel>
</rdf:Description>

<rdf:Description rdf:about="http://resource.geolba.ac.at/doc/27">
	<rdf:type rdf:resource="http://www.w3.org/2004/02/skos/core#Concept"/>
</rdf:Description>

<rdf:Description rdf:about="http://resource.geolba.ac.at/doc/47">
	<skos:prefLabel xml:lang="de">Was ist ein Thesaurus?</skos:prefLabel>
</rdf:Description>

<rdf:Description rdf:about="http://resource.geolba.ac.at/doc/79">
	<skos:definition xml:lang="de">http://resource.geolba.ac.at/PoolParty/sparql/gbaex</skos:definition>
</rdf:Description>

<rdf:Description rdf:about="http://resource.geolba.ac.at/doc/39">
	<skos:narrower rdf:resource="http://resource.geolba.ac.at/doc/47"/>
</rdf:Description>

<rdf:Description rdf:about="http://resource.geolba.ac.at/doc/80">
	<dcterms:creator rdf:resource="http://resource.geolba.ac.at/user/schmar"/>
</rdf:Description>

<rdf:Description rdf:about="http://resource.geolba.ac.at/doc/27">
	<dcterms:creator rdf:resource="http://resource.geolba.ac.at/user/schmar"/>
</rdf:Description>

<rdf:Description rdf:about="http://resource.geolba.ac.at/doc/5">
	<skos:prefLabel xml:lang="de">GBA_Struktur</skos:prefLabel>
</rdf:Description>

<rdf:Description rdf:about="http://resource.geolba.ac.at/doc/18">
	<dcterms:hasVersion rdf:datatype="http://www.w3.org/2001/XMLSchema#int">1</dcterms:hasVersion>
</rdf:Description>

<rdf:Description rdf:about="http://resource.geolba.ac.at/doc/79">
	<dcterms:creator rdf:resource="http://resource.geolba.ac.at/user/schmar"/>
</rdf:Description>

<rdf:Description rdf:about="http://resource.geolba.ac.at/doc/21">
	<skos:definition xml:lang="de">PREFIX dcterms:&lt;http://purl.org/dc/terms/&gt;&amp;#xa;PREFIX skos:&lt;http://www.w3.org/2004/02/skos/core#&gt;&amp;#xa;SELECT ?URI ?prefLabelDE ?descEN ?desc2EN&amp;#xa;WHERE&amp;#xa;{&amp;#xa;?URI a skos:Concept . ?URI skos:prefLabel ?prefLabelDE . FILTER(lang(?prefLabelDE)='de') .&amp;#xa;?URI dcterms:references &lt;http://resource.geolba.ac.at/ref/900&gt; . &amp;#xa;?URI skos:definition ?descEN . FILTER(lang(?descEN)='en') .&amp;#xa;FILTER regex(str(?descEN), 'Validity: Valid')&amp;#xa;OPTIONAL{?URI dcterms:description ?desc2EN . FILTER(lang(?desc2EN)!='de')}&amp;#xa;}&amp;#xa;ORDER BY ?prefLabelDE</skos:definition>
</rdf:Description>

<rdf:Description rdf:about="http://resource.geolba.ac.at/doc/166">
	<skos:prefLabel xml:lang="en">Concepts with photos or graphics</skos:prefLabel>
</rdf:Description>

<rdf:Description rdf:about="http://resource.geolba.ac.at/doc/47">
	<skos:broader rdf:resource="http://resource.geolba.ac.at/doc/39"/>
</rdf:Description>

<rdf:Description rdf:about="http://resource.geolba.ac.at/doc/51">
	<dcterms:creator rdf:resource="http://resource.geolba.ac.at/user/schmar"/>
	<skos:prefLabel xml:lang="de">Impressum</skos:prefLabel>
	<skos:broader rdf:resource="http://resource.geolba.ac.at/doc/39"/>
	<rdf:type rdf:resource="http://www.w3.org/2004/02/skos/core#Concept"/>
</rdf:Description>

<rdf:Description rdf:about="http://resource.geolba.ac.at/doc/39">
	<skos:narrower rdf:resource="http://resource.geolba.ac.at/doc/51"/>
</rdf:Description>

<rdf:Description rdf:about="http://resource.geolba.ac.at/doc/51">
	<dcterms:created rdf:datatype="http://www.w3.org/2001/XMLSchema#dateTime">2019-07-11T13:40:58.144Z</dcterms:created>
	<skos:prefLabel xml:lang="en">Imprint</skos:prefLabel>
</rdf:Description>

<rdf:Description rdf:about="http://resource.geolba.ac.at/doc/52">
	<dcterms:creator rdf:resource="http://resource.geolba.ac.at/user/schmar"/>
	<dcterms:created rdf:datatype="http://www.w3.org/2001/XMLSchema#dateTime">2019-07-11T13:49:13.848Z</dcterms:created>
	<rdf:type rdf:resource="http://www.w3.org/2004/02/skos/core#Concept"/>
</rdf:Description>

<rdf:Description rdf:about="http://resource.geolba.ac.at/doc/53">
	<dcterms:creator rdf:resource="http://resource.geolba.ac.at/user/schmar"/>
	<skos:broader rdf:resource="http://resource.geolba.ac.at/doc/39"/>
	<rdf:type rdf:resource="http://www.w3.org/2004/02/skos/core#Concept"/>
</rdf:Description>

<rdf:Description rdf:about="http://resource.geolba.ac.at/doc/39">
	<skos:narrower rdf:resource="http://resource.geolba.ac.at/doc/53"/>
</rdf:Description>

<rdf:Description rdf:about="http://resource.geolba.ac.at/doc/53">
	<skos:prefLabel xml:lang="de">Haftungsausschluss</skos:prefLabel>
	<dcterms:created rdf:datatype="http://www.w3.org/2001/XMLSchema#dateTime">2019-07-11T13:59:53.063Z</dcterms:created>
	<skos:definition xml:lang="de">Die Geologische Bundesanstalt (GBA) übernimmt keine Verantwortung für die Richtigkeit der Inhalte bzw. keine Haftung irgendeiner Art für die zur Verfügung gestellten Informationen oder Services und etwaiger Folgeschäden die aus deren Verwendung resultieren. Obwohl versucht wird die Daten sorgfältig zu überprüfen sind die Inhalte dieser Seite nicht notwendigerweise vollständig, aktuell oder fehlerfrei. Die zur Verfügung gestellten Daten und Dienste stellen eine (wissenschaftliche) Kompilation dar die nicht notwendigerweise die offizielle Meinung der GBA widerspiegelt. Es wird versucht die Information fehlerfrei und so aktuell wie möglich zu halten, darüber hinaus wird versucht berichtete Fehler wenn möglich zu korrigieren. Diese Webseite beinhaltet Links zu externen Seiten über die die GBA keine Kontrolle hat und daher keine Verantwortung übernimmt. Weder die GBA noch Personen die in ihrem Auftrag handeln, können für die Inhalte auf dieser Webseite noch auf deren Verwendung in irgendeiner Weise haftbar gemacht werden. Die GBA behält sich das Recht vor die Inhalte dieser Seite bzw. die Nutzungsbedingungen ohne vorherige Ankündigung zu ändern. Der Nutzer nimmt diesen Haftungsausschluss ausdrücklich zur Kenntnis.&lt;br&gt;&lt;br&gt;Die Website nutzt die Standards HTML5/ES16/JQuery und wurde für die Ansicht in Firefox, Chrome, Safari oder Edge optimiert. MS InternetExplorer11 oder älter wird deshalb nicht mehr unterstützt.</skos:definition>
	<skos:definition xml:lang="en">The Geological Survey of Austria takes no responsibility for the correctness of the contents and no liability (of any sorts) for the information and services provided and possible consequential damage resulting from the use of these. Although we try to scrutinise our data the information on this site is not necessarily complete, up to date or accurate. The provided data and services represent a scientific compilation that may not reflect the official opinion of the Geological Survey of Austria. We try to keep our data as accurate and up to date as possible and in addition we attempt to correct errors if they are reported to us. This website contains links to other external sites over which the Geological Survey of Austria has no control and therefore can take no responsibility. Neither the Geological Survey of Austria nor persons acting in their behalf can be held liable for the contents of this website or their use. The Geological Survey of Austria reserves its right to change the contents of this website and its terms of use without prior announcement. The user of this site takes note and approves this disclaimer.&lt;br&gt;&lt;br&gt;The application uses standards like HTML5/ES16/JQuery and is best viewed with Firefox, Chrome, Safari or Edge. MS InternetExplorer11 and older versions are not supported.</skos:definition>
	<skos:prefLabel xml:lang="en">Disclaimer</skos:prefLabel>
</rdf:Description>

<rdf:Description rdf:about="http://resource.geolba.ac.at/doc/42">
	<skos:definition xml:lang="en">According to Wikipedia Linked Open Data is freely available data - describing a method of publishing structured data so that it can be interlinked and become more useful. This data can directly be accessed via HTTP and/or also via URIs linked to other data. The Thesaurus of the geological survey of Austria fulfills all &lt;a href="http://5stardata.info/"&gt;5 criterias&lt;/a&gt; of Tim Berners-Lee (inventor of the World Wide Web), namely: published on the web, structured data, open format (SKOS, RDF), URIs to denote things, linked to other data to provide context (e.g. dbPedia, GeosciML).</skos:definition>
	<skos:definition xml:lang="de">Laut  Wikipedia werden mit Linked Open Data (LOD) im World Wide Web frei verfügbare Daten bezeichnet, die über Uniform Resource Identifier (URI, Webadresse) identifizierbar sind und direkt per HTTP abgerufen werden können, und ebenfalls per URI auf andere Daten verweisen. Der GBA Thesaurus erfüllt alle  &lt;a href="http://5stardata.info/"&gt;5 Kriterien&lt;/a&gt; von Tim Berners-Lee (Erfinder des www), nämlich im Web publiziert, maschinenlesbar, offenes Format (SKOS), RDF Standard, verlinkt auf andere Resourcen (z.B. dbPedia, GeoSciML).</skos:definition>
</rdf:Description>

<rdf:Description rdf:about="http://resource.geolba.ac.at/doc/39">
	<skos:prefLabel xml:lang="de">Allgemeine Fragen</skos:prefLabel>
	<skos:prefLabel xml:lang="en">General questions</skos:prefLabel>
</rdf:Description>

<rdf:Description rdf:about="http://resource.geolba.ac.at/doc/38">
	<skos:prefLabel xml:lang="en">Practical use</skos:prefLabel>
	<skos:prefLabel xml:lang="de">Anwendung</skos:prefLabel>
</rdf:Description>

<rdf:Description rdf:about="http://resource.geolba.ac.at/doc/54">
	<skos:prefLabel xml:lang="de">FAQ - häufig gestellte Fragen</skos:prefLabel>
	<dcterms:created rdf:datatype="http://www.w3.org/2001/XMLSchema#dateTime">2019-07-23T07:43:06.005Z</dcterms:created>
	<dcterms:creator rdf:resource="http://resource.geolba.ac.at/user/schmar"/>
</rdf:Description>

<rdf:Description rdf:about="http://resource.geolba.ac.at/doc/37">
	<skos:hasTopConcept rdf:resource="http://resource.geolba.ac.at/doc/54"/>
</rdf:Description>

<rdf:Description rdf:about="http://resource.geolba.ac.at/doc/54">
	<skos:topConceptOf rdf:resource="http://resource.geolba.ac.at/doc/37"/>
	<rdf:type rdf:resource="http://www.w3.org/2004/02/skos/core#Concept"/>
	<skos:prefLabel xml:lang="en">FAQ - frequently asked questions</skos:prefLabel>
	<skos:narrower rdf:resource="http://resource.geolba.ac.at/doc/39"/>
</rdf:Description>

<rdf:Description rdf:about="http://resource.geolba.ac.at/doc/39">
	<skos:broader rdf:resource="http://resource.geolba.ac.at/doc/54"/>
</rdf:Description>

<rdf:Description rdf:about="http://resource.geolba.ac.at/doc/54">
	<skos:narrower rdf:resource="http://resource.geolba.ac.at/doc/38"/>
</rdf:Description>

<rdf:Description rdf:about="http://resource.geolba.ac.at/doc/38">
	<skos:broader rdf:resource="http://resource.geolba.ac.at/doc/54"/>
</rdf:Description>

<rdf:Description rdf:about="http://resource.geolba.ac.at/doc/54">
	<skos:narrower rdf:resource="http://resource.geolba.ac.at/doc/40"/>
</rdf:Description>

<rdf:Description rdf:about="http://resource.geolba.ac.at/doc/40">
	<skos:broader rdf:resource="http://resource.geolba.ac.at/doc/54"/>
</rdf:Description>

<rdf:Description rdf:about="http://resource.geolba.ac.at/doc/52">
	<skos:prefLabel xml:lang="de">Über den GBA Thesaurus</skos:prefLabel>
	<skos:prefLabel xml:lang="en">About the GBA Thesaurus</skos:prefLabel>
</rdf:Description>

<rdf:Description rdf:about="http://resource.geolba.ac.at/doc/54">
	<skos:narrower rdf:resource="http://resource.geolba.ac.at/doc/52"/>
</rdf:Description>

<rdf:Description rdf:about="http://resource.geolba.ac.at/doc/52">
	<skos:broader rdf:resource="http://resource.geolba.ac.at/doc/54"/>
</rdf:Description>

<rdf:Description rdf:about="http://resource.geolba.ac.at/doc/51">
	<skos:definition xml:lang="de">Koordination: Martin Schiegl&lt;br&gt;Redaktion: Christine Hörfarter&lt;br&gt;Inhalte:  ExpertInnenteams aus den Fachabteilungen Rohstoffe,&lt;br&gt;Kristallingeologie und Sedimentgeologie&lt;br&gt;&lt;br&gt;Geologische Bundesanstalt&lt;br&gt;  Neulinggasse 38&lt;br&gt;  1030 Wien&lt;br&gt;&lt;br&gt;Kontakt: thesaurus@geologie.ac.at
</skos:definition>
</rdf:Description>

<rdf:Description rdf:about="http://resource.geolba.ac.at/doc/86">
	<skos:definition xml:lang="en">The GBA status describes the processing status of the concepts (examination of the content and quality assurance) and their range of use.&lt;br&gt;&lt;br&gt;a) Concept status 0 „Not defined“ - terms and definitions, which are still in process and/or not yet reviewed or assigned to a status by the respective GBA editors.&lt;br&gt;&lt;br&gt;b) Concept status &lt;strong&gt;official use&lt;/strong&gt; - valid for the purposes of the GBA - Editorial reviewed and commonly used term as recommended by the GBA considering the „Empfehlungen (Richtlinien) zur Handhabung der stratigraphischen Nomenklatur“ (Steininger &amp; Piller, 1999) and/or the „North American Stratigraphic Code“ (NACSN, 2005). This applies particularly to recently published units or the creation of new concepts.&lt;br&gt;&lt;br&gt;c) Concept status &lt;strong&gt;informal use&lt;/strong&gt; - informal use within the meaning of the GBA - editorial reviewed and informally used term by the GBA (e.g. inadequately described, is a lithologic term without type locality, etc.), but provides an important basis for the interpretation of the regional geology.&lt;br&gt;&lt;br&gt;d) Concept status &lt;strong&gt;obsolete&lt;/strong&gt; - invalid within the meaning of the GBA - editorial reviewed term, not recommended for use on the part of the GBA since the term is misleading and/or has not been defined correctly or does not correspond to current scientific knowledge.</skos:definition>
</rdf:Description>

<rdf:Description rdf:about="http://resource.geolba.ac.at/doc/33">
	<skos:prefLabel xml:lang="en">brit. nat. bibliography (BNB)</skos:prefLabel>
</rdf:Description>

<rdf:Description rdf:about="http://resource.geolba.ac.at/doc/31">
	<skos:prefLabel xml:lang="en">de.dbPedia (Wikipedia DE)</skos:prefLabel>
</rdf:Description>

<rdf:Description rdf:about="http://resource.geolba.ac.at/doc/13">
	<skos:prefLabel xml:lang="en">enipedia (TU Delft)</skos:prefLabel>
</rdf:Description>

<rdf:Description rdf:about="http://resource.geolba.ac.at/doc/29">
	<skos:prefLabel xml:lang="en">environment agency EEA</skos:prefLabel>
</rdf:Description>

<rdf:Description rdf:about="http://resource.geolba.ac.at/doc/25">
	<skos:prefLabel xml:lang="en"> eurostat</skos:prefLabel>
</rdf:Description>

<rdf:Description rdf:about="http://resource.geolba.ac.at/doc/17">
	<skos:prefLabel xml:lang="en">factForge</skos:prefLabel>
</rdf:Description>

<rdf:Description rdf:about="http://resource.geolba.ac.at/doc/73">
	<skos:prefLabel xml:lang="en">reegle-data</skos:prefLabel>
</rdf:Description>

<rdf:Description rdf:about="http://resource.geolba.ac.at/doc/15">
	<skos:prefLabel xml:lang="en">dbPedia.org (Wikipedia)</skos:prefLabel>
</rdf:Description>

<rdf:Description rdf:about="http://resource.geolba.ac.at/doc/79">
	<skos:prefLabel xml:lang="en">geoexkursionen</skos:prefLabel>
</rdf:Description>

<rdf:Description rdf:about="http://resource.geolba.ac.at/doc/158">
	<dcterms:title xml:lang="en">Bookmarks</dcterms:title>
</rdf:Description>

<rdf:Description rdf:about="http://resource.geolba.ac.at/doc/61">
	<dcterms:title xml:lang="en">Organisation</dcterms:title>
</rdf:Description>

<rdf:Description rdf:about="http://resource.geolba.ac.at/doc/37">
	<dcterms:title xml:lang="en">FAQ</dcterms:title>
	<dcterms:description xml:lang="de">Häufig gestellte Fragen</dcterms:description>
	<dcterms:description xml:lang="en">Frequently asked questions</dcterms:description>
</rdf:Description>

<rdf:Description rdf:about="http://resource.geolba.ac.at/doc/33">
	<dcterms:contributor rdf:resource="http://resource.geolba.ac.at/user/schmar"/>
</rdf:Description>

<rdf:Description rdf:about="http://resource.geolba.ac.at/doc/32">
	<dcterms:contributor rdf:resource="http://resource.geolba.ac.at/user/schmar"/>
</rdf:Description>

<rdf:Description rdf:about="http://resource.geolba.ac.at/doc/158">
	<dcterms:modified rdf:datatype="http://www.w3.org/2001/XMLSchema#dateTime">2019-07-23T08:50:53.022Z</dcterms:modified>
</rdf:Description>

<rdf:Description rdf:about="http://resource.geolba.ac.at/doc/157">
	<dcterms:modified rdf:datatype="http://www.w3.org/2001/XMLSchema#dateTime">2016-10-19T12:55:53.000Z</dcterms:modified>
</rdf:Description>

<rdf:Description rdf:about="http://resource.geolba.ac.at/doc/156">
	<dcterms:modified rdf:datatype="http://www.w3.org/2001/XMLSchema#dateTime">2016-06-02T13:02:17.000Z</dcterms:modified>
</rdf:Description>

<rdf:Description rdf:about="http://resource.geolba.ac.at/doc/28">
	<dcterms:modified rdf:datatype="http://www.w3.org/2001/XMLSchema#dateTime">2014-07-01T11:27:42.000Z</dcterms:modified>
</rdf:Description>

<rdf:Description rdf:about="http://resource.geolba.ac.at/doc/27">
	<dcterms:modified rdf:datatype="http://www.w3.org/2001/XMLSchema#dateTime">2014-07-01T11:28:07.000Z</dcterms:modified>
</rdf:Description>

<rdf:Description rdf:about="http://resource.geolba.ac.at/doc/26">
	<dcterms:modified rdf:datatype="http://www.w3.org/2001/XMLSchema#dateTime">2014-09-26T13:06:02.000Z</dcterms:modified>
</rdf:Description>

<rdf:Description rdf:about="http://resource.geolba.ac.at/doc/25">
	<dcterms:modified rdf:datatype="http://www.w3.org/2001/XMLSchema#dateTime">2019-07-23T08:48:51.872Z</dcterms:modified>
</rdf:Description>

<rdf:Description rdf:about="http://resource.geolba.ac.at/doc/29">
	<dcterms:modified rdf:datatype="http://www.w3.org/2001/XMLSchema#dateTime">2019-07-23T08:48:40.824Z</dcterms:modified>
</rdf:Description>

<rdf:Description rdf:about="http://resource.geolba.ac.at/doc/20">
	<dcterms:modified rdf:datatype="http://www.w3.org/2001/XMLSchema#dateTime">2014-09-26T12:58:12.000Z</dcterms:modified>
</rdf:Description>

<rdf:Description rdf:about="http://resource.geolba.ac.at/doc/8">
	<dcterms:modified rdf:datatype="http://www.w3.org/2001/XMLSchema#dateTime">2014-09-26T13:01:06.000Z</dcterms:modified>
</rdf:Description>

<rdf:Description rdf:about="http://resource.geolba.ac.at/doc/7">
	<dcterms:modified rdf:datatype="http://www.w3.org/2001/XMLSchema#dateTime">2014-09-26T12:58:58.000Z</dcterms:modified>
</rdf:Description>

<rdf:Description rdf:about="http://resource.geolba.ac.at/doc/62">
	<dcterms:modified rdf:datatype="http://www.w3.org/2001/XMLSchema#dateTime">2015-11-25T09:35:35.000Z</dcterms:modified>
</rdf:Description>

<rdf:Description rdf:about="http://resource.geolba.ac.at/doc/5">
	<dcterms:modified rdf:datatype="http://www.w3.org/2001/XMLSchema#dateTime">2014-06-13T09:28:11.000Z</dcterms:modified>
</rdf:Description>

<rdf:Description rdf:about="http://resource.geolba.ac.at/doc/61">
	<dcterms:modified rdf:datatype="http://www.w3.org/2001/XMLSchema#dateTime">2019-07-23T08:51:06.321Z</dcterms:modified>
</rdf:Description>

<rdf:Description rdf:about="http://resource.geolba.ac.at/doc/24">
	<dcterms:modified rdf:datatype="http://www.w3.org/2001/XMLSchema#dateTime">2014-09-26T13:03:27.000Z</dcterms:modified>
</rdf:Description>

<rdf:Description rdf:about="http://resource.geolba.ac.at/doc/23">
	<dcterms:modified rdf:datatype="http://www.w3.org/2001/XMLSchema#dateTime">2014-09-26T13:00:33.000Z</dcterms:modified>
</rdf:Description>

<rdf:Description rdf:about="http://resource.geolba.ac.at/doc/66">
	<dcterms:modified rdf:datatype="http://www.w3.org/2001/XMLSchema#dateTime">2014-10-28T07:46:22.000Z</dcterms:modified>
</rdf:Description>

<rdf:Description rdf:about="http://resource.geolba.ac.at/doc/21">
	<dcterms:modified rdf:datatype="http://www.w3.org/2001/XMLSchema#dateTime">2014-09-26T13:00:10.000Z</dcterms:modified>
</rdf:Description>

<rdf:Description rdf:about="http://resource.geolba.ac.at/doc/9">
	<dcterms:modified rdf:datatype="http://www.w3.org/2001/XMLSchema#dateTime">2014-09-26T13:01:27.000Z</dcterms:modified>
</rdf:Description>

<rdf:Description rdf:about="http://resource.geolba.ac.at/doc/4">
	<dcterms:modified rdf:datatype="http://www.w3.org/2001/XMLSchema#dateTime">2014-06-13T09:29:14.000Z</dcterms:modified>
</rdf:Description>

<rdf:Description rdf:about="http://resource.geolba.ac.at/doc/3">
	<dcterms:modified rdf:datatype="http://www.w3.org/2001/XMLSchema#dateTime">2016-10-19T12:56:19.000Z</dcterms:modified>
</rdf:Description>

<rdf:Description rdf:about="http://resource.geolba.ac.at/doc/2">
	<dcterms:modified rdf:datatype="http://www.w3.org/2001/XMLSchema#dateTime">2016-06-02T11:47:57.000Z</dcterms:modified>
</rdf:Description>

<rdf:Description rdf:about="http://resource.geolba.ac.at/doc/1">
	<dcterms:modified rdf:datatype="http://www.w3.org/2001/XMLSchema#dateTime">2014-06-13T09:27:31.000Z</dcterms:modified>
</rdf:Description>

<rdf:Description rdf:about="http://resource.geolba.ac.at/doc/17">
	<dcterms:modified rdf:datatype="http://www.w3.org/2001/XMLSchema#dateTime">2019-07-23T08:49:01.780Z</dcterms:modified>
</rdf:Description>

<rdf:Description rdf:about="http://resource.geolba.ac.at/doc/16">
	<dcterms:modified rdf:datatype="http://www.w3.org/2001/XMLSchema#dateTime">2014-09-26T13:04:20.000Z</dcterms:modified>
</rdf:Description>

<rdf:Description rdf:about="http://resource.geolba.ac.at/doc/15">
	<dcterms:modified rdf:datatype="http://www.w3.org/2001/XMLSchema#dateTime">2019-07-23T08:49:54.465Z</dcterms:modified>
</rdf:Description>

<rdf:Description rdf:about="http://resource.geolba.ac.at/doc/14">
	<dcterms:modified rdf:datatype="http://www.w3.org/2001/XMLSchema#dateTime">2014-09-26T13:05:08.000Z</dcterms:modified>
</rdf:Description>

<rdf:Description rdf:about="http://resource.geolba.ac.at/doc/19">
	<dcterms:modified rdf:datatype="http://www.w3.org/2001/XMLSchema#dateTime">2015-03-26T07:17:18.000Z</dcterms:modified>
</rdf:Description>

<rdf:Description rdf:about="http://resource.geolba.ac.at/doc/18">
	<dcterms:modified rdf:datatype="http://www.w3.org/2001/XMLSchema#dateTime">2014-09-26T13:05:46.000Z</dcterms:modified>
</rdf:Description>

<rdf:Description rdf:about="http://resource.geolba.ac.at/doc/53">
	<dcterms:modified rdf:datatype="http://www.w3.org/2001/XMLSchema#dateTime">2019-07-11T14:01:01.767Z</dcterms:modified>
</rdf:Description>

<rdf:Description rdf:about="http://resource.geolba.ac.at/doc/51">
	<dcterms:modified rdf:datatype="http://www.w3.org/2001/XMLSchema#dateTime">2019-07-23T08:16:08.684Z</dcterms:modified>
</rdf:Description>

<rdf:Description rdf:about="http://resource.geolba.ac.at/doc/13">
	<dcterms:modified rdf:datatype="http://www.w3.org/2001/XMLSchema#dateTime">2019-07-23T08:48:32.386Z</dcterms:modified>
</rdf:Description>

<rdf:Description rdf:about="http://resource.geolba.ac.at/doc/11">
	<dcterms:modified rdf:datatype="http://www.w3.org/2001/XMLSchema#dateTime">2014-09-26T13:02:08.000Z</dcterms:modified>
</rdf:Description>

<rdf:Description rdf:about="http://resource.geolba.ac.at/doc/10">
	<dcterms:modified rdf:datatype="http://www.w3.org/2001/XMLSchema#dateTime">2014-09-26T13:01:48.000Z</dcterms:modified>
</rdf:Description>

<rdf:Description rdf:about="http://resource.geolba.ac.at/doc/54">
	<dcterms:modified rdf:datatype="http://www.w3.org/2001/XMLSchema#dateTime">2019-07-23T08:15:17.024Z</dcterms:modified>
</rdf:Description>

<rdf:Description rdf:about="http://resource.geolba.ac.at/doc/adms/0.1">
	<dcterms:modified rdf:datatype="http://www.w3.org/2001/XMLSchema#dateTime">2018-10-02T11:19:53.000Z</dcterms:modified>
</rdf:Description>

<rdf:Description rdf:about="http://resource.geolba.ac.at/doc/48">
	<dcterms:modified rdf:datatype="http://www.w3.org/2001/XMLSchema#dateTime">2014-09-30T09:31:22.000Z</dcterms:modified>
</rdf:Description>

<rdf:Description rdf:about="http://resource.geolba.ac.at/doc/47">
	<dcterms:modified rdf:datatype="http://www.w3.org/2001/XMLSchema#dateTime">2014-09-30T09:30:29.000Z</dcterms:modified>
</rdf:Description>

<rdf:Description rdf:about="http://resource.geolba.ac.at/doc/42">
	<dcterms:modified rdf:datatype="http://www.w3.org/2001/XMLSchema#dateTime">2019-07-18T13:34:25.691Z</dcterms:modified>
</rdf:Description>

<rdf:Description rdf:about="http://resource.geolba.ac.at/doc/41">
	<dcterms:modified rdf:datatype="http://www.w3.org/2001/XMLSchema#dateTime">2014-09-30T09:43:50.000Z</dcterms:modified>
</rdf:Description>

<rdf:Description rdf:about="http://resource.geolba.ac.at/doc/84">
	<dcterms:modified rdf:datatype="http://www.w3.org/2001/XMLSchema#dateTime">2015-03-23T09:20:35.000Z</dcterms:modified>
</rdf:Description>

<rdf:Description rdf:about="http://resource.geolba.ac.at/doc/46">
	<dcterms:modified rdf:datatype="http://www.w3.org/2001/XMLSchema#dateTime">2014-09-30T09:32:27.000Z</dcterms:modified>
</rdf:Description>

<rdf:Description rdf:about="http://resource.geolba.ac.at/doc/45">
	<dcterms:modified rdf:datatype="http://www.w3.org/2001/XMLSchema#dateTime">2015-04-02T09:25:00.000Z</dcterms:modified>
</rdf:Description>

<rdf:Description rdf:about="http://resource.geolba.ac.at/doc/88">
	<dcterms:modified rdf:datatype="http://www.w3.org/2001/XMLSchema#dateTime">2015-06-12T08:05:27.000Z</dcterms:modified>
</rdf:Description>

<rdf:Description rdf:about="http://resource.geolba.ac.at/doc/82">
	<dcterms:modified rdf:datatype="http://www.w3.org/2001/XMLSchema#dateTime">2015-03-23T10:52:09.000Z</dcterms:modified>
</rdf:Description>

<rdf:Description rdf:about="http://resource.geolba.ac.at/doc/81">
	<dcterms:modified rdf:datatype="http://www.w3.org/2001/XMLSchema#dateTime">2015-01-09T13:18:53.000Z</dcterms:modified>
</rdf:Description>

<rdf:Description rdf:about="http://resource.geolba.ac.at/doc/80">
	<dcterms:modified rdf:datatype="http://www.w3.org/2001/XMLSchema#dateTime">2014-12-18T13:11:08.000Z</dcterms:modified>
</rdf:Description>

<rdf:Description rdf:about="http://resource.geolba.ac.at/doc/39">
	<dcterms:modified rdf:datatype="http://www.w3.org/2001/XMLSchema#dateTime">2019-07-23T08:15:34.012Z</dcterms:modified>
</rdf:Description>

<rdf:Description rdf:about="http://resource.geolba.ac.at/doc/38">
	<dcterms:modified rdf:datatype="http://www.w3.org/2001/XMLSchema#dateTime">2019-07-23T07:44:35.825Z</dcterms:modified>
</rdf:Description>

<rdf:Description rdf:about="http://resource.geolba.ac.at/doc/37">
	<dcterms:modified rdf:datatype="http://www.w3.org/2001/XMLSchema#dateTime">2019-07-23T08:56:06.708Z</dcterms:modified>
</rdf:Description>

<rdf:Description rdf:about="http://resource.geolba.ac.at/doc/36">
	<dcterms:modified rdf:datatype="http://www.w3.org/2001/XMLSchema#dateTime">2014-09-26T13:02:28.000Z</dcterms:modified>
</rdf:Description>

<rdf:Description rdf:about="http://resource.geolba.ac.at/doc/75">
	<dcterms:modified rdf:datatype="http://www.w3.org/2001/XMLSchema#dateTime">2014-12-09T13:41:56.000Z</dcterms:modified>
</rdf:Description>

<rdf:Description rdf:about="http://resource.geolba.ac.at/doc/31">
	<dcterms:modified rdf:datatype="http://www.w3.org/2001/XMLSchema#dateTime">2019-07-23T08:48:21.450Z</dcterms:modified>
</rdf:Description>

<rdf:Description rdf:about="http://resource.geolba.ac.at/doc/74">
	<dcterms:modified rdf:datatype="http://www.w3.org/2001/XMLSchema#dateTime">2014-12-09T13:12:11.000Z</dcterms:modified>
</rdf:Description>

<rdf:Description rdf:about="http://resource.geolba.ac.at/doc/30">
	<dcterms:modified rdf:datatype="http://www.w3.org/2001/XMLSchema#dateTime">2014-09-26T13:05:27.000Z</dcterms:modified>
</rdf:Description>

<rdf:Description rdf:about="http://resource.geolba.ac.at/doc/73">
	<dcterms:modified rdf:datatype="http://www.w3.org/2001/XMLSchema#dateTime">2019-07-23T08:49:18.457Z</dcterms:modified>
</rdf:Description>

<rdf:Description rdf:about="http://resource.geolba.ac.at/doc/72">
	<dcterms:modified rdf:datatype="http://www.w3.org/2001/XMLSchema#dateTime">2014-12-09T10:33:56.000Z</dcterms:modified>
</rdf:Description>

<rdf:Description rdf:about="http://resource.geolba.ac.at/doc/79">
	<dcterms:modified rdf:datatype="http://www.w3.org/2001/XMLSchema#dateTime">2019-07-23T08:50:05.388Z</dcterms:modified>
</rdf:Description>

<rdf:Description rdf:about="http://resource.geolba.ac.at/doc/34">
	<dcterms:modified rdf:datatype="http://www.w3.org/2001/XMLSchema#dateTime">2014-07-02T13:40:26.000Z</dcterms:modified>
</rdf:Description>

<rdf:Description rdf:about="http://resource.geolba.ac.at/doc/78">
	<dcterms:modified rdf:datatype="http://www.w3.org/2001/XMLSchema#dateTime">2014-12-09T14:47:13.000Z</dcterms:modified>
</rdf:Description>

<rdf:Description rdf:about="http://resource.geolba.ac.at/doc/77">
	<dcterms:modified rdf:datatype="http://www.w3.org/2001/XMLSchema#dateTime">2014-12-09T14:46:02.000Z</dcterms:modified>
</rdf:Description>

<rdf:Description rdf:about="http://resource.geolba.ac.at/doc/33">
	<dcterms:modified rdf:datatype="http://www.w3.org/2001/XMLSchema#dateTime">2019-07-23T08:48:04.167Z</dcterms:modified>
</rdf:Description>

<rdf:Description rdf:about="http://resource.geolba.ac.at/doc/76">
	<dcterms:modified rdf:datatype="http://www.w3.org/2001/XMLSchema#dateTime">2014-12-09T13:43:37.000Z</dcterms:modified>
</rdf:Description>

<rdf:Description rdf:about="http://resource.geolba.ac.at/doc/32">
	<dcterms:modified rdf:datatype="http://www.w3.org/2001/XMLSchema#dateTime">2014-09-26T13:04:49.000Z</dcterms:modified>
</rdf:Description>

<rdf:Description rdf:about="http://resource.geolba.ac.at/doc/71">
	<dcterms:modified rdf:datatype="http://www.w3.org/2001/XMLSchema#dateTime">2014-12-09T10:32:18.000Z</dcterms:modified>
</rdf:Description>

<rdf:Description rdf:about="http://resource.geolba.ac.at/doc/154">
	<dcterms:contributor rdf:resource="http://resource.geolba.ac.at/user/schmar"/>
</rdf:Description>

<rdf:Description rdf:about="http://resource.geolba.ac.at/doc/157">
	<dcterms:contributor rdf:resource="http://resource.geolba.ac.at/user/schmar"/>
</rdf:Description>

<rdf:Description rdf:about="http://resource.geolba.ac.at/doc/156">
	<dcterms:contributor rdf:resource="http://resource.geolba.ac.at/user/schmar"/>
</rdf:Description>

<rdf:Description rdf:about="http://resource.geolba.ac.at/doc/28">
	<dcterms:contributor rdf:resource="http://resource.geolba.ac.at/user/schmar"/>
</rdf:Description>

<rdf:Description rdf:about="http://resource.geolba.ac.at/doc/27">
	<dcterms:contributor rdf:resource="http://resource.geolba.ac.at/user/schmar"/>
</rdf:Description>

<rdf:Description rdf:about="http://resource.geolba.ac.at/doc/26">
	<dcterms:contributor rdf:resource="http://resource.geolba.ac.at/user/schmar"/>
</rdf:Description>

<rdf:Description rdf:about="http://resource.geolba.ac.at/doc/25">
	<dcterms:contributor rdf:resource="http://resource.geolba.ac.at/user/schmar"/>
</rdf:Description>

<rdf:Description rdf:about="http://resource.geolba.ac.at/doc/159">
	<dcterms:contributor rdf:resource="http://resource.geolba.ac.at/user/schmar"/>
</rdf:Description>

<rdf:Description rdf:about="http://resource.geolba.ac.at/doc/29">
	<dcterms:contributor rdf:resource="http://resource.geolba.ac.at/user/schmar"/>
</rdf:Description>

<rdf:Description rdf:about="http://resource.geolba.ac.at/doc/8">
	<dcterms:contributor rdf:resource="http://resource.geolba.ac.at/user/schmar"/>
</rdf:Description>

<rdf:Description rdf:about="http://resource.geolba.ac.at/doc/20">
	<dcterms:contributor rdf:resource="http://resource.geolba.ac.at/user/schmar"/>
</rdf:Description>

<rdf:Description rdf:about="http://resource.geolba.ac.at/doc/7">
	<dcterms:contributor rdf:resource="http://resource.geolba.ac.at/user/schmar"/>
</rdf:Description>

<rdf:Description rdf:about="http://resource.geolba.ac.at/doc/62">
	<dcterms:contributor rdf:resource="http://resource.geolba.ac.at/user/schmar"/>
</rdf:Description>

<rdf:Description rdf:about="http://resource.geolba.ac.at/doc/5">
	<dcterms:contributor rdf:resource="http://resource.geolba.ac.at/user/schmar"/>
</rdf:Description>

<rdf:Description rdf:about="http://resource.geolba.ac.at/doc/24">
	<dcterms:contributor rdf:resource="http://resource.geolba.ac.at/user/schmar"/>
</rdf:Description>

<rdf:Description rdf:about="http://resource.geolba.ac.at/doc/23">
	<dcterms:contributor rdf:resource="http://resource.geolba.ac.at/user/schmar"/>
</rdf:Description>

<rdf:Description rdf:about="http://resource.geolba.ac.at/doc/9">
	<dcterms:contributor rdf:resource="http://resource.geolba.ac.at/user/schmar"/>
</rdf:Description>

<rdf:Description rdf:about="http://resource.geolba.ac.at/doc/21">
	<dcterms:contributor rdf:resource="http://resource.geolba.ac.at/user/schmar"/>
</rdf:Description>

<rdf:Description rdf:about="http://resource.geolba.ac.at/doc/4">
	<dcterms:contributor rdf:resource="http://resource.geolba.ac.at/user/schmar"/>
</rdf:Description>

<rdf:Description rdf:about="http://resource.geolba.ac.at/doc/161">
	<dcterms:contributor rdf:resource="http://resource.geolba.ac.at/user/schmar"/>
</rdf:Description>

<rdf:Description rdf:about="http://resource.geolba.ac.at/doc/3">
	<dcterms:contributor rdf:resource="http://resource.geolba.ac.at/user/schmar"/>
</rdf:Description>

<rdf:Description rdf:about="http://resource.geolba.ac.at/doc/160">
	<dcterms:contributor rdf:resource="http://resource.geolba.ac.at/user/schmar"/>
</rdf:Description>

<rdf:Description rdf:about="http://resource.geolba.ac.at/doc/2">
	<dcterms:contributor rdf:resource="http://resource.geolba.ac.at/user/schmar"/>
</rdf:Description>

<rdf:Description rdf:about="http://resource.geolba.ac.at/doc/1">
	<dcterms:contributor rdf:resource="http://resource.geolba.ac.at/user/schmar"/>
</rdf:Description>

<rdf:Description rdf:about="http://resource.geolba.ac.at/doc/165">
	<dcterms:contributor rdf:resource="http://resource.geolba.ac.at/user/schmar"/>
</rdf:Description>

<rdf:Description rdf:about="http://resource.geolba.ac.at/doc/164">
	<dcterms:contributor rdf:resource="http://resource.geolba.ac.at/user/schmar"/>
</rdf:Description>

<rdf:Description rdf:about="http://resource.geolba.ac.at/doc/163">
	<dcterms:contributor rdf:resource="http://resource.geolba.ac.at/user/schmar"/>
</rdf:Description>

<rdf:Description rdf:about="http://resource.geolba.ac.at/doc/162">
	<dcterms:contributor rdf:resource="http://resource.geolba.ac.at/user/schmar"/>
</rdf:Description>

<rdf:Description rdf:about="http://resource.geolba.ac.at/doc/167">
	<dcterms:contributor rdf:resource="http://resource.geolba.ac.at/user/schmar"/>
</rdf:Description>

<rdf:Description rdf:about="http://resource.geolba.ac.at/doc/166">
	<dcterms:contributor rdf:resource="http://resource.geolba.ac.at/user/schmar"/>
</rdf:Description>

<rdf:Description rdf:about="http://resource.geolba.ac.at/doc/17">
	<dcterms:contributor rdf:resource="http://resource.geolba.ac.at/user/schmar"/>
</rdf:Description>

<rdf:Description rdf:about="http://resource.geolba.ac.at/doc/16">
	<dcterms:contributor rdf:resource="http://resource.geolba.ac.at/user/schmar"/>
</rdf:Description>

<rdf:Description rdf:about="http://resource.geolba.ac.at/doc/15">
	<dcterms:contributor rdf:resource="http://resource.geolba.ac.at/user/schmar"/>
</rdf:Description>

<rdf:Description rdf:about="http://resource.geolba.ac.at/doc/14">
	<dcterms:contributor rdf:resource="http://resource.geolba.ac.at/user/schmar"/>
</rdf:Description>

<rdf:Description rdf:about="http://resource.geolba.ac.at/doc/19">
	<dcterms:contributor rdf:resource="http://resource.geolba.ac.at/user/schmar"/>
</rdf:Description>

<rdf:Description rdf:about="http://resource.geolba.ac.at/doc/18">
	<dcterms:contributor rdf:resource="http://resource.geolba.ac.at/user/schmar"/>
</rdf:Description>

<rdf:Description rdf:about="http://resource.geolba.ac.at/doc/53">
	<dcterms:contributor rdf:resource="http://resource.geolba.ac.at/user/schmar"/>
</rdf:Description>

<rdf:Description rdf:about="http://resource.geolba.ac.at/doc/52">
	<dcterms:contributor rdf:resource="http://resource.geolba.ac.at/user/schmar"/>
</rdf:Description>

<rdf:Description rdf:about="http://resource.geolba.ac.at/doc/51">
	<dcterms:contributor rdf:resource="http://resource.geolba.ac.at/user/schmar"/>
</rdf:Description>

<rdf:Description rdf:about="http://resource.geolba.ac.at/doc/13">
	<dcterms:contributor rdf:resource="http://resource.geolba.ac.at/user/schmar"/>
</rdf:Description>

<rdf:Description rdf:about="http://resource.geolba.ac.at/doc/11">
	<dcterms:contributor rdf:resource="http://resource.geolba.ac.at/user/schmar"/>
</rdf:Description>

<rdf:Description rdf:about="http://resource.geolba.ac.at/doc/10">
	<dcterms:contributor rdf:resource="http://resource.geolba.ac.at/user/schmar"/>
</rdf:Description>

<rdf:Description rdf:about="http://resource.geolba.ac.at/doc/54">
	<dcterms:contributor rdf:resource="http://resource.geolba.ac.at/user/schmar"/>
</rdf:Description>

<rdf:Description rdf:about="http://resource.geolba.ac.at/doc/42">
	<dcterms:contributor rdf:resource="http://resource.geolba.ac.at/user/schmar"/>
</rdf:Description>

<rdf:Description rdf:about="http://resource.geolba.ac.at/doc/86">
	<dcterms:contributor rdf:resource="http://resource.geolba.ac.at/user/schmar"/>
</rdf:Description>

<rdf:Description rdf:about="http://resource.geolba.ac.at/doc/85">
	<dcterms:contributor rdf:resource="http://resource.geolba.ac.at/user/schmar"/>
</rdf:Description>

<rdf:Description rdf:about="http://resource.geolba.ac.at/doc/40">
	<dcterms:contributor rdf:resource="http://resource.geolba.ac.at/user/schmar"/>
</rdf:Description>

<rdf:Description rdf:about="http://resource.geolba.ac.at/doc/83">
	<dcterms:contributor rdf:resource="http://resource.geolba.ac.at/user/schmar"/>
</rdf:Description>

<rdf:Description rdf:about="http://resource.geolba.ac.at/doc/39">
	<dcterms:contributor rdf:resource="http://resource.geolba.ac.at/user/schmar"/>
</rdf:Description>

<rdf:Description rdf:about="http://resource.geolba.ac.at/doc/38">
	<dcterms:contributor rdf:resource="http://resource.geolba.ac.at/user/schmar"/>
</rdf:Description>

<rdf:Description rdf:about="http://resource.geolba.ac.at/doc/31">
	<dcterms:contributor rdf:resource="http://resource.geolba.ac.at/user/schmar"/>
</rdf:Description>

<rdf:Description rdf:about="http://resource.geolba.ac.at/doc/30">
	<dcterms:contributor rdf:resource="http://resource.geolba.ac.at/user/schmar"/>
</rdf:Description>

<rdf:Description rdf:about="http://resource.geolba.ac.at/doc/73">
	<dcterms:contributor rdf:resource="http://resource.geolba.ac.at/user/schmar"/>
</rdf:Description>

<rdf:Description rdf:about="http://resource.geolba.ac.at/doc/79">
	<dcterms:contributor rdf:resource="http://resource.geolba.ac.at/user/schmar"/>
</rdf:Description>

<rdf:Description rdf:about="http://resource.geolba.ac.at/doc/34">
	<dcterms:contributor rdf:resource="http://resource.geolba.ac.at/user/schmar"/>
</rdf:Description>

<rdf:Description rdf:about="http://resource.geolba.ac.at/doc/0">
	<dcterms:title xml:lang="de">sparqlBookmarks (ALT)</dcterms:title>
	<dcterms:title xml:lang="en">sparqlBookmarks (OLD)</dcterms:title>
</rdf:Description>

<rdf:Description rdf:about="http://resource.geolba.ac.at/doc/161">
	<skos:prefLabel xml:lang="de">Alle untergeordneten Begriffe von einem Begriff mit Beschreibungen</skos:prefLabel>
	<skos:prefLabel xml:lang="en">All narrower concepts plus descriptions</skos:prefLabel>
</rdf:Description>

<rdf:Description rdf:about="http://resource.geolba.ac.at/doc/164">
	<dcterms:modified rdf:datatype="http://www.w3.org/2001/XMLSchema#dateTime">2019-09-27T13:39:28.794Z</dcterms:modified>
</rdf:Description>

<rdf:Description rdf:about="http://resource.geolba.ac.at/doc/161">
	<skos:definition xml:lang="de">E.g. replace [insert URI] with concept URI http://resource.geolba.ac.at/lithology/6&lt;br&gt;&lt;br&gt;
&lt;pre&gt;PREFIX skos:&amp;lt;http://www.w3.org/2004/02/skos/core#&amp;gt;
SELECT *
WHERE {
&amp;lt;[insert URI]&amp;gt; skos:narrower* ?s . 
?s skos:prefLabel ?Label . FILTER(lang(?Label)='en')
OPTIONAL {?s skos:definition ?Definition .
FILTER(lang(?Definition)='en')}
}
&lt;/pre&gt;
and try &amp;nbsp;&amp;nbsp;&lt;a href="https://resource.geolba.ac.at/PoolParty/sparql/lithology"&gt;https://resource.geolba.ac.at/PoolParty/sparql/lithology&lt;/a&amp;&gt;</skos:definition>
	<dcterms:modified rdf:datatype="http://www.w3.org/2001/XMLSchema#dateTime">2019-09-27T13:33:09.063Z</dcterms:modified>
</rdf:Description>

<rdf:Description rdf:about="http://resource.geolba.ac.at/doc/160">
	<skos:definition xml:lang="de">&lt;pre&gt;PREFIX skos:&amp;lt;http://www.w3.org/2004/02/skos/core#&amp;gt;
PREFIX dcterms:&amp;lt;http://purl.org/dc/terms/&amp;gt;
SELECT ?URI ?prefLabelDE ?date
WHERE
{
?URI a skos:Concept . ?URI skos:prefLabel ?prefLabelDE . 
FILTER(lang(?prefLabelDE)='de') . ?URI dcterms:modified ?date
}
ORDER BY DESC (?date)
LIMIT 10
&lt;/pre&gt;
e.g. try &amp;nbsp;&amp;nbsp;&lt;a href="https://resource.geolba.ac.at/PoolParty/sparql/lithology"&gt;https://resource.geolba.ac.at/PoolParty/sparql/lithology&lt;/a&amp;&gt;</skos:definition>
	<dcterms:modified rdf:datatype="http://www.w3.org/2001/XMLSchema#dateTime">2019-09-27T13:37:31.584Z</dcterms:modified>
</rdf:Description>

<rdf:Description rdf:about="http://resource.geolba.ac.at/doc/167">
	<skos:definition xml:lang="de">&lt;pre&gt;PREFIX dcterms:&amp;lt;http://purl.org/dc/terms/&amp;gt;
PREFIX skos:&amp;lt;http://www.w3.org/2004/02/skos/core#&amp;gt;
PREFIX geo:&amp;lt;http://www.w3.org/2003/01/geo/wgs84_pos#&amp;gt;
PREFIX dbpo:&amp;lt;http://dbpedia.org/ontology/&amp;gt;
PREFIX gba:&amp;lt;http://resource.geolba.ac.at/schema/thes#&amp;gt;

SELECT ?URI 
(MIN(?prefLabelDE) AS ?PrefLabelDe) (MIN(?prefLabelEN) AS ?PrefLabelEn)
(MIN(?descDE) AS ?DescriptionDe) (MIN(?descEN) AS ?DescriptionEn)
(GROUP_CONCAT(DISTINCT ?tc; separator = '; ') as ?TopConceptURI)
(GROUP_CONCAT(DISTINCT ?tcpDE; separator = '; ') as ?TopConceptPrefLabelDe)
(GROUP_CONCAT(DISTINCT ?tcpEN; separator = '; ') as ?TopConceptPrefLabelEn)
(GROUP_CONCAT(DISTINCT ?cs; separator = '; ') as ?ConceptSchemeURI)
(GROUP_CONCAT(DISTINCT ?cspDE; separator = '; ') as ?ConceptSchemeTitleDe)
(GROUP_CONCAT(DISTINCT ?cspEN; separator = '; ') as ?ConceptSchemeTitleEn)
(MIN(?color) AS ?HexColor) (MIN(?status) AS ?GBA_Status) 
(MIN(?lat_long) AS ?Pos_Lat_Long)
(GROUP_CONCAT(DISTINCT ?broader; separator = '; ') as ?BroaderConceptURI)
(GROUP_CONCAT(DISTINCT ?broaderDE; separator = '; ') as ?BroaderConceptPrefLabelDe)
(GROUP_CONCAT(DISTINCT ?broaderEN; separator = '; ') as ?BroaderConceptPrefLabelEn)

(MIN(?inspire) AS ?InspireMappingURI) 
(MIN(?dbp) AS ?DBpediaMappingURI) 
(MIN(?gsml) AS ?GeoscimlMappingURI) 
(MIN(?bgs) AS ?BgsMappingURI) 
(MIN(?notation) AS ?Notation)
(MIN(?DC) AS ?DateCreated) 
(MIN(?DM) AS ?DateModified)

WHERE
{
?URI a skos:Concept .
FILTER (regex(str(?URI), '^http://resource.geolba.ac.at/.'))  
OPTIONAL {?URI skos:prefLabel ?prefLabelDE . FILTER(lang(?prefLabelDE)='de')} .
OPTIONAL {?URI skos:prefLabel ?prefLabelEN . FILTER(lang(?prefLabelEN)='en')} .
OPTIONAL {?URI skos:definition ?descDE . FILTER(lang(?descDE)='de')} .
OPTIONAL {?URI skos:definition ?descEN . FILTER(lang(?descEN)='en')} .
OPTIONAL {?URI dbpo:colourHexCode ?color} .
OPTIONAL {?URI gba:status ?status} .
OPTIONAL {?URI geo:lat_long ?lat_long} .
OPTIONAL {?URI skos:broader ?broader . ?broader skos:prefLabel ?broaderDE .
FILTER(lang(?broaderDE)='de')} . 
OPTIONAL {?URI skos:broader ?broader . ?broader skos:prefLabel ?broaderEN .
FILTER(lang(?broaderEN)='en')} .

OPTIONAL {
{?URI skos:exactMatch ?inspire}
UNION
{?URI skos:closeMatch ?inspire}
UNION
{?URI skos:broadMatch ?inspire}
UNION
{?URI skos:narrowMatch ?inspire} .
FILTER regex(str(?inspire), '^http://inspire.ec.europa.eu')} .

OPTIONAL {
{?URI skos:exactMatch ?dbp} UNION {?URI skos:closeMatch ?dbp}
UNION
{?URI skos:broadMatch ?dbp} UNION {?URI skos:narrowMatch ?dbp} .
FILTER regex(str(?dbp), '^http://dbpedia.org')} .

OPTIONAL {
{?URI skos:exactMatch ?gsml} UNION {?URI skos:closeMatch ?gsml}
UNION
{?URI skos:broadMatch ?gsml} UNION {?URI skos:narrowMatch ?gsml} .
FILTER regex(str(?gsml), '^http://resource.geosciml.org')} .

OPTIONAL {
{?URI skos:exactMatch ?bgs} UNION {?URI skos:closeMatch ?bgs}
UNION
{?URI skos:broadMatch ?bgs} UNION {?URI skos:narrowMatch ?bgs} .
FILTER regex(str(?bgs), '^http://data.bgs.ac.uk')} .

OPTIONAL {?URI skos:notation ?notation} .
OPTIONAL {?URI dcterms:created  ?DC} .
OPTIONAL {?URI dcterms:modified  ?DM} .
OPTIONAL {?URI skos:broader* ?tc . ?cs skos:hasTopConcept ?tc .
?cs dcterms:title ?cspDE . FILTER(lang(?cspDE)='de') . 
?cs dcterms:title ?cspEN . FILTER(lang(?cspEN)='en') .
?tc skos:prefLabel ?tcpDE . FILTER(lang(?tcpDE)='de') . 
?tc skos:prefLabel ?tcpEN . FILTER(lang(?tcpEN)='en')}

}
GROUP BY ?URI
ORDER BY ?URI
&lt;/pre&gt;
e.g. try &amp;nbsp;&amp;nbsp;&lt;a href="https://resource.geolba.ac.at/PoolParty/sparql/lithology"&gt;https://resource.geolba.ac.at/PoolParty/sparql/lithology&lt;/a&amp;&gt;</skos:definition>
	<dcterms:modified rdf:datatype="http://www.w3.org/2001/XMLSchema#dateTime">2019-09-27T13:37:54.992Z</dcterms:modified>
</rdf:Description>

<rdf:Description rdf:about="http://resource.geolba.ac.at/doc/162">
	<skos:definition xml:lang="de">&lt;pre&gt;PREFIX skos:&amp;lt;http://www.w3.org/2004/02/skos/core#&amp;gt;
SELECT ?URI ?prefLabelDE ?definitionDE ?prefLabelEN ?definitionEN 
WHERE {
?URI a skos:Concept ; skos:prefLabel ?prefLabelDE .
FILTER(lang(?prefLabelDE)='de') .
FILTER (!strStarts(?prefLabelDE, '['^^xsd:string)) .
OPTIONAL{?URI skos:prefLabel ?prefLabelEN .
FILTER(lang(?prefLabelEN)='en')}
OPTIONAL{?URI skos:definition ?definitionDE .
FILTER(lang(?definitionDE)='de')} 
OPTIONAL{?URI skos:definition ?definitionEN .
FILTER(lang(?definitionEN)='en')}
} 
ORDER BY ?prefLabelDE
&lt;/pre&gt;
e.g. try &amp;nbsp;&amp;nbsp;&lt;a href="https://resource.geolba.ac.at/PoolParty/sparql/GeologicUnit"&gt;https://resource.geolba.ac.at/PoolParty/sparql/GeologicUnit&lt;/a&amp;&gt;</skos:definition>
	<dcterms:modified rdf:datatype="http://www.w3.org/2001/XMLSchema#dateTime">2019-09-27T13:38:14.085Z</dcterms:modified>
</rdf:Description>

<rdf:Description rdf:about="http://resource.geolba.ac.at/doc/163">
	<skos:definition xml:lang="de">&lt;pre&gt;PREFIX skos:&amp;lt;http://www.w3.org/2004/02/skos/core#&amp;gt;
PREFIX gba:&amp;lt;http://resource.geolba.ac.at/schema/thes#&amp;gt;
SELECT ?URI ?prefLabelDE
WHERE
{
?URI a skos:Concept . ?URI skos:prefLabel ?prefLabelDE . 
FILTER(lang(?prefLabelDE)='de') .
?URI gba:status ?status . 
FILTER regex(str(?status), '1')
}
ORDER BY ?prefLabelDE
&lt;/pre&gt;
e.g. try &amp;nbsp;&amp;nbsp;&lt;a href="https://resource.geolba.ac.at/PoolParty/sparql/GeologicUnit"&gt;https://resource.geolba.ac.at/PoolParty/sparql/GeologicUnit&lt;/a&amp;&gt;</skos:definition>
	<dcterms:modified rdf:datatype="http://www.w3.org/2001/XMLSchema#dateTime">2019-09-27T13:38:46.662Z</dcterms:modified>
</rdf:Description>

<rdf:Description rdf:about="http://resource.geolba.ac.at/doc/166">
	<skos:definition xml:lang="de">&lt;pre&gt;PREFIX skos:&amp;lt;http://www.w3.org/2004/02/skos/core#&amp;gt;
PREFIX foaf:&amp;lt;http://xmlns.com/foaf/0.1/&amp;gt;
SELECT ?s ?Label ?picture
WHERE {
?s foaf:depiction ?picture .
?s skos:prefLabel ?Label . FILTER(lang(?Label)='en')
}
&lt;/pre&gt;
e.g. try &amp;nbsp;&amp;nbsp;&lt;a href="https://resource.geolba.ac.at/PoolParty/sparql/GeologicUnit"&gt;https://resource.geolba.ac.at/PoolParty/sparql/GeologicUnit&lt;/a&amp;&gt;</skos:definition>
	<dcterms:modified rdf:datatype="http://www.w3.org/2001/XMLSchema#dateTime">2019-09-27T13:38:59.669Z</dcterms:modified>
</rdf:Description>

<rdf:Description rdf:about="http://resource.geolba.ac.at/doc/164">
	<skos:definition xml:lang="de">&lt;pre&gt;PREFIX skos:&amp;lt;http://www.w3.org/2004/02/skos/core#&amp;gt;
PREFIX geo:&amp;lt;http://www.w3.org/2003/01/geo/wgs84_pos#&amp;gt;
SELECT 
?URI ?prefLabelDE ?lat_long
WHERE
{
?URI a skos:Concept . ?URI skos:prefLabel ?prefLabelDE . 
FILTER(lang(?prefLabelDE)='en') .
?URI geo:lat_long ?lat_long
}
ORDER BY ?prefLabelDE
&lt;/pre&gt;
e.g. try &amp;nbsp;&amp;nbsp;&lt;a href="https://resource.geolba.ac.at/PoolParty/sparql/GeologicUnit"&gt;https://resource.geolba.ac.at/PoolParty/sparql/GeologicUnit&lt;/a&amp;&gt;</skos:definition>
</rdf:Description>

<rdf:Description rdf:about="http://resource.geolba.ac.at/doc/40">
	<skos:narrower rdf:resource="http://resource.geolba.ac.at/doc/159"/>
</rdf:Description>

<rdf:Description rdf:about="http://resource.geolba.ac.at/doc/159">
	<skos:broader rdf:resource="http://resource.geolba.ac.at/doc/40"/>
</rdf:Description>

<rdf:Description rdf:about="http://resource.geolba.ac.at/doc/40">
	<dcterms:modified rdf:datatype="http://www.w3.org/2001/XMLSchema#dateTime">2019-09-27T13:41:54.227Z</dcterms:modified>
</rdf:Description>

<rdf:Description rdf:about="http://resource.geolba.ac.at/doc/159">
	<skos:definition xml:lang="de">Alle Informationen und Begriffe aus dem GBA Thesaurus können auch direkt über die Datenbank-Schnittstelle (Sparql Endpoint) abgefragt werden. Dazu wird in der Abfragesprache SPARQL der gewünschte Datenbestand definiert und im betreffenden Endpoint abgesendet. Für jedes Thema des GBA Thesaurus steht ein eigener Endpoint zur Verfügung (für Geologische Einheiten z.B. &lt;a href="https://resource.geolba.ac.at/PoolParty/sparql/GeologicUnit"&gt;https://resource.geolba.ac.at/PoolParty/sparql/GeologicUnit&lt;/a&amp;&gt;).</skos:definition>
	<skos:definition xml:lang="en">All information and terms from the GBA thesaurus can also be queried directly via the database interface (Sparql Endpoint). For this purpose, the desired data set is defined in the query language SPARQL and sent in the relevant endpoint. Each topic of the GBA thesaurus has its own endpoint (for geological units e.g. &lt;a href="https://resource.geolba.ac.at/PoolParty/sparql/GeologicUnit"&gt;https://resource.geolba.ac.at/PoolParty/sparql/GeologicUnit&lt;/a&amp;&gt;).</skos:definition>
	<skos:prefLabel xml:lang="de">Beispiele für Datenbank-Abfragen (Sparql bookmarks)</skos:prefLabel>
	<skos:prefLabel xml:lang="en">Examples of database queries (Sparql bookmarks)</skos:prefLabel>
</rdf:Description>

<rdf:Description rdf:about="http://resource.geolba.ac.at/doc/165">
	<skos:broader rdf:resource="http://resource.geolba.ac.at/doc/44"/>
</rdf:Description>

<rdf:Description rdf:about="http://resource.geolba.ac.at/doc/44">
	<skos:narrower rdf:resource="http://resource.geolba.ac.at/doc/165"/>
	<dcterms:contributor rdf:resource="http://resource.geolba.ac.at/user/schmar"/>
</rdf:Description>

<rdf:Description rdf:about="http://resource.geolba.ac.at/doc/165">
	<skos:definition xml:lang="de">&lt;pre&gt;PREFIX skos:&amp;lt;http://www.w3.org/2004/02/skos/core#&amp;gt;
SELECT ?URI ?prefLabel ?desc ?inspire ?gsml
WHERE {
?URI a skos:Concept . ?URI skos:prefLabel ?prefLabel . 
FILTER(lang(?prefLabel)='en') .
OPTIONAL {?URI skos:definition ?desc . 
FILTER(lang(?desc)='en')} .
OPTIONAL {?URI ?p1 ?inspire . 
FILTER (regex(str(?inspire), '^http://inspire.ec.europa.eu'))}
 OPTIONAL {?URI ?p2 ?gsml . 
FILTER (regex(str(?gsml), '^http://resource.geosciml.org'))} 
FILTER (BOUND(?inspire) &amp;vert;&amp;vert; BOUND(?gsml))
}
ORDER BY ?prefLabel
&lt;/pre&gt;
e.g. try &amp;nbsp;&amp;nbsp;&lt;a href="https://resource.geolba.ac.at/PoolParty/sparql/lithology"&gt;https://resource.geolba.ac.at/PoolParty/sparql/lithology&lt;/a&amp;&gt;</skos:definition>
	<dcterms:modified rdf:datatype="http://www.w3.org/2001/XMLSchema#dateTime">2019-09-30T08:14:48.768Z</dcterms:modified>
</rdf:Description>

<rdf:Description rdf:about="http://resource.geolba.ac.at/doc/44">
	<skos:definition xml:lang="de">Begriffe mit Links auf INSPIRE-Codes finden sich hautsächlich in den Themenbereichen: Lithologie, Zeitskala und Rohstoffgeologie - bei den betreffenden Begriffsbeschreibungen unter "Verwandte Begriffe, Relationen" - häufig als "exactMatch" (exakte Übereinstimmung). INSPIRE Links sind auch im "Network diagram" dargestellt und können durch deaktivierien von "Linked Data" aus der Ansicht auch wieder entfernt werden. Zudem können auch detallierte Liste über Datenbankabfragen in Sparql erstellt werden. Siehe auch "Beispiele für Datenbankabfragen".</skos:definition>
	<skos:definition xml:lang="en">Concepts with links to INSPIRE codes can be found mainly in the specific fields: Lithology, time scale and Geology of mineral resources - in the relevant concept descriptions under "Concept relations" - often assigned as "exactMatch". INSPIRE links are also shown in the "Network diagram" and can also be removed by deactivating "Linked Data" from the view. In addition, a detailed list of database queries may be created in Sparql. See also "Database query examples".</skos:definition>
</rdf:Description>

<rdf:Description rdf:about="http://resource.geolba.ac.at/doc/56">
	<dcterms:created rdf:datatype="http://www.w3.org/2001/XMLSchema#dateTime">2019-09-30T11:19:10.972Z</dcterms:created>
	<skos:prefLabel xml:lang="de">Liste aller Begriffe mit Symbolfarbe</skos:prefLabel>
	<skos:broader rdf:resource="http://resource.geolba.ac.at/doc/159"/>
	<dcterms:creator rdf:resource="http://resource.geolba.ac.at/user/schmar"/>
	<rdf:type rdf:resource="http://www.w3.org/2004/02/skos/core#Concept"/>
</rdf:Description>

<rdf:Description rdf:about="http://resource.geolba.ac.at/doc/159">
	<skos:narrower rdf:resource="http://resource.geolba.ac.at/doc/56"/>
</rdf:Description>

<rdf:Description rdf:about="http://resource.geolba.ac.at/doc/56">
	<dcterms:contributor rdf:resource="http://resource.geolba.ac.at/user/schmar"/>
	<skos:prefLabel xml:lang="en">All concepts with web color</skos:prefLabel>
</rdf:Description>

<rdf:Description rdf:about="http://resource.geolba.ac.at/doc/43">
	<skos:definition xml:lang="de">Ja, am besten über die Sparql-Endpoints der Themenbereiche (z.B. auf &lt;a href="https://resource.geolba.ac.at/PoolParty/sparql/lithology"&gt;https://resource.geolba.ac.at/PoolParty/sparql/lithology&lt;/a&gt; für den Themenbereich Lithologie). Es gibt auch eine Sammlung von Abfragebeispielen (Sparql bookmarks, siehe unten). Weiters steht der gesamte Thesaurus auch themenbereichsweise zum Download - im Datenformat RDF/XML auf der Startseite unter "read more".</skos:definition>
	<dcterms:contributor rdf:resource="http://resource.geolba.ac.at/user/schmar"/>
	<skos:narrower rdf:resource="http://resource.geolba.ac.at/doc/159"/>
</rdf:Description>

<rdf:Description rdf:about="http://resource.geolba.ac.at/doc/159">
	<skos:broader rdf:resource="http://resource.geolba.ac.at/doc/43"/>
	<dcterms:modified rdf:datatype="http://www.w3.org/2001/XMLSchema#dateTime">2019-09-30T11:25:22.317Z</dcterms:modified>
</rdf:Description>

<rdf:Description rdf:about="http://resource.geolba.ac.at/doc/43">
	<skos:definition xml:lang="en">Yes, best of all via the Sparql endpoints of the specific fields (eg on &lt;a href="https://resource.geolba.ac.at/PoolParty/sparql/lithology"&gt;https://resource.geolba.ac.at/PoolParty/sparql/lithology&lt;/a&gt; for the topic area lithology). There is also a collection of query examples (Sparql bookmarks, see below). Furthermore, the whole thesaurus can also be downloaded by specific fields - in the data format RDF/XML on the home page under "read more".</skos:definition>
	<dcterms:modified rdf:datatype="http://www.w3.org/2001/XMLSchema#dateTime">2019-09-30T11:27:40.832Z</dcterms:modified>
</rdf:Description>

<rdf:Description rdf:about="http://resource.geolba.ac.at/doc/49">
	<skos:definition xml:lang="de">Alle Texte und Bilder aus dem Thesaurus sind unter der Lizenz: Creative Commons BY-SA 3.0 AT (Namensnennung - Weitergabe unter gleichen Bedingungen 3.0 Österreich, siehe &lt;a href="https://creativecommons.org/licenses/by-sa/3.0/"&gt;https://creativecommons.org/licenses/by-sa/3.0/&lt;/a&gt;) frei verwendbar.</skos:definition>
	<dcterms:contributor rdf:resource="http://resource.geolba.ac.at/user/schmar"/>
	<skos:definition xml:lang="en">Each text or image from the thesaurus is free to use under the license: Creative Commons BY-SA 3.0 AT (Attribution, ShareAlike - read more under &lt;a href="https://creativecommons.org/licenses/by-sa/3.0/"&gt;https://creativecommons.org/licenses/by-sa/3.0/&lt;/a&gt;) </skos:definition>
	<dcterms:modified rdf:datatype="http://www.w3.org/2001/XMLSchema#dateTime">2019-09-30T11:36:20.789Z</dcterms:modified>
</rdf:Description>

<rdf:Description rdf:about="http://resource.geolba.ac.at/doc/56">
	<skos:definition xml:lang="de">&lt;pre&gt;PREFIX skos:&amp;lt;http://www.w3.org/2004/02/skos/core#&amp;gt;
PREFIX dbpo:&amp;lt;http://dbpedia.org/ontology/&amp;gt;
SELECT ?Label ?color ?r ?g ?b ?uri
WHERE {
?uri a skos:Concept; skos:prefLabel ?Label; 
dbpo:colourHexCode ?c . FILTER(lang(?Label)="de") .
BIND(CONCAT("\u003Cspan style='background-color:",?c,
";'\u003E",?c,"\u003C\u002Fspan\u003E") AS ?color)

BIND(REPLACE(REPLACE(REPLACE(REPLACE(REPLACE
(REPLACE(REPLACE(REPLACE(REPLACE(REPLACE
(REPLACE(REPLACE(REPLACE(REPLACE(REPLACE(REPLACE
(?c,"0","00"),"9","09"),"8","08"),
"7","07"),"6","06"),"5","05"),"4","04"),
"3","03"),"2","02"),"1","01"),"F","15"),
"E","14"),"D","13"),"C","12"),"B","11"),
"A","10") AS ?F) .
BIND(xsd:integer(SUBSTR(?F,2,2))*16 + 
xsd:integer(SUBSTR(?F,4,2)) AS ?r) 
BIND(xsd:integer(SUBSTR(?F,6,2))*16 + 
xsd:integer(SUBSTR(?F,8,2)) AS ?g) 
BIND(xsd:integer(SUBSTR(?F,10,2))*16 + 
xsd:integer(SUBSTR(?F,12,2)) AS ?b) 
}
ORDER BY ?Label
&lt;/pre&gt;
e.g. try &amp;nbsp;&amp;nbsp;&lt;a href="https://resource.geolba.ac.at/PoolParty/sparql/lithology"&gt;https://resource.geolba.ac.at/PoolParty/sparql/lithology&lt;/a&gt;</skos:definition>
	<dcterms:modified rdf:datatype="http://www.w3.org/2001/XMLSchema#dateTime">2019-10-01T06:56:22.659Z</dcterms:modified>
</rdf:Description>

<rdf:Description rdf:about="http://resource.geolba.ac.at/doc/50">
	<dcterms:modified rdf:datatype="http://www.w3.org/2001/XMLSchema#dateTime">2019-10-01T11:20:34.088Z</dcterms:modified>
	<skos:definition xml:lang="de">Per Email an das Thesaurus-Redaktionsteam der Geologische Bundesanstalt - &lt;a href="mailto:thesaurus@geologie.ac.at"&gt;thesaurus@geologie.ac.at&lt;/a&gt;. &lt;br&gt;Zusätzlich kann über den Tab "Feedback" im Navigationsbereich rechts oben ein Thesauruskonzept direkt per Email an das Thesaurus-Redaktionsteam kommentiert werden.</skos:definition>
	<dcterms:contributor rdf:resource="http://resource.geolba.ac.at/user/schmar"/>
	<skos:definition xml:lang="en">By email to the Thesaurus editorial team of Geologic Survey of Austria - &lt;a href="mailto:thesaurus@geologie.ac.at"&gt;thesaurus@geologie.ac.at&lt;/a&gt;.
In addition, a thesaurus concept can be commented directly to the Thesaurus Editorial Team via the "Feedback" tab in the navigation area on the top right.</skos:definition>
</rdf:Description>

<rdf:Description rdf:about="http://resource.geolba.ac.at/doc/86">
	<skos:definition xml:lang="de">Der „GBA-Status“ beschreibt den Bearbeitungsstand der Konzepte (Begriffe und ihrer Definitionen), innerhalb des redaktionellen Arbeitsablaufes (Prüfung der Inhalte und Qualitätssicherung), zum Zeitpunkt der Abfrage.&lt;br&gt;&lt;br&gt;a) Konzeptstatus 0 „Not defined“ – Begriffe und Definitionen, welche noch keiner redaktionellen Prüfung bzw. Statuszuweisung durch die jeweiligen GBA-Redakteure unterlaufen sind.&lt;br&gt;&lt;br&gt;b) Konzeptstatus &lt;strong&gt;official use&lt;/strong&gt; – gültig im Sinne der GBA – Redaktionell geprüfter und gebräuchlicher, von der GBA empfohlener Begriff, wenn es sich um Konzepte (Begriffe) handelt, deren Erstellung die „Empfehlungen (Richtlinien) zur Handhabung der stratigraphischen Nomenklatur“ (Steininger &amp; Piller, 1999), bzw. den „North American Stratigraphic Code“ (NACSN, 2005) berücksichtigt. Dies trifft vor allem auf jüngst veröffentlichte Einheiten bzw. auf die Erstellung neuer Konzepte zu. &lt;br&gt;&lt;br&gt;c) Konzeptstatus &lt;strong&gt;informal use&lt;/strong&gt; – informelle Verwendung im Sinne der GBA – Redaktionell geprüfter und von der GBA nur informell verwendeter Begriff (der z.B. unzureichend beschrieben ist, von seiner Bedeutung überholt ist, einen lithologischen Begriff ohne Typlokalität darstellt, usw.), der aber eine wichtige Grundlage zur Interpretation der regionalen Geologie liefert.&lt;br&gt;&lt;br&gt;d) Konzeptstatus &lt;strong&gt;obsolete&lt;/strong&gt; – ungültig im Sinne der GBA – Redaktionell geprüfter und von der GBA nicht zur Verwendung empfohlener Begriff, der nicht unter die praktische Verwendung der Geologischen Bundesanstalt fällt, da dieser irreführend bis gar nicht definiert ist, oder nicht dem aktuellen wissenschaftlichen Stand entspricht. &lt;br&gt;</skos:definition>
	<dcterms:modified rdf:datatype="http://www.w3.org/2001/XMLSchema#dateTime">2019-10-01T11:33:48.624Z</dcterms:modified>
</rdf:Description>

<rdf:Description rdf:about="http://resource.geolba.ac.at/doc/154">
	<skos:definition xml:lang="de">Ja, das "Network Diagram" zeigt alle direkt verbundenen Thesaurus-Begriffe ausgehend von dem gewählten Begriff. Also alle SKOS-Relationen (broader, narrower und related) zwischen den einzelnen Konzepten innerhalb der semantischen Distanz von 1. Zusätzlich werden auch alle Relationen zu externen Konzepten (ohne Umrandung, in grau) gezeigt. Durch Anklicken eines Knotens, mit grauem Schatten hinterlegt, kann das Netzwerk um neue Knoten erweitert werden. Ein Doppelklick (oder Langklick für mobile Geräte) navigiert zur Detailansicht im Thesaurus. Zusätzlich stehen noch die Einstellungen, zum Umschalten in eine hierarchische Ansicht, entfernen von externen Knoten, und aktivieren von Webfarben, zur Verfügung.</skos:definition>
	<skos:definition xml:lang="en">Yes, the "Network Diagram" shows all directly related thesaurus concepts based on the selected concept. So all SKOS relations (broader, narrower and related) between the individual concepts within the semantic distance of 1. In addition, all relations to external concepts (without border, in gray color) are also shown. By clicking on a gray shadowed node the network can be extended by new nodes. A double-click (or long-click for mobile devices) navigates to the details view in the thesaurus. In addition, the settings for switching to a hierarchical view, removing external nodes, and activating web colors are available.</skos:definition>
	<dcterms:modified rdf:datatype="http://www.w3.org/2001/XMLSchema#dateTime">2019-10-01T14:29:34.963Z</dcterms:modified>
</rdf:Description>

<rdf:Description rdf:about="http://resource.geolba.ac.at/doc/85">
	<skos:definition xml:lang="de">Der DataViewer ist eine Erweiterung des GBA-Thesaurus (im Testbetrieb), die zeigt, wo und in welchen GBA-Geodatensätzen ein Konzept (Thesaurus-Begriff) verwendet wurde. Zu beachten ist, dass dabei nur die Datensätze (verschiedener Maßstäbe, derzeit 1:50.000 und 1:500.000) analysiert werden, die bereits nach INSPIRE harmonisiert wurden!&lt;br&gt;&lt;strong&gt;Hier ein Beispiel:&lt;/strong&gt; Beim Konzept &lt;a href='http://resource.geolba.ac.at/GeologicTimeScale/71'&gt;Oberjura&lt;/a&gt; - auf das Symbol &lt;i class="fas fa-map"&gt;&lt;/i&gt; 'DataViewer' klicken um die Anwendung zu öffnen.&lt;br&gt;Das Suchresultat ist in der Kartenansicht mit roten Punkten &lt;svg  xmlns='http://www.w3.org/2000/svg' width='8' height='10'&gt;&lt;circle fill='#FF4444' stroke-width='1' stroke='#CC0000' r='3' cy='4' cx='4'&gt;&lt;/circle&gt;&lt;/svg&gt; (für Abfragen, die eine maximale Darstellung nicht überschreiten) und roten Flächen visualisiert. Ein Klick auf einen Punkt zeigt den Original-Legendentext der zugrundeliegenden Publikation. Bei Abfragen nach Lithologie wird zusätzlich in der Darstellung der Punkte (ausgefüllt, leer) nach Hauptbestandteil &lt;svg  xmlns='http://www.w3.org/2000/svg' width='8' height='10'&gt;&lt;circle fill='#FF4444' stroke-width='1' stroke='#CC0000' r='3' cy='4' cx='4'&gt;&lt;/circle&gt;&lt;/svg&gt; (Proportion 'all', 'most abundant') und dem Vorkommen als Nebenbestandteil &lt;svg  xmlns='http://www.w3.org/2000/svg' width='8' height='10'&gt;&lt;circle fill='#FFFFFF' stroke-width='1' stroke='#CC0000' r='3' cy='4' cx='4'&gt;&lt;/circle&gt;&lt;/svg&gt; (Proportion 'present') unterschieden. Als Kartengrundlage ist derzeit zwischen der Verwaltungsgrundkarte (basemap.at), der 'Metallogenetischen Karte 1:500.000', und den Images der Geologischen Karte 1:50.000 zu wählen.&lt;br&gt;&lt;br&gt;In unserem Beispiel wäre die Abfrage: 'Wo gibt es geologische Einheiten aus dem Oberjura in Österreich?', exakter formuliert: 'Wo wurde das Konzept mit der URI &lt;a href='http://resource.geolba.ac.at/GeologicTimeScale/71'&gt;http://resource.geolba.ac.at/GeologicTimeScale/71&lt;/a&gt; (bevorzugter Begriff Oberjura, alternativ Malm, etc.) als ein (oder eines von mehreren) Eventalter einer Geologischen Einheit, zur Attributierung eines geologischen Datensatzes der GBA, bereits verwendet?'.&lt;br&gt;&lt;br&gt;In diese Suche können auch Datensätze einbezogen werden, die mit untergeordneten Begriffen (Default-Einstellung), übergeordneten oder verwandten Begriffen attributiert sind (semantische Erweiterung). Links von der Kartenansicht bietet der DataViewer eine weitere Filtermöglichkeit nach Konzepten, die in Kombination mit dem ursprünglich gewählten Konzept vorkommen - z.B. 'Geologische Einheiten im Oberjura mit lithologischem Bestandteil Mergel (inkl. Kalkmergel)' usw.. Die Zahl in Klammer zeigt die Anzahl der betreffenden Features (entsprechend den Legendenkästchen auf einer geologischen Karte), und der Info-Button ist zum Öffnen der Thesaurus-Detailseite des Konzeptes.&lt;br&gt;&lt;br&gt;Bei der Darstellung der ausgewählten bzw. gefilterten Konzepte im Bereich unter der Karte, bedeuten umrandete Begriffe, dass sie in der aktuellen Suche vorkommen bzw. der Auswahl hinzugefügt werden können. Begriffe ohne Umrandung stehen für die restlichen Konzepte im GBA-Thesaurus. Durch Klicken auf diese Begriffe kann der DataViewer mit einer neuerlichen Suche gestartet werden.&lt;br&gt;&lt;br&gt;Der DataViewer ermöglicht eine strukturierte Suche in den zentralen Datensätzen der GBA und ist als &lt;span style='color:red'&gt;ergänzende Information zu publizierten Kartenblättern&lt;/span&gt; zu verstehen und zu verwenden.</skos:definition>
	<skos:definition xml:lang="en">The Data Viewer is an extension of the GBA Thesaurus in test mode, showing where and in which GBA-spatial datasets a thesaurus concept was used. It should be noted that only these datasets (various scales, currently 1: 50,000 and 1: 500,000) are analyzed, which already are harmonized according to INSPIRE data model!&lt;br&gt;&lt;strong&gt;Example:&lt;/strong&gt; Open the concept &lt;a href='http://resource.geolba.ac.at/GeologicTimeScale/71'&gt;Upper Jurassic&lt;/a&gt; - see 'DataViewer' click on the symbol &lt;i class="fas fa-map"&gt;&lt;/i&gt;&lt;br&gt;The search result is visualized geographically in a map with red areas and red markers &lt;svg  xmlns='http://www.w3.org/2000/svg' width='8' height='10'&gt;&lt;circle fill='#FF4444' stroke-width='1' stroke='#CC0000' r='3' cy='4' cx='4'&gt;&lt;/circle&gt;&lt;/svg&gt; (for queries that do not exceed a maximum of display). Clicking a marker identifys the original legend text as published on a map. For lithological queries the representation of markers (filled or hollow) is distinguished by the proportion role as a main part &lt;svg  xmlns='http://www.w3.org/2000/svg' width='8' height='10'&gt;&lt;circle fill='#FF4444' stroke-width='1' stroke='#CC0000' r='3' cy='4' cx='4'&gt;&lt;/circle&gt;&lt;/svg&gt; (proportion 'all', 'most abundant') and the occurrence as a minor part &lt;svg  xmlns='http://www.w3.org/2000/svg' width='8' height='10'&gt;&lt;circle fill='#FFFFFF' stroke-width='1' stroke='#CC0000' r='3' cy='4' cx='4'&gt;&lt;/circle&gt;&lt;/svg&gt; (proportion 'present'). Regarding the base for the map display currently you can choose between 'basemap.at' (default setting), 'Metallogenetic Map 1: 500,000' and the images of the Geological Map 1:50,000.&lt;br&gt;&lt;br&gt;Referring to our example: 'Where are Geologic Units related to Upper Jurassic in Austria?', Formulated more exactly: 'Where a concept (with the URI &lt;a href='http://resource.geolba.ac.at/GeologicTimeScale/71'&gt;http://resource.geolba.ac.at/GeologicTimeScale/71&lt;/a&gt; - preferred label Upper Jurassic) already was used for attributing geological datasets of the GBA - as (the only one or one of several) Geologic Event(s) of a geological unit? '.&lt;br&gt;&lt;br&gt;Search results may include records attributed with narrower concepts (default setting), broader or related concepts (semantic approach). Left sided of the map (left bar) the Data Viewer provides more concepts to refine the search. Concepts which occur in combination with the concept selected originally - eg 'Geologic Units in Upper Jurassic with composition parts of Marl (incl. calcareous marl)', etc .. The number of relevant feature results (analogous to the count of map legend items) is put in parentheses. And an info button provides a link to the thesaurus concept page.&lt;br&gt;&lt;br&gt;Representing actually selected and filtered concepts (zone below the map), bordered (tagged) labels mean that they are part of the current selection, or they could be added to. Labels without a border stand for the remaining concepts completing GBA thesaurus hierarchy. Clicking on these labels the Data Viewer will be resetted performing a new concept query.&lt;br&gt;&lt;br&gt;The Data Viewer allows a structured query on the database with intended use &lt;span style='color:red'&gt;complementing the published information&lt;/span&gt; of geological maps.</skos:definition>
	<dcterms:modified rdf:datatype="http://www.w3.org/2001/XMLSchema#dateTime">2019-10-01T14:46:12.114Z</dcterms:modified>
</rdf:Description>

<rdf:Description rdf:about="http://resource.geolba.ac.at/doc/65">
	<dcterms:contributor rdf:resource="http://resource.geolba.ac.at/user/schmar"/>
	<skos:definition xml:lang="de">a) Suchbegriff (oder Wortteil) in das Suchfeld oben eingeben. Wird der gewünschte Begriff aus der Dropdown Liste angeklickt, so navigiert man direkt zum ausgewählten Konzept.&lt;br&gt; 
b) Wird hingegen der Suchbegriff jedoch mit Enter oder dem "Go!" Button bestätigt, so werden alle Begriffe sowie Beschreibungstexte durchsucht und in einer Liste präsentiert.&lt;br&gt;
c) Alternativ kann natürlich auch auf der Startseite &lt;a href="http://resource.geolba.ac.at/GeologicUnit/198"&gt;Lithostratigraphische Einheiten in Österreich&lt;/a&gt; ausgewählt werden und über die hierarchisch untergeordneten Begriffe das gewünschte Konzept gefunden werden.
</skos:definition>
	<skos:definition xml:lang="en">a) Enter the search term (or part of it) in the search bar above. If you click on the term from the drop-down list, you would navigate directly to the selected concept page.&lt;br&gt;
b) If the search term is confirmed by "Enter" or "Go!" button all labels and description texts are searched and presented in a results list.&lt;br&gt;
c) Alternatively, of course, on the start page &lt;a href="http://resource.geolba.ac.at/GeologicUnit/198"&gt;Lithostratigraphic Units in Austria&lt;/a&gt; can be selected and found on the hierarchically subordinate terms the desired concept.
</skos:definition>
	<dcterms:modified rdf:datatype="http://www.w3.org/2001/XMLSchema#dateTime">2019-11-05T14:04:51.037Z</dcterms:modified>
</rdf:Description>

<rdf:Description rdf:about="http://resource.geolba.ac.at/doc/83">
	<skos:definition xml:lang="en">If concepts have metadata for the geographical position in WGS84 latitude/longitude, a link &lt;i class="fas fa-map-pin" style="color:#029ACF;"&gt;&lt;/i&gt; provides the position in Google Maps. Actually this function is available for around 100 type section locations with Geologic Units.</skos:definition>
	<skos:definition xml:lang="de">Ist bei einem Konzept (Thesaurusbegriff) eine geografische Lage mit WGS84 Länge und Breite angegeben, dann kann diese über einen Link &lt;i class="fas fa-map-pin" style="color:#029ACF;"&gt;&lt;/i&gt; auf Google Maps angezeigt werden. Aktuell steht diese Funktion nur für ca. 100 Typlokalitäten (Lage des Typusprofils) Geologischer Einheiten zur Verfügung.</skos:definition>
	<skos:prefLabel xml:lang="de">Wofür ist type location (Anwendung) gedacht?</skos:prefLabel>
	<skos:prefLabel xml:lang="en">What is type location (application)?</skos:prefLabel>
	<dcterms:modified rdf:datatype="http://www.w3.org/2001/XMLSchema#dateTime">2019-11-12T14:25:14.944Z</dcterms:modified>
</rdf:Description>

<rdf:Description rdf:about="http://resource.geolba.ac.at/doc/52">
	<skos:definition xml:lang="de">&lt;p&gt;&lt;strong&gt;GBA-Thesaurus - &lt;br&gt;Das Online-Vokabular der Österreichischen Geologischen Bundesanstalt (GBA)&lt;/strong&gt;&lt;/p&gt;Finden sie Definitionen, Synonyme und Zitate von mehr als 2000 Begriffen zu geowissenschaftlichen Themenbereichen aus Karten- und Textpublikationen der Geologischen Bundesanstalt.&lt;br&gt;Visualisieren Sie die bedeutungsmäßige (semantische) Verknüpfung der Begriffe und verwenden Sie die Links zur Kennzeichnung und Vernetzung von geowissenschaftlichen Informationen.&lt;br&gt;Der GBA-Thesaurus unterstützt unsere gesetzliche Verpflichtung zur Umsetzung von &lt;a href="http://inspire.ec.europa.eu/registry/"&gt;INSPIRE&lt;/a&gt; und stellt publiziertes Wissen der GBA FachexpertInnen öffentlich zur Verfügung.&lt;br&gt;&lt;br&gt;&lt;strong&gt;Koordination:&lt;/strong&gt; Schiegl M.&lt;br&gt;&lt;strong&gt;Redaktion:&lt;/strong&gt; Hörfarter Ch.&lt;br&gt;&lt;strong&gt;Inhalte:&lt;/strong&gt;  ExpertInnenteams aus den Fachabteilungen Rohstoffe, Kristallingeologie und Sedimentgeologie - mit Beiträgen von: Auer Ch., Dobramysl L., Ebner M., Haider V., Hintersberger E., Huet B., Iglseder Ch., Krenmayr H., Linner M., Lipiarski P., Palzer-Khomenko M., Pavlik B., Reiser M., Reitner J., Schedl A., Schuster R., Weber L. &lt;br&gt;&lt;br&gt;Geologische Bundesanstalt&lt;br&gt;  Neulinggasse 38&lt;br&gt;  1030 Wien&lt;br&gt;&lt;br&gt;&lt;strong&gt;Kontakt:&lt;/strong&gt; &lt;a href="mailto:thesaurus@geologie.ac.at"&gt;thesaurus[et]geologie.ac.at&lt;/a&gt;&lt;br&gt;&lt;br&gt;&lt;a href="https://www.geologie.ac.at/datenschutz/"&gt;Datenschutzhinweise&lt;/a&gt; für die Benutzung der GBA-Websites&lt;br&gt;&lt;br&gt;Nicht die Antworten gefunden, die Sie erwartet haben?&lt;br&gt;
Werfen Sie auch einen Blick in unsere FAQs</skos:definition>
	<skos:definition xml:lang="en">&lt;p&gt;&lt;strong&gt;GBA-Thesaurus - &lt;br&gt;The online vocabulary of the Geological Survey of Austria&lt;/strong&gt;&lt;/p&gt;Find definitions, synonyms and citations from more than 2000 concepts on geoscientific topics from map and text publications of the Geological Survey.&lt;br&gt;Visualize the linked (semantic) context of concepts and use the relations to identify and link geoscientific information.&lt;br&gt;The GBA Thesaurus supports our legal obligation to implement &lt;a href="http://inspire.ec.europa.eu/registry/"&gt;INSPIRE&lt;/a&gt; and publishes publicly available knowledge of our experts.
&lt;br&gt;&lt;br&gt;&lt;strong&gt;Coordination:&lt;/strong&gt; Schiegl M.&lt;br&gt;&lt;strong&gt;Editor:&lt;/strong&gt; Hörfarter Ch.&lt;br&gt;&lt;strong&gt;Contents:&lt;/strong&gt; Teams of experts from departments of mineral resources, hard rock and sedimentary geology - with contributions from: Auer Ch., Dobramysl L., Ebner M., Haider V., Hintersberger E., Huet B., Iglseder Ch., Krenmayr H., Linner M., Lipiarski P., Palzer-Khomenko M., Pavlik B., Reiser M., Reitner J., Schedl A., Schuster R., Weber L. &lt;br&gt;&lt;br&gt; 
Geological Survey of Austria&lt;br&gt;  Neulinggasse 38&lt;br&gt;  1030 Wien&lt;br&gt;&lt;br&gt;&lt;strong&gt;Contact:&lt;/strong&gt; &lt;a href="mailto:thesaurus@geologie.ac.at"&gt;thesaurus[et]geologie.ac.at&lt;/a&gt;&lt;br&gt;&lt;br&gt;&lt;a href="https://www.geologie.ac.at/datenschutz/"&gt;Privacy Policy&lt;/a&gt; to use GBA websites&lt;br&gt;&lt;br&gt;Did not find the answers you expected?&lt;br&gt;Also take a look at our FAQs</skos:definition>
	<dcterms:modified rdf:datatype="http://www.w3.org/2001/XMLSchema#dateTime">2020-10-05T08:00:01.557Z</dcterms:modified>
</rdf:Description>

</rdf:RDF>